<?xml version="1.0"?>
<rdf:RDF xmlns="http://purl.obolibrary.org/obo/upheno/patterns/pattern.owl#"
     xml:base="http://purl.obolibrary.org/obo/upheno/patterns/pattern.owl"
     xmlns:obo="http://purl.obolibrary.org/obo/"
     xmlns:owl="http://www.w3.org/2002/07/owl#"
     xmlns:rdf="http://www.w3.org/1999/02/22-rdf-syntax-ns#"
     xmlns:xml="http://www.w3.org/XML/1998/namespace"
     xmlns:xsd="http://www.w3.org/2001/XMLSchema#"
     xmlns:rdfs="http://www.w3.org/2000/01/rdf-schema#"
     xmlns:terms="http://purl.org/dc/terms/"
     xmlns:oboInOwl="http://www.geneontology.org/formats/oboInOwl#">
    <owl:Ontology rdf:about="http://purl.obolibrary.org/obo/upheno/patterns/pattern.owl"/>
    


    <!-- 
    ///////////////////////////////////////////////////////////////////////////////////////
    //
    // Annotation properties
    //
    ///////////////////////////////////////////////////////////////////////////////////////
     -->

    


    <!-- http://purl.obolibrary.org/obo/IAO_0000115 -->

    <owl:AnnotationProperty rdf:about="http://purl.obolibrary.org/obo/IAO_0000115"/>
    


    <!-- http://purl.org/dc/terms/title -->

    <owl:AnnotationProperty rdf:about="http://purl.org/dc/terms/title"/>
    


    <!-- http://www.geneontology.org/formats/oboInOwl#hasBroadSynonym -->

    <owl:AnnotationProperty rdf:about="http://www.geneontology.org/formats/oboInOwl#hasBroadSynonym"/>
    


    <!-- http://www.geneontology.org/formats/oboInOwl#hasExactSynonym -->

    <owl:AnnotationProperty rdf:about="http://www.geneontology.org/formats/oboInOwl#hasExactSynonym"/>
    


    <!-- http://www.geneontology.org/formats/oboInOwl#hasNarrowSynonym -->

    <owl:AnnotationProperty rdf:about="http://www.geneontology.org/formats/oboInOwl#hasNarrowSynonym"/>
    


    <!-- http://www.geneontology.org/formats/oboInOwl#hasRelatedSynonym -->

    <owl:AnnotationProperty rdf:about="http://www.geneontology.org/formats/oboInOwl#hasRelatedSynonym"/>
    


    <!-- 
    ///////////////////////////////////////////////////////////////////////////////////////
    //
    // Classes
    //
    ///////////////////////////////////////////////////////////////////////////////////////
     -->

    


    <!-- http://purl.obolibrary.org/obo/upheno/patterns-dev/abnormalAbsenceOfAnatomicalEntity.yaml -->

    <owl:Class rdf:about="http://purl.obolibrary.org/obo/upheno/patterns-dev/abnormalAbsenceOfAnatomicalEntity.yaml">
        <rdfs:subClassOf rdf:resource="http://purl.obolibrary.org/obo/upheno/patterns-dev/abnormalNumberOfAnatomicalEntity.yaml"/>
        <obo:IAO_0000115>Absence of &apos;anatomical entity&apos;.</obo:IAO_0000115>
        <terms:title>abnormalAbsenceOfAnatomicalEntity</terms:title>
        <oboInOwl:hasExactSynonym>missing &apos;anatomical entity&apos;</oboInOwl:hasExactSynonym>
        <rdfs:label>absent &apos;anatomical entity&apos;</rdfs:label>
    </owl:Class>
    


    <!-- http://purl.obolibrary.org/obo/upheno/patterns-dev/abnormalAbsenceOfAnatomicalEntityDueToDegeneration.yaml -->

    <owl:Class rdf:about="http://purl.obolibrary.org/obo/upheno/patterns-dev/abnormalAbsenceOfAnatomicalEntityDueToDegeneration.yaml">
        <rdfs:subClassOf rdf:resource="http://purl.obolibrary.org/obo/upheno/patterns-dev/abnormalDegenerationOfAnatomicalEntity.yaml"/>
        <obo:IAO_0000115>Complete wasting (loss) of &apos;anatomical entity&apos; tissue that was once present.</obo:IAO_0000115>
        <terms:title>abnormalAbsenceOfAnatomicalEntityDueToDegeneration</terms:title>
        <oboInOwl:hasExactSynonym>loss of &apos;anatomical entity&apos; due to degeneration</oboInOwl:hasExactSynonym>
        <rdfs:label>missing &apos;anatomical entity&apos; due to degeneration</rdfs:label>
    </owl:Class>
    


    <!-- http://purl.obolibrary.org/obo/upheno/patterns-dev/abnormalAbsenceOfAnatomicalEntityInLocation.yaml -->

    <owl:Class rdf:about="http://purl.obolibrary.org/obo/upheno/patterns-dev/abnormalAbsenceOfAnatomicalEntityInLocation.yaml">
        <rdfs:subClassOf rdf:resource="http://purl.obolibrary.org/obo/upheno/patterns-dev/abnormalAbsenceOfAnatomicalEntity.yaml"/>
        <rdfs:subClassOf rdf:resource="http://purl.obolibrary.org/obo/upheno/patterns-dev/abnormalNumberOfAnatomicalEntityInLocation.yaml"/>
        <obo:IAO_0000115>Absence of the &apos;anatomical entity&apos; in the &apos;independent continuant&apos;.</obo:IAO_0000115>
        <terms:title>abnormalAbsenceOfAnatomicalEntityInLocation</terms:title>
        <oboInOwl:hasExactSynonym>Missing &apos;anatomical entity&apos; in the &apos;independent continuant&apos;</oboInOwl:hasExactSynonym>
        <rdfs:label>absent &apos;anatomical entity&apos; in the &apos;independent continuant&apos;</rdfs:label>
    </owl:Class>
    


    <!-- http://purl.obolibrary.org/obo/upheno/patterns-dev/abnormalAbsenceOfBehavior.yaml -->

    <owl:Class rdf:about="http://purl.obolibrary.org/obo/upheno/patterns-dev/abnormalAbsenceOfBehavior.yaml">
        <obo:IAO_0000115>Absence of &apos;behavior process&apos;.</obo:IAO_0000115>
        <terms:title>abnormalAbsenceOfBehavior</terms:title>
        <rdfs:label>absent &apos;behavior process&apos;</rdfs:label>
    </owl:Class>
    


    <!-- http://purl.obolibrary.org/obo/upheno/patterns-dev/abnormalAbsenceOfBiologicalProcess.yaml -->

    <owl:Class rdf:about="http://purl.obolibrary.org/obo/upheno/patterns-dev/abnormalAbsenceOfBiologicalProcess.yaml">
        <obo:IAO_0000115>Lack of &apos;biological process&apos;.</obo:IAO_0000115>
        <terms:title>abnormalAbsenceOfBiologicalProcess</terms:title>
        <rdfs:label>absent &apos;biological process&apos;</rdfs:label>
    </owl:Class>
    


    <!-- http://purl.obolibrary.org/obo/upheno/patterns-dev/abnormalAbsenceOfBiologicalProcessInLocation.yaml -->

    <owl:Class rdf:about="http://purl.obolibrary.org/obo/upheno/patterns-dev/abnormalAbsenceOfBiologicalProcessInLocation.yaml">
        <rdfs:subClassOf rdf:resource="http://purl.obolibrary.org/obo/upheno/patterns-dev/abnormalAbsenceOfBiologicalProcess.yaml"/>
        <obo:IAO_0000115>Absent or undetectable &apos;biological process&apos; in &apos;independent continuant&apos;.</obo:IAO_0000115>
        <terms:title>abnormalAbsenceOfBiologicalProcessInLocation</terms:title>
        <rdfs:label>absent &apos;biological process&apos; in &apos;independent continuant&apos;</rdfs:label>
    </owl:Class>
    


    <!-- http://purl.obolibrary.org/obo/upheno/patterns-dev/abnormalAbsenceOfChemicalEntity.yaml -->

    <owl:Class rdf:about="http://purl.obolibrary.org/obo/upheno/patterns-dev/abnormalAbsenceOfChemicalEntity.yaml">
        <rdfs:subClassOf rdf:resource="http://purl.obolibrary.org/obo/upheno/patterns/abnormalLevelOfChemicalEntity.yaml"/>
        <obo:IAO_0000115>Absent or undetectable level of &apos;chemical entity&apos;.</obo:IAO_0000115>
        <terms:title>abnormalAbsenceOfChemicalEntity</terms:title>
        <rdfs:label>absent &apos;chemical entity&apos;</rdfs:label>
    </owl:Class>
    


    <!-- http://purl.obolibrary.org/obo/upheno/patterns-dev/abnormalAbsenceOfChemicalEntityInLocation.yaml -->

    <owl:Class rdf:about="http://purl.obolibrary.org/obo/upheno/patterns-dev/abnormalAbsenceOfChemicalEntityInLocation.yaml">
        <rdfs:subClassOf rdf:resource="http://purl.obolibrary.org/obo/upheno/patterns-dev/abnormalAbsenceOfChemicalEntity.yaml"/>
        <rdfs:subClassOf rdf:resource="http://purl.obolibrary.org/obo/upheno/patterns/abnormalLevelOfChemicalEntityInLocation.yaml"/>
        <obo:IAO_0000115>Absent or undetectable level of &apos;chemical entity&apos; in &apos;independent continuant&apos;.</obo:IAO_0000115>
        <terms:title>abnormalAbsenceOfChemicalEntityInLocation</terms:title>
        <rdfs:label>absent &apos;chemical entity&apos; in &apos;independent continuant&apos;</rdfs:label>
    </owl:Class>
    


    <!-- http://purl.obolibrary.org/obo/upheno/patterns-dev/abnormalAbsenceOfMolecularFunction.yaml -->

    <owl:Class rdf:about="http://purl.obolibrary.org/obo/upheno/patterns-dev/abnormalAbsenceOfMolecularFunction.yaml">
        <obo:IAO_0000115>Absent or undetectable level of &apos;molecular function&apos;.</obo:IAO_0000115>
        <terms:title>abnormalAbsenceOfMolecularFunction</terms:title>
        <rdfs:label>absent &apos;molecular function&apos;</rdfs:label>
    </owl:Class>
    


    <!-- http://purl.obolibrary.org/obo/upheno/patterns-dev/abnormalAbsenceOfMotilityOfCellularComponentInLocation.yaml -->

    <owl:Class rdf:about="http://purl.obolibrary.org/obo/upheno/patterns-dev/abnormalAbsenceOfMotilityOfCellularComponentInLocation.yaml">
        <obo:IAO_0000115>Inability to move &apos;cellular component&apos; in &apos;independent continuant&apos;.</obo:IAO_0000115>
        <terms:title>abnormalAbsenceOfMotilityOfCellularComponentInLocation</terms:title>
        <oboInOwl:hasExactSynonym>immotile &apos;cellular component&apos; in &apos;independent continuant&apos;</oboInOwl:hasExactSynonym>
        <rdfs:label>absent &apos;cellular component&apos; motility in &apos;independent continuant&apos;</rdfs:label>
    </owl:Class>
    


    <!-- http://purl.obolibrary.org/obo/upheno/patterns-dev/abnormalAbsenceOfPigmentationOfAnatomicalEntity.yaml -->

    <owl:Class rdf:about="http://purl.obolibrary.org/obo/upheno/patterns-dev/abnormalAbsenceOfPigmentationOfAnatomicalEntity.yaml">
        <rdfs:subClassOf rdf:resource="http://purl.obolibrary.org/obo/upheno/patterns-dev/abnormalPigmentationOfAnatomicalEntity.yaml"/>
        <obo:IAO_0000115>complete loss of pigmenation of the &apos;anatomical entity&apos;.</obo:IAO_0000115>
        <terms:title>abnormalAbsenceOfPigmentationOfAnatomicalEntity</terms:title>
        <oboInOwl:hasExactSynonym>absence of pigment in the &apos;anatomical entity&apos;</oboInOwl:hasExactSynonym>
        <oboInOwl:hasExactSynonym>complete loss of pigmentation in the &apos;anatomical entity&apos;</oboInOwl:hasExactSynonym>
        <rdfs:label>unpigmented &apos;anatomical entity&apos;</rdfs:label>
    </owl:Class>
    


    <!-- http://purl.obolibrary.org/obo/upheno/patterns-dev/abnormalAbsenceOfProteinLocalizationInCellularComponent.yaml -->

    <owl:Class rdf:about="http://purl.obolibrary.org/obo/upheno/patterns-dev/abnormalAbsenceOfProteinLocalizationInCellularComponent.yaml">
        <rdfs:subClassOf rdf:resource="http://purl.obolibrary.org/obo/upheno/patterns-dev/abnormalAbsenceOfBiologicalProcess.yaml"/>
        <obo:IAO_0000115>Absent or undetectable protein localization &apos;cellular component&apos;.</obo:IAO_0000115>
        <terms:title>abnormalAbsenceOfProteinLocalizationInCellularComponent</terms:title>
        <rdfs:label>absent protein localization in &apos;cellular component&apos;</rdfs:label>
    </owl:Class>
    


    <!-- http://purl.obolibrary.org/obo/upheno/patterns-dev/abnormalAgenesisOfAnatomicalEntity.yaml -->

    <owl:Class rdf:about="http://purl.obolibrary.org/obo/upheno/patterns-dev/abnormalAgenesisOfAnatomicalEntity.yaml">
        <rdfs:subClassOf rdf:resource="http://purl.obolibrary.org/obo/upheno/patterns-dev/abnormalMorphologyOfAnatomicalEntity.yaml"/>
        <obo:IAO_0000115>Agenesis of &apos;anatomical entity&apos;.</obo:IAO_0000115>
        <terms:title>abnormalAgenesisOfAnatomicalEntity</terms:title>
        <rdfs:label>agenesis of &apos;anatomical entity&apos;</rdfs:label>
    </owl:Class>
    


    <!-- http://purl.obolibrary.org/obo/upheno/patterns-dev/abnormalAnatomicalEntityNotParts.yaml -->

    <owl:Class rdf:about="http://purl.obolibrary.org/obo/upheno/patterns-dev/abnormalAnatomicalEntityNotParts.yaml">
        <rdfs:subClassOf rdf:resource="http://purl.obolibrary.org/obo/upheno/patterns/abnormalAnatomicalEntity.yaml"/>
        <obo:IAO_0000115>Abnormality of &apos;anatomical entity&apos;.</obo:IAO_0000115>
        <terms:title>abnormalAnatomicalEntityNotParts</terms:title>
        <oboInOwl:hasExactSynonym>abnormality of &apos;anatomical entity&apos;</oboInOwl:hasExactSynonym>
        <rdfs:label>abnormal &apos;anatomical entity&apos;</rdfs:label>
    </owl:Class>
    


    <!-- http://purl.obolibrary.org/obo/upheno/patterns-dev/abnormalArrestedDevelopmentDuringStage.yaml -->

    <owl:Class rdf:about="http://purl.obolibrary.org/obo/upheno/patterns-dev/abnormalArrestedDevelopmentDuringStage.yaml">
        <rdfs:subClassOf rdf:resource="http://purl.obolibrary.org/obo/upheno/patterns-dev/abnormallyArrestedBiologicalProcess.yaml"/>
        <obo:IAO_0000115>Abnormal(ly) arrested (of) &apos;developmental_process&apos; in the &apos;life_cycle_stage&apos;.</obo:IAO_0000115>
        <terms:title>abnormalArrestedDevelopmentDuringStage</terms:title>
        <rdfs:label>arrested &apos;developmental_process&apos; during &apos;life_cycle_stage&apos;</rdfs:label>
    </owl:Class>
    


    <!-- http://purl.obolibrary.org/obo/upheno/patterns-dev/abnormalBehavior.yaml -->

    <owl:Class rdf:about="http://purl.obolibrary.org/obo/upheno/patterns-dev/abnormalBehavior.yaml">
        <obo:IAO_0000115>An anomaly in &apos;behavior process&apos;.</obo:IAO_0000115>
        <terms:title>abnormalBehavior</terms:title>
        <rdfs:label>abnormal &apos;behavior process&apos;</rdfs:label>
    </owl:Class>
    


    <!-- http://purl.obolibrary.org/obo/upheno/patterns-dev/abnormalBiologicalProcess.yaml -->

    <owl:Class rdf:about="http://purl.obolibrary.org/obo/upheno/patterns-dev/abnormalBiologicalProcess.yaml">
        <obo:IAO_0000115>Abnormal &apos;biological_process&apos;.</obo:IAO_0000115>
        <terms:title>abnormalBiologicalProcess</terms:title>
        <rdfs:label>abnormal &apos;biological_process&apos;</rdfs:label>
    </owl:Class>
    


    <!-- http://purl.obolibrary.org/obo/upheno/patterns-dev/abnormalBiologicalProcessInLocation.yaml -->

    <owl:Class rdf:about="http://purl.obolibrary.org/obo/upheno/patterns-dev/abnormalBiologicalProcessInLocation.yaml">
        <rdfs:subClassOf rdf:resource="http://purl.obolibrary.org/obo/upheno/patterns-dev/abnormalBiologicalProcess.yaml"/>
        <obo:IAO_0000115>An abnormality of the &apos;biological process&apos; in &apos;independent continuant&apos;.</obo:IAO_0000115>
        <terms:title>abnormalBiologicalProcessInLocation</terms:title>
        <rdfs:label>abnormal &apos;biological process&apos; in &apos;independent continuant&apos;</rdfs:label>
    </owl:Class>
    


    <!-- http://purl.obolibrary.org/obo/upheno/patterns-dev/abnormalCellDifferentiation.yaml -->

    <owl:Class rdf:about="http://purl.obolibrary.org/obo/upheno/patterns-dev/abnormalCellDifferentiation.yaml">
        <rdfs:subClassOf rdf:resource="http://purl.obolibrary.org/obo/upheno/patterns-dev/abnormalDevelopmentOfAnatomicalEntity.yaml"/>
        <obo:IAO_0000115>An abnormality in the cell differentiation of the &apos;cell type&apos;.</obo:IAO_0000115>
        <terms:title>abnormalCellDifferentiation</terms:title>
        <rdfs:label>abnormal &apos;cell type&apos; cell differentiation</rdfs:label>
    </owl:Class>
    


    <!-- http://purl.obolibrary.org/obo/upheno/patterns-dev/abnormalCellProliferationActingOnCellsOfType.yaml -->

    <owl:Class rdf:about="http://purl.obolibrary.org/obo/upheno/patterns-dev/abnormalCellProliferationActingOnCellsOfType.yaml">
        <rdfs:subClassOf rdf:resource="http://purl.obolibrary.org/obo/upheno/patterns-dev/abnormalBiologicalProcess.yaml"/>
        <obo:IAO_0000115>Abnormal proliferation of &apos;cell&apos;.</obo:IAO_0000115>
        <terms:title>abnormalCellProliferationActingOnCellsOfType</terms:title>
        <rdfs:label>abnormal &apos;cell&apos; proliferation</rdfs:label>
    </owl:Class>
    


    <!-- http://purl.obolibrary.org/obo/upheno/patterns-dev/abnormalCellProliferationActingOnCellsOfTypeInLocation.yaml -->

    <owl:Class rdf:about="http://purl.obolibrary.org/obo/upheno/patterns-dev/abnormalCellProliferationActingOnCellsOfTypeInLocation.yaml">
        <rdfs:subClassOf rdf:resource="http://purl.obolibrary.org/obo/upheno/patterns-dev/abnormalCellProliferationActingOnCellsOfType.yaml"/>
        <rdfs:subClassOf rdf:resource="http://purl.obolibrary.org/obo/upheno/patterns-dev/abnormalCellProliferationInAnatomicalEntity.yaml"/>
        <obo:IAO_0000115>Abnormal proliferation of &apos;cell&apos; in &apos;anatomical entity&apos;.</obo:IAO_0000115>
        <terms:title>abnormalCellProliferationActingOnCellsOfTypeInLocation</terms:title>
        <rdfs:label>abnormal &apos;cell&apos; proliferation in &apos;anatomical entity&apos;</rdfs:label>
    </owl:Class>
    


    <!-- http://purl.obolibrary.org/obo/upheno/patterns-dev/abnormalCellProliferationInAnatomicalEntity.yaml -->

    <owl:Class rdf:about="http://purl.obolibrary.org/obo/upheno/patterns-dev/abnormalCellProliferationInAnatomicalEntity.yaml">
        <rdfs:subClassOf rdf:resource="http://purl.obolibrary.org/obo/upheno/patterns-dev/abnormalBiologicalProcessInLocation.yaml"/>
        <obo:IAO_0000115>Abnormal cell proliferation in &apos;anatomical_entity&apos;.</obo:IAO_0000115>
        <terms:title>abnormalCellProliferationInAnatomicalEntity</terms:title>
        <rdfs:label>abnormal cell proliferation in &apos;anatomical_entity&apos;</rdfs:label>
    </owl:Class>
    


    <!-- http://purl.obolibrary.org/obo/upheno/patterns-dev/abnormalCellularComponentProcess.yaml -->

    <owl:Class rdf:about="http://purl.obolibrary.org/obo/upheno/patterns-dev/abnormalCellularComponentProcess.yaml">
        <rdfs:subClassOf rdf:resource="http://purl.obolibrary.org/obo/upheno/patterns-dev/abnormalBiologicalProcess.yaml"/>
        <obo:IAO_0000115>Abnormal &apos;biological process&apos; involving the active participant &apos;cellular component&apos;.</obo:IAO_0000115>
        <terms:title>abnormalCellularComponentProcess</terms:title>
        <rdfs:label>abnormal &apos;biological process&apos; involving &apos;cellular component&apos;</rdfs:label>
    </owl:Class>
    


    <!-- http://purl.obolibrary.org/obo/upheno/patterns-dev/abnormalCoilingOfAnatomicalEntity.yaml -->

    <owl:Class rdf:about="http://purl.obolibrary.org/obo/upheno/patterns-dev/abnormalCoilingOfAnatomicalEntity.yaml">
        <rdfs:subClassOf rdf:resource="http://purl.obolibrary.org/obo/upheno/patterns-dev/abnormalShapeOfAnatomicalEntityByShapeType.yaml"/>
        <obo:IAO_0000115>Any abnormal coiling of the &apos;anatomical entity&apos;.</obo:IAO_0000115>
        <terms:title>abnormalCoilingOfAnatomicalEntity</terms:title>
        <oboInOwl:hasExactSynonym>abnormal coiling of &apos;anatomical entity&apos;</oboInOwl:hasExactSynonym>
        <rdfs:label>abnormally coiled &apos;anatomical entity&apos;</rdfs:label>
    </owl:Class>
    


    <!-- http://purl.obolibrary.org/obo/upheno/patterns-dev/abnormalColorOfAnatomicalEntity.yaml -->

    <owl:Class rdf:about="http://purl.obolibrary.org/obo/upheno/patterns-dev/abnormalColorOfAnatomicalEntity.yaml">
        <rdfs:subClassOf rdf:resource="http://purl.obolibrary.org/obo/upheno/patterns-dev/abnormalMorphologyOfAnatomicalEntity.yaml"/>
        <obo:IAO_0000115>Abnormal color of &apos;anatomical entity&apos;.</obo:IAO_0000115>
        <terms:title>abnormalColorOfAnatomicalEntity</terms:title>
        <oboInOwl:hasExactSynonym>abnormal &apos;anatomical entity&apos; colour</oboInOwl:hasExactSynonym>
        <oboInOwl:hasExactSynonym>abnormality of &apos;anatomical entity&apos; color</oboInOwl:hasExactSynonym>
        <rdfs:label>abnormal &apos;anatomical entity&apos; color</rdfs:label>
    </owl:Class>
    


    <!-- http://purl.obolibrary.org/obo/upheno/patterns-dev/abnormalColorOfAnatomicalEntityByColor.yaml -->

    <owl:Class rdf:about="http://purl.obolibrary.org/obo/upheno/patterns-dev/abnormalColorOfAnatomicalEntityByColor.yaml">
        <rdfs:subClassOf rdf:resource="http://purl.obolibrary.org/obo/upheno/patterns-dev/abnormalMorphologyOfAnatomicalEntity.yaml"/>
        <obo:IAO_0000115>An abnormally &apos;color&apos; &apos;anatomical_entity&apos;.</obo:IAO_0000115>
        <terms:title>abnormalColorOfAnatomicalEntityByColor</terms:title>
        <oboInOwl:hasExactSynonym>&apos;color&apos; type abnormality of &apos;anatomical_entity&apos; color</oboInOwl:hasExactSynonym>
        <oboInOwl:hasExactSynonym>abnormal &apos;color&apos; color of &apos;anatomical_entity&apos;</oboInOwl:hasExactSynonym>
        <rdfs:label>abnormally &apos;color&apos; &apos;anatomical_entity&apos; color</rdfs:label>
    </owl:Class>
    


    <!-- http://purl.obolibrary.org/obo/upheno/patterns-dev/abnormalConcentrationOfChemicalEntity.yaml -->

    <owl:Class rdf:about="http://purl.obolibrary.org/obo/upheno/patterns-dev/abnormalConcentrationOfChemicalEntity.yaml">
        <rdfs:subClassOf rdf:resource="http://purl.obolibrary.org/obo/upheno/patterns/abnormalLevelOfChemicalEntity.yaml"/>
        <obo:IAO_0000115>An abnormal concentration of chemical.</obo:IAO_0000115>
        <terms:title>abnormalConcentrationOfChemicalEntity</terms:title>
        <rdfs:label>abnormal chemical concentration</rdfs:label>
    </owl:Class>
    


    <!-- http://purl.obolibrary.org/obo/upheno/patterns-dev/abnormalConcentrationOfChemicalEntityInLocation.yaml -->

    <owl:Class rdf:about="http://purl.obolibrary.org/obo/upheno/patterns-dev/abnormalConcentrationOfChemicalEntityInLocation.yaml">
        <rdfs:subClassOf rdf:resource="http://purl.obolibrary.org/obo/upheno/patterns-dev/abnormalConcentrationOfChemicalEntity.yaml"/>
        <rdfs:subClassOf rdf:resource="http://purl.obolibrary.org/obo/upheno/patterns/abnormalLevelOfChemicalEntityInLocation.yaml"/>
        <obo:IAO_0000115>An abnormal concentration of chemical in &apos;independent continuant&apos;.</obo:IAO_0000115>
        <terms:title>abnormalConcentrationOfChemicalEntityInLocation</terms:title>
        <rdfs:label>abnormal chemical concentration in &apos;independent continuant&apos;</rdfs:label>
    </owl:Class>
    


    <!-- http://purl.obolibrary.org/obo/upheno/patterns-dev/abnormalConstrictionOfAnatomicalEntity.yaml -->

    <owl:Class rdf:about="http://purl.obolibrary.org/obo/upheno/patterns-dev/abnormalConstrictionOfAnatomicalEntity.yaml">
        <rdfs:subClassOf rdf:resource="http://purl.obolibrary.org/obo/upheno/patterns-dev/abnormalMorphologyOfPartOfAnatomicalEntity.yaml"/>
        <obo:IAO_0000115>An &apos;anatomical entity&apos; that is being drawn together, compressed or squeezed physically.</obo:IAO_0000115>
        <terms:title>abnormalConstrictionOfAnatomicalEntity</terms:title>
        <oboInOwl:hasExactSynonym>Constriction of the &apos;anatomical entity&apos;</oboInOwl:hasExactSynonym>
        <rdfs:label>constricted &apos;anatomical entity&apos;</rdfs:label>
    </owl:Class>
    


    <!-- http://purl.obolibrary.org/obo/upheno/patterns-dev/abnormalDegenerationOfAnatomicalEntity.yaml -->

    <owl:Class rdf:about="http://purl.obolibrary.org/obo/upheno/patterns-dev/abnormalDegenerationOfAnatomicalEntity.yaml">
        <rdfs:subClassOf rdf:resource="http://purl.obolibrary.org/obo/upheno/patterns-dev/abnormalMorphologyOfAnatomicalEntity.yaml"/>
        <obo:IAO_0000115>Partial or complete degeneration of &apos;anatomical entity&apos; tissue that was once present.</obo:IAO_0000115>
        <terms:title>abnormalDegenerationOfAnatomicalEntity</terms:title>
        <oboInOwl:hasExactSynonym>degeneration of the &apos;anatomical entity&apos;</oboInOwl:hasExactSynonym>
        <rdfs:label>&apos;anatomical entity&apos; degeneration</rdfs:label>
    </owl:Class>
    


    <!-- http://purl.obolibrary.org/obo/upheno/patterns-dev/abnormalDegenerationOfAnatomicalEntityInLocation.yaml -->

    <owl:Class rdf:about="http://purl.obolibrary.org/obo/upheno/patterns-dev/abnormalDegenerationOfAnatomicalEntityInLocation.yaml">
        <rdfs:subClassOf rdf:resource="http://purl.obolibrary.org/obo/upheno/patterns-dev/abnormalDegenerationOfAnatomicalEntity.yaml"/>
        <rdfs:subClassOf rdf:resource="http://purl.obolibrary.org/obo/upheno/patterns-dev/abnormalMorphologyOfAnatomicalEntityInLocation.yaml"/>
        <obo:IAO_0000115>Partial or complete degeneration of &apos;anatomical entity&apos; tissue in the &apos;independent continuant&apos; that was once present.</obo:IAO_0000115>
        <terms:title>abnormalDegenerationOfAnatomicalEntityInLocation</terms:title>
        <oboInOwl:hasExactSynonym>degeneration of the &apos;anatomical entity&apos; in &apos;independent continuant&apos;</oboInOwl:hasExactSynonym>
        <rdfs:label>&apos;anatomical entity&apos; degeneration in &apos;independent continuant&apos;</rdfs:label>
    </owl:Class>
    


    <!-- http://purl.obolibrary.org/obo/upheno/patterns-dev/abnormalDegenerationOfCellularComponent.yaml -->

    <owl:Class rdf:about="http://purl.obolibrary.org/obo/upheno/patterns-dev/abnormalDegenerationOfCellularComponent.yaml">
        <rdfs:subClassOf rdf:resource="http://purl.obolibrary.org/obo/upheno/patterns-dev/abnormalMorphologyOfCellularComponent.yaml"/>
        <obo:IAO_0000115>Partial or complete degeneration of &apos;cellular component&apos;.</obo:IAO_0000115>
        <terms:title>abnormalDegenerationOfCellularComponent</terms:title>
        <oboInOwl:hasExactSynonym>degeneration of the &apos;cellular component&apos;</oboInOwl:hasExactSynonym>
        <rdfs:label>&apos;cellular component&apos; degeneration</rdfs:label>
    </owl:Class>
    


    <!-- http://purl.obolibrary.org/obo/upheno/patterns-dev/abnormalDegenerationOfCellularComponentInLocation.yaml -->

    <owl:Class rdf:about="http://purl.obolibrary.org/obo/upheno/patterns-dev/abnormalDegenerationOfCellularComponentInLocation.yaml">
        <rdfs:subClassOf rdf:resource="http://purl.obolibrary.org/obo/upheno/patterns-dev/abnormalDegenerationOfCellularComponent.yaml"/>
        <obo:IAO_0000115>Partial or complete degeneration of &apos;cellular component&apos; tissue in the &apos;independent continuant&apos; that was once present.</obo:IAO_0000115>
        <terms:title>abnormalDegenerationOfCellularComponentInLocation</terms:title>
        <oboInOwl:hasExactSynonym>degeneration of the &apos;cellular component&apos; in &apos;independent continuant&apos;</oboInOwl:hasExactSynonym>
        <rdfs:label>&apos;cellular component&apos; degeneration in &apos;independent continuant&apos;</rdfs:label>
    </owl:Class>
    


    <!-- http://purl.obolibrary.org/obo/upheno/patterns-dev/abnormalDevelopmentOfAnatomicalEntity.yaml -->

    <owl:Class rdf:about="http://purl.obolibrary.org/obo/upheno/patterns-dev/abnormalDevelopmentOfAnatomicalEntity.yaml">
        <rdfs:subClassOf rdf:resource="http://purl.obolibrary.org/obo/upheno/patterns-dev/abnormalBiologicalProcess.yaml"/>
        <obo:IAO_0000115>An abnormal development of the &apos;anatomical entity&apos;.</obo:IAO_0000115>
        <terms:title>abnormalDevelopmentOfAnatomicalEntity</terms:title>
        <rdfs:label>abnormal development of &apos;anatomical entity&apos;</rdfs:label>
    </owl:Class>
    


    <!-- http://purl.obolibrary.org/obo/upheno/patterns-dev/abnormalDistanceBetweenAnatomicalEntities.yaml -->

    <owl:Class rdf:about="http://purl.obolibrary.org/obo/upheno/patterns-dev/abnormalDistanceBetweenAnatomicalEntities.yaml">
        <rdfs:subClassOf rdf:resource="http://purl.obolibrary.org/obo/upheno/patterns-dev/abnormalAnatomicalEntityNotParts.yaml"/>
        <obo:IAO_0000115>abnormal distance between &apos;anatomical_entity1&apos; and &apos;anatomical_entity2&apos;.</obo:IAO_0000115>
        <terms:title>abnormalDistanceBetweenAnatomicalEntities</terms:title>
        <oboInOwl:hasExactSynonym>abnormal distance between &apos;anatomical_entity1&apos; and &apos;anatomical_entity2&apos;</oboInOwl:hasExactSynonym>
        <oboInOwl:hasExactSynonym>distance abnormal between &apos;anatomical_entity1&apos; and &apos;anatomical_entity2&apos;</oboInOwl:hasExactSynonym>
        <rdfs:label>abnormal distance between &apos;anatomical_entity1&apos; and &apos;anatomical_entity2&apos;</rdfs:label>
    </owl:Class>
    


    <!-- http://purl.obolibrary.org/obo/upheno/patterns-dev/abnormalEfficacyOfProteinLocalizationInCellularComponent.yaml -->

    <owl:Class rdf:about="http://purl.obolibrary.org/obo/upheno/patterns-dev/abnormalEfficacyOfProteinLocalizationInCellularComponent.yaml">
        <rdfs:subClassOf rdf:resource="http://purl.obolibrary.org/obo/upheno/patterns-dev/abnormalBiologicalProcess.yaml"/>
        <obo:IAO_0000115>Abnormal protein localization &apos;cellular component&apos;.</obo:IAO_0000115>
        <terms:title>abnormalEfficacyOfProteinLocalizationInCellularComponent</terms:title>
        <rdfs:label>abnormal protein localization in &apos;cellular component&apos;</rdfs:label>
    </owl:Class>
    


    <!-- http://purl.obolibrary.org/obo/upheno/patterns-dev/abnormalFunctionalityOfAnatomicalEntity.yaml -->

    <owl:Class rdf:about="http://purl.obolibrary.org/obo/upheno/patterns-dev/abnormalFunctionalityOfAnatomicalEntity.yaml">
        <rdfs:subClassOf rdf:resource="http://purl.obolibrary.org/obo/upheno/patterns-dev/abnormalAnatomicalEntityNotParts.yaml"/>
        <rdfs:subClassOf rdf:resource="http://purl.obolibrary.org/obo/upheno/patterns-dev/abnormalFunctionalityOfPartOfAnatomicalEntity.yaml"/>
        <obo:IAO_0000115>Any functional anomaly of the &apos;anatomical entity&apos;.</obo:IAO_0000115>
        <terms:title>abnormalFunctionalityOfAnatomicalEntity</terms:title>
        <rdfs:label>abnormality of &apos;anatomical entity&apos; physiology</rdfs:label>
    </owl:Class>
    


    <!-- http://purl.obolibrary.org/obo/upheno/patterns-dev/abnormalFunctionalityOfCellularComponent.yaml -->

    <owl:Class rdf:about="http://purl.obolibrary.org/obo/upheno/patterns-dev/abnormalFunctionalityOfCellularComponent.yaml">
        <rdfs:subClassOf rdf:resource="http://purl.obolibrary.org/obo/upheno/patterns/abnormalCellularComponent.yaml"/>
        <obo:IAO_0000115>Any functional anomaly of the &apos;cellular component&apos;.</obo:IAO_0000115>
        <terms:title>abnormalFunctionalityOfCellularComponent</terms:title>
        <rdfs:label>abnormality of &apos;cellular component&apos; function</rdfs:label>
    </owl:Class>
    


    <!-- http://purl.obolibrary.org/obo/upheno/patterns-dev/abnormalFunctionalityOfPartOfAnatomicalEntity.yaml -->

    <owl:Class rdf:about="http://purl.obolibrary.org/obo/upheno/patterns-dev/abnormalFunctionalityOfPartOfAnatomicalEntity.yaml">
        <rdfs:subClassOf rdf:resource="http://purl.obolibrary.org/obo/upheno/patterns/abnormalAnatomicalEntity.yaml"/>
        <obo:IAO_0000115>Any functional anomaly of the &apos;anatomical entity&apos; or one of its parts.</obo:IAO_0000115>
        <terms:title>abnormalFunctionalityOfPartOfAnatomicalEntity</terms:title>
        <rdfs:label>abnormality of &apos;anatomical entity&apos; physiology</rdfs:label>
    </owl:Class>
    


    <!-- http://purl.obolibrary.org/obo/upheno/patterns-dev/abnormalHasExtraPartsOfTypeAnatomicalEntity.yaml -->

    <owl:Class rdf:about="http://purl.obolibrary.org/obo/upheno/patterns-dev/abnormalHasExtraPartsOfTypeAnatomicalEntity.yaml">
        <rdfs:subClassOf rdf:resource="http://purl.obolibrary.org/obo/upheno/patterns-dev/abnormalMorphologyOfAnatomicalEntity.yaml"/>
        <rdfs:subClassOf rdf:resource="http://purl.obolibrary.org/obo/upheno/patterns-dev/abnormallyIncreasedNumberOfAnatomicalEntity.yaml"/>
        <obo:IAO_0000115>Any structural anomaly that causes there to be extra parts of type &apos;anatomical entity&apos;.</obo:IAO_0000115>
        <terms:title>abnormalHasExtraPartsOfTypeAnatomicalEntity</terms:title>
        <oboInOwl:hasExactSynonym>extra &apos;anatomical entity&apos;s</oboInOwl:hasExactSynonym>
        <rdfs:label>has extra parts of type &apos;anatomical entity&apos;</rdfs:label>
    </owl:Class>
    


    <!-- http://purl.obolibrary.org/obo/upheno/patterns-dev/abnormalHasFewerPartsOfTypeAnatomicalEntity.yaml -->

    <owl:Class rdf:about="http://purl.obolibrary.org/obo/upheno/patterns-dev/abnormalHasFewerPartsOfTypeAnatomicalEntity.yaml">
        <rdfs:subClassOf rdf:resource="http://purl.obolibrary.org/obo/upheno/patterns-dev/abnormalMorphologyOfAnatomicalEntity.yaml"/>
        <rdfs:subClassOf rdf:resource="http://purl.obolibrary.org/obo/upheno/patterns-dev/abnormallyDecreasedNumberOfAnatomicalEntity.yaml"/>
        <obo:IAO_0000115>Any structural anomaly of &apos;anatomical entity&apos; that causes there to be fewer parts of type &apos;anatomical entity&apos;.</obo:IAO_0000115>
        <terms:title>abnormalHasFewerPartsOfTypeAnatomicalEntity</terms:title>
        <oboInOwl:hasExactSynonym>fewer &apos;anatomical entity&apos;s in &apos;anatomical entity&apos;</oboInOwl:hasExactSynonym>
        <rdfs:label>&apos;anatomical entity&apos; that has fewer parts of type &apos;anatomical entity&apos;</rdfs:label>
    </owl:Class>
    


    <!-- http://purl.obolibrary.org/obo/upheno/patterns-dev/abnormalHeightOfAnatomicalEntity.yaml -->

    <owl:Class rdf:about="http://purl.obolibrary.org/obo/upheno/patterns-dev/abnormalHeightOfAnatomicalEntity.yaml">
        <rdfs:subClassOf rdf:resource="http://purl.obolibrary.org/obo/upheno/patterns-dev/abnormalSizeOfAnatomicalEntity.yaml"/>
        <obo:IAO_0000115>Deviation from the norm of &apos;anatomical entity&apos; height with respect to that which is expected according to age and gender norms.</obo:IAO_0000115>
        <terms:title>abnormalHeightOfAnatomicalEntity</terms:title>
        <oboInOwl:hasExactSynonym>Abnormal &apos;anatomical entity&apos; height</oboInOwl:hasExactSynonym>
        <rdfs:label>abnormality of &apos;anatomical entity&apos; height</rdfs:label>
    </owl:Class>
    


    <!-- http://purl.obolibrary.org/obo/upheno/patterns-dev/abnormalLengthOfAnatomicalEntity.yaml -->

    <owl:Class rdf:about="http://purl.obolibrary.org/obo/upheno/patterns-dev/abnormalLengthOfAnatomicalEntity.yaml">
        <rdfs:subClassOf rdf:resource="http://purl.obolibrary.org/obo/upheno/patterns-dev/abnormalSizeOfAnatomicalEntity.yaml"/>
        <obo:IAO_0000115>Abnormal length of &apos;anatomical_entity&apos;.</obo:IAO_0000115>
        <terms:title>abnormalLengthOfAnatomicalEntity</terms:title>
        <oboInOwl:hasExactSynonym>abnormal length of &apos;anatomical_entity&apos;</oboInOwl:hasExactSynonym>
        <rdfs:label>abnormal &apos;anatomical_entity&apos; length</rdfs:label>
    </owl:Class>
    


    <!-- http://purl.obolibrary.org/obo/upheno/patterns-dev/abnormalLevelOfChemicalEntityWithRole.yaml -->

    <owl:Class rdf:about="http://purl.obolibrary.org/obo/upheno/patterns-dev/abnormalLevelOfChemicalEntityWithRole.yaml">
        <rdfs:subClassOf rdf:resource="http://purl.obolibrary.org/obo/upheno/patterns/abnormalLevelOfChemicalEntity.yaml"/>
        <obo:IAO_0000115>An abnormal amount of role.</obo:IAO_0000115>
        <terms:title>abnormalLevelOfChemicalEntityWithRole</terms:title>
        <rdfs:label>abnormal role level</rdfs:label>
    </owl:Class>
    


    <!-- http://purl.obolibrary.org/obo/upheno/patterns-dev/abnormalLevelOfChemicalEntityWithRoleInLocation.yaml -->

    <owl:Class rdf:about="http://purl.obolibrary.org/obo/upheno/patterns-dev/abnormalLevelOfChemicalEntityWithRoleInLocation.yaml">
        <rdfs:subClassOf rdf:resource="http://purl.obolibrary.org/obo/upheno/patterns-dev/abnormalLevelOfChemicalEntityWithRole.yaml"/>
        <rdfs:subClassOf rdf:resource="http://purl.obolibrary.org/obo/upheno/patterns/abnormalLevelOfChemicalEntityInLocation.yaml"/>
        <obo:IAO_0000115>An abnormal amount of role in the &apos;independent continuant&apos;.</obo:IAO_0000115>
        <terms:title>abnormalLevelOfChemicalEntityWithRoleInLocation</terms:title>
        <rdfs:label>abnormal role &apos;independent continuant&apos; level</rdfs:label>
    </owl:Class>
    


    <!-- http://purl.obolibrary.org/obo/upheno/patterns-dev/abnormalMassDensityOfAnatomicalEntity.yaml -->

    <owl:Class rdf:about="http://purl.obolibrary.org/obo/upheno/patterns-dev/abnormalMassDensityOfAnatomicalEntity.yaml">
        <rdfs:subClassOf rdf:resource="http://purl.obolibrary.org/obo/upheno/patterns-dev/abnormalAnatomicalEntityNotParts.yaml"/>
        <obo:IAO_0000115>Abnormal mass density (mass per unit volume) of &apos;anatomical_entity&apos;.</obo:IAO_0000115>
        <terms:title>abnormalMassDensityOfAnatomicalEntity</terms:title>
        <oboInOwl:hasExactSynonym>abnormal mass density of &apos;anatomical_entity&apos;</oboInOwl:hasExactSynonym>
        <rdfs:label>abnormal &apos;anatomical_entity&apos; mass density</rdfs:label>
    </owl:Class>
    


    <!-- http://purl.obolibrary.org/obo/upheno/patterns-dev/abnormalMassDensityOfAnatomicalEntityInLocation.yaml -->

    <owl:Class rdf:about="http://purl.obolibrary.org/obo/upheno/patterns-dev/abnormalMassDensityOfAnatomicalEntityInLocation.yaml">
        <rdfs:subClassOf rdf:resource="http://purl.obolibrary.org/obo/upheno/patterns-dev/abnormalMassDensityOfAnatomicalEntity.yaml"/>
        <obo:IAO_0000115>Abnormal mass density (mass per unit volume) of &apos;anatomical_entity&apos; of &apos;independent_continuant&apos;.</obo:IAO_0000115>
        <terms:title>abnormalMassDensityOfAnatomicalEntityInLocation.yaml</terms:title>
        <oboInOwl:hasExactSynonym>abnormal mass density of &apos;anatomical_entity&apos; of &apos;independent_continuant&apos;</oboInOwl:hasExactSynonym>
        <rdfs:label>abnormal &apos;anatomical_entity&apos; of &apos;independent_continuant&apos; mass density</rdfs:label>
    </owl:Class>
    


    <!-- http://purl.obolibrary.org/obo/upheno/patterns-dev/abnormalMobilityOfAnatomicalEntity.yaml -->

    <owl:Class rdf:about="http://purl.obolibrary.org/obo/upheno/patterns-dev/abnormalMobilityOfAnatomicalEntity.yaml">
        <rdfs:subClassOf rdf:resource="http://purl.obolibrary.org/obo/upheno/patterns-dev/abnormalAnatomicalEntityNotParts.yaml"/>
        <obo:IAO_0000115>anomaly in the ability to move &apos;anatomical entity&apos;.</obo:IAO_0000115>
        <terms:title>abnormalMobilityOfAnatomicalEntity</terms:title>
        <rdfs:label>abnormal &apos;anatomical entity&apos; mobility</rdfs:label>
    </owl:Class>
    


    <!-- http://purl.obolibrary.org/obo/upheno/patterns-dev/abnormalMolecularFunction.yaml -->

    <owl:Class rdf:about="http://purl.obolibrary.org/obo/upheno/patterns-dev/abnormalMolecularFunction.yaml">
        <obo:IAO_0000115>Abnormal &apos;molecular function&apos;.</obo:IAO_0000115>
        <terms:title>abnormalMolecularFunction</terms:title>
        <rdfs:label>abnormal &apos;molecular function&apos;</rdfs:label>
    </owl:Class>
    


    <!-- http://purl.obolibrary.org/obo/upheno/patterns-dev/abnormalMorphologyOfAnatomicalEntity.yaml -->

    <owl:Class rdf:about="http://purl.obolibrary.org/obo/upheno/patterns-dev/abnormalMorphologyOfAnatomicalEntity.yaml">
        <rdfs:subClassOf rdf:resource="http://purl.obolibrary.org/obo/upheno/patterns-dev/abnormalAnatomicalEntityNotParts.yaml"/>
        <rdfs:subClassOf rdf:resource="http://purl.obolibrary.org/obo/upheno/patterns-dev/abnormalMorphologyOfPartOfAnatomicalEntity.yaml"/>
        <obo:IAO_0000115>Any unspecified morphological anomaly of the &apos;anatomical entity&apos;, such as, for example, abnormal shape or colour.</obo:IAO_0000115>
        <terms:title>abnormalMorphologyOfAnatomicalEntity</terms:title>
        <oboInOwl:hasExactSynonym>abnormal morphology of &apos;anatomical entity&apos;</oboInOwl:hasExactSynonym>
        <rdfs:label>abnormal &apos;anatomical entity&apos; morphology</rdfs:label>
    </owl:Class>
    


    <!-- http://purl.obolibrary.org/obo/upheno/patterns-dev/abnormalMorphologyOfAnatomicalEntityInLocation.yaml -->

    <owl:Class rdf:about="http://purl.obolibrary.org/obo/upheno/patterns-dev/abnormalMorphologyOfAnatomicalEntityInLocation.yaml">
        <rdfs:subClassOf rdf:resource="http://purl.obolibrary.org/obo/upheno/patterns-dev/abnormalMorphologyOfAnatomicalEntity.yaml"/>
        <obo:IAO_0000115>A morphological abnormality of the &apos;anatomical entity&apos; in the &apos;independent continuant&apos;.</obo:IAO_0000115>
        <terms:title>abnormalMorphologyOfAnatomicalEntityInLocation</terms:title>
        <oboInOwl:hasExactSynonym>Abnormal morphology of the &apos;anatomical entity&apos; in the &apos;independent continuant&apos;</oboInOwl:hasExactSynonym>
        <rdfs:label>abnormal &apos;anatomical entity&apos; morphology in the &apos;independent continuant&apos;</rdfs:label>
    </owl:Class>
    


    <!-- http://purl.obolibrary.org/obo/upheno/patterns-dev/abnormalMorphologyOfCellularComponent.yaml -->

    <owl:Class rdf:about="http://purl.obolibrary.org/obo/upheno/patterns-dev/abnormalMorphologyOfCellularComponent.yaml">
        <rdfs:subClassOf rdf:resource="http://purl.obolibrary.org/obo/upheno/patterns/abnormalCellularComponent.yaml"/>
        <obo:IAO_0000115>Any structural anomaly of the &apos;cellular component&apos;.</obo:IAO_0000115>
        <terms:title>abnormalMorphologyOfCellularComponent</terms:title>
        <oboInOwl:hasExactSynonym>abnormal shape of &apos;cellular component&apos;</oboInOwl:hasExactSynonym>
        <rdfs:label>abnormal morphology of &apos;cellular component&apos;</rdfs:label>
    </owl:Class>
    


    <!-- http://purl.obolibrary.org/obo/upheno/patterns-dev/abnormalMorphologyOfPartOfAnatomicalEntity.yaml -->

    <owl:Class rdf:about="http://purl.obolibrary.org/obo/upheno/patterns-dev/abnormalMorphologyOfPartOfAnatomicalEntity.yaml">
        <rdfs:subClassOf rdf:resource="http://purl.obolibrary.org/obo/upheno/patterns/abnormalAnatomicalEntity.yaml"/>
        <obo:IAO_0000115>Any unspecified morphological anomaly of part of the &apos;anatomical entity&apos;, such as, for example, abnormal shape or colour.</obo:IAO_0000115>
        <terms:title>abnormalMorphologyOfPartOfAnatomicalEntity</terms:title>
        <oboInOwl:hasExactSynonym>abnormal morphology of &apos;anatomical entity&apos;</oboInOwl:hasExactSynonym>
        <rdfs:label>abnormal &apos;anatomical entity&apos; morphology</rdfs:label>
    </owl:Class>
    


    <!-- http://purl.obolibrary.org/obo/upheno/patterns-dev/abnormalMotilityOfCellularComponent.yaml -->

    <owl:Class rdf:about="http://purl.obolibrary.org/obo/upheno/patterns-dev/abnormalMotilityOfCellularComponent.yaml">
        <obo:IAO_0000115>Abnormal ability to move &apos;cellular component&apos;.</obo:IAO_0000115>
        <terms:title>abnormalMotilityOfCellularComponent</terms:title>
        <rdfs:label>abnormal &apos;cellular component&apos; motility</rdfs:label>
    </owl:Class>
    


    <!-- http://purl.obolibrary.org/obo/upheno/patterns-dev/abnormalNumberOfAnatomicalEntity.yaml -->

    <owl:Class rdf:about="http://purl.obolibrary.org/obo/upheno/patterns-dev/abnormalNumberOfAnatomicalEntity.yaml">
        <rdfs:subClassOf rdf:resource="http://purl.obolibrary.org/obo/upheno/patterns-dev/abnormalAnatomicalEntityNotParts.yaml"/>
        <obo:IAO_0000115>Any structural anomaly that causes there to be an abnormal number &apos;anatomical entity&apos;.</obo:IAO_0000115>
        <terms:title>abnormalNumberOfAnatomicalEntity</terms:title>
        <oboInOwl:hasExactSynonym>abnormal number of &apos;anatomical entity&apos;s</oboInOwl:hasExactSynonym>
        <oboInOwl:hasExactSynonym>altered number of &apos;anatomical entity&apos;s</oboInOwl:hasExactSynonym>
        <rdfs:label>abnormal number of anatomical enitites of type &apos;anatomical entity&apos;</rdfs:label>
    </owl:Class>
    


    <!-- http://purl.obolibrary.org/obo/upheno/patterns-dev/abnormalNumberOfAnatomicalEntityInLocation.yaml -->

    <owl:Class rdf:about="http://purl.obolibrary.org/obo/upheno/patterns-dev/abnormalNumberOfAnatomicalEntityInLocation.yaml">
        <rdfs:subClassOf rdf:resource="http://purl.obolibrary.org/obo/upheno/patterns-dev/abnormalNumberOfAnatomicalEntity.yaml"/>
        <obo:IAO_0000115>Any structural anomaly that causes there to be an abnormal number &apos;anatomical entity&apos; in &apos;independent continuant&apos;.</obo:IAO_0000115>
        <terms:title>abnormalNumberOfAnatomicalEntityInLocation</terms:title>
        <oboInOwl:hasExactSynonym>abnormal number of &apos;anatomical entity&apos;s in &apos;independent continuant&apos;</oboInOwl:hasExactSynonym>
        <oboInOwl:hasExactSynonym>altered number of &apos;anatomical entity&apos;s in &apos;independent continuant&apos;</oboInOwl:hasExactSynonym>
        <rdfs:label>abnormal number of anatomical entities of type &apos;anatomical entity&apos; in &apos;independent continuant&apos;</rdfs:label>
    </owl:Class>
    


    <!-- http://purl.obolibrary.org/obo/upheno/patterns-dev/abnormalNumberOfCellularComponent.yaml -->

    <owl:Class rdf:about="http://purl.obolibrary.org/obo/upheno/patterns-dev/abnormalNumberOfCellularComponent.yaml">
        <rdfs:subClassOf rdf:resource="http://purl.obolibrary.org/obo/upheno/patterns/abnormalCellularComponent.yaml"/>
        <obo:IAO_0000115>Any anomaly that causes there to be an abnormal number &apos;cellular component&apos;.</obo:IAO_0000115>
        <terms:title>abnormalNumberOfCellularComponent</terms:title>
        <oboInOwl:hasExactSynonym>abnormal number of &apos;cellular component&apos;s</oboInOwl:hasExactSynonym>
        <oboInOwl:hasExactSynonym>altered number of &apos;cellular component&apos;s</oboInOwl:hasExactSynonym>
        <rdfs:label>abnormal number of &apos;cellular component&apos;</rdfs:label>
    </owl:Class>
    


    <!-- http://purl.obolibrary.org/obo/upheno/patterns-dev/abnormalPersistenceOfAnatomicalEntity.yaml -->

    <owl:Class rdf:about="http://purl.obolibrary.org/obo/upheno/patterns-dev/abnormalPersistenceOfAnatomicalEntity.yaml">
        <rdfs:subClassOf rdf:resource="http://purl.obolibrary.org/obo/upheno/patterns-dev/abnormalAnatomicalEntityNotParts.yaml"/>
        <obo:IAO_0000115>The abnormal persistence of &apos;anatomical entity&apos;.</obo:IAO_0000115>
        <terms:title>abnormalPersistenceOfAnatomicalEntity</terms:title>
        <rdfs:label>abnormally persistent &apos;anatomical entity&apos;</rdfs:label>
    </owl:Class>
    


    <!-- http://purl.obolibrary.org/obo/upheno/patterns-dev/abnormalPigmentationOfAnatomicalEntity.yaml -->

    <owl:Class rdf:about="http://purl.obolibrary.org/obo/upheno/patterns-dev/abnormalPigmentationOfAnatomicalEntity.yaml">
        <rdfs:subClassOf rdf:resource="http://purl.obolibrary.org/obo/upheno/patterns-dev/abnormalMorphologyOfAnatomicalEntity.yaml"/>
        <obo:IAO_0000115>abnormal degree of pigmentation of the &apos;anatomical entity&apos;.</obo:IAO_0000115>
        <terms:title>abnormalPigmentationOfAnatomicalEntity</terms:title>
        <oboInOwl:hasExactSynonym>abnormal pigmentation of the &apos;anatomical entity&apos;</oboInOwl:hasExactSynonym>
        <rdfs:label>abnormal degree of pigmentation of the &apos;anatomical entity&apos;</rdfs:label>
    </owl:Class>
    


    <!-- http://purl.obolibrary.org/obo/upheno/patterns-dev/abnormalPositionOfAnatomicalEntity.yaml -->

    <owl:Class rdf:about="http://purl.obolibrary.org/obo/upheno/patterns-dev/abnormalPositionOfAnatomicalEntity.yaml">
        <rdfs:subClassOf rdf:resource="http://purl.obolibrary.org/obo/upheno/patterns-dev/abnormalAnatomicalEntityNotParts.yaml"/>
        <obo:IAO_0000115>An abnormal location of &apos;anatomical entity&apos;.</obo:IAO_0000115>
        <terms:title>abnormalPositionOfAnatomicalEntity</terms:title>
        <rdfs:label>abnormal location of &apos;anatomical entity&apos;</rdfs:label>
    </owl:Class>
    


    <!-- http://purl.obolibrary.org/obo/upheno/patterns-dev/abnormalPositionOfAnatomicalEntityInLocation.yaml -->

    <owl:Class rdf:about="http://purl.obolibrary.org/obo/upheno/patterns-dev/abnormalPositionOfAnatomicalEntityInLocation.yaml">
        <rdfs:subClassOf rdf:resource="http://purl.obolibrary.org/obo/upheno/patterns-dev/abnormalPositionOfAnatomicalEntity.yaml"/>
        <obo:IAO_0000115>An abnormal position of the &apos;anatomical entity&apos; in the &apos;independent continuant&apos;.</obo:IAO_0000115>
        <terms:title>abnormalPositionOfAnatomicalEntityInLocation</terms:title>
        <rdfs:label>abnormal &apos;anatomical entity&apos; topology in &apos;independent continuant&apos;</rdfs:label>
    </owl:Class>
    


    <!-- http://purl.obolibrary.org/obo/upheno/patterns-dev/abnormalProportionOfCellTypeInLocation.yaml -->

    <owl:Class rdf:about="http://purl.obolibrary.org/obo/upheno/patterns-dev/abnormalProportionOfCellTypeInLocation.yaml">
        <rdfs:subClassOf rdf:resource="http://purl.obolibrary.org/obo/upheno/patterns-dev/abnormalAnatomicalEntityNotParts.yaml"/>
        <obo:IAO_0000115>A deviation from the normal proportion of &apos;cell&apos; in the &apos;independent continuant&apos;.</obo:IAO_0000115>
        <terms:title>abnormalProportionOfCellTypeInLocation</terms:title>
        <rdfs:label>abnormal proportion of &apos;cell&apos; in &apos;independent continuant&apos;</rdfs:label>
    </owl:Class>
    


    <!-- http://purl.obolibrary.org/obo/upheno/patterns-dev/abnormalProportionOfCellTypeTowardsCellTypeInLocation.yaml -->

    <owl:Class rdf:about="http://purl.obolibrary.org/obo/upheno/patterns-dev/abnormalProportionOfCellTypeTowardsCellTypeInLocation.yaml">
        <rdfs:subClassOf rdf:resource="http://purl.obolibrary.org/obo/upheno/patterns-dev/abnormalAnatomicalEntityNotParts.yaml"/>
        <obo:IAO_0000115>A deviation from the normal proportion of &apos;cell&apos; relative to &apos;cell&apos; in the &apos;independent continuant&apos;.</obo:IAO_0000115>
        <terms:title>abnormalProportionOfCellTypeTowardsCellTypeInLocation</terms:title>
        <rdfs:label>abnormal proportion of &apos;cell&apos; relative to &apos;cell&apos; in &apos;independent continuant&apos;</rdfs:label>
    </owl:Class>
    


    <!-- http://purl.obolibrary.org/obo/upheno/patterns-dev/abnormalRateOfBiologicalProcess.yaml -->

    <owl:Class rdf:about="http://purl.obolibrary.org/obo/upheno/patterns-dev/abnormalRateOfBiologicalProcess.yaml">
        <rdfs:subClassOf rdf:resource="http://purl.obolibrary.org/obo/upheno/patterns-dev/abnormalBiologicalProcess.yaml"/>
        <obo:IAO_0000115>Changed rate of &apos;biological_process&apos;.</obo:IAO_0000115>
        <terms:title>abnormalRateOfBiologicalProcess</terms:title>
        <rdfs:label>changed &apos;biological_process&apos; rate</rdfs:label>
    </owl:Class>
    


    <!-- http://purl.obolibrary.org/obo/upheno/patterns-dev/abnormalRateOfBiologicalProcessBeforeStage.yaml -->

    <owl:Class rdf:about="http://purl.obolibrary.org/obo/upheno/patterns-dev/abnormalRateOfBiologicalProcessBeforeStage.yaml">
        <rdfs:subClassOf rdf:resource="http://purl.obolibrary.org/obo/upheno/patterns-dev/abnormalRateOfBiologicalProcess.yaml"/>
        <obo:IAO_0000115>Abnormal rate of &apos;biological_process&apos; before the &apos;life_cycle_stage&apos;.</obo:IAO_0000115>
        <terms:title>abnormalRateOfBiologicalProcessBeforeStage</terms:title>
        <rdfs:label>abnormal &apos;biological_process&apos; rate before &apos;life_cycle_stage&apos;</rdfs:label>
    </owl:Class>
    


    <!-- http://purl.obolibrary.org/obo/upheno/patterns-dev/abnormalRateOfBiologicalProcessInLocation.yaml -->

    <owl:Class rdf:about="http://purl.obolibrary.org/obo/upheno/patterns-dev/abnormalRateOfBiologicalProcessInLocation.yaml">
        <rdfs:subClassOf rdf:resource="http://purl.obolibrary.org/obo/upheno/patterns-dev/abnormalBiologicalProcessInLocation.yaml"/>
        <rdfs:subClassOf rdf:resource="http://purl.obolibrary.org/obo/upheno/patterns-dev/abnormalRateOfBiologicalProcess.yaml"/>
        <obo:IAO_0000115>Changed rate of &apos;biological_process&apos; in &apos;independent continuant&apos;.</obo:IAO_0000115>
        <terms:title>abnormalRateOfBiologicalProcessInLocation</terms:title>
        <rdfs:label>changed &apos;biological_process&apos; rate in &apos;independent continuant&apos;</rdfs:label>
    </owl:Class>
    


    <!-- http://purl.obolibrary.org/obo/upheno/patterns-dev/abnormalRateOfContinuousBiologicalProcess.yaml -->

    <owl:Class rdf:about="http://purl.obolibrary.org/obo/upheno/patterns-dev/abnormalRateOfContinuousBiologicalProcess.yaml">
        <rdfs:subClassOf rdf:resource="http://purl.obolibrary.org/obo/upheno/patterns-dev/abnormalRateOfBiologicalProcess.yaml"/>
        <obo:IAO_0000115>Abnormal continuous rate of &apos;biological_process&apos;, i.e. &apos;biological_process&apos; has a different amount of output per unit time while it is occurring.</obo:IAO_0000115>
        <terms:title>abnormalRateOfContinuousBiologicalProcess</terms:title>
        <oboInOwl:hasExactSynonym>abnormal &apos;biological_process&apos; velocity</oboInOwl:hasExactSynonym>
        <oboInOwl:hasExactSynonym>abnormal speed of &apos;biological_process&apos;</oboInOwl:hasExactSynonym>
        <oboInOwl:hasExactSynonym>changed continuous rate of &apos;biological_process&apos;</oboInOwl:hasExactSynonym>
        <oboInOwl:hasExactSynonym>changed speed of &apos;biological_process&apos;</oboInOwl:hasExactSynonym>
        <rdfs:label>abnormal continuous rate of &apos;biological_process&apos;</rdfs:label>
    </owl:Class>
    


    <!-- http://purl.obolibrary.org/obo/upheno/patterns-dev/abnormalRateOfDevelopmentDuringStage.yaml -->

    <owl:Class rdf:about="http://purl.obolibrary.org/obo/upheno/patterns-dev/abnormalRateOfDevelopmentDuringStage.yaml">
        <rdfs:subClassOf rdf:resource="http://purl.obolibrary.org/obo/upheno/patterns-dev/abnormalRateOfBiologicalProcess.yaml"/>
        <obo:IAO_0000115>Abnormal rate of &apos;developmental_process&apos; in the &apos;life_cycle_stage&apos;.</obo:IAO_0000115>
        <terms:title>abnormalRateOfDevelopmentDuringStage</terms:title>
        <rdfs:label>abnormal &apos;developmental_process&apos; rate during &apos;life_cycle_stage&apos;</rdfs:label>
    </owl:Class>
    


    <!-- http://purl.obolibrary.org/obo/upheno/patterns-dev/abnormalResistanceOfWholeOrganismToEntity.yaml -->

    <owl:Class rdf:about="http://purl.obolibrary.org/obo/upheno/patterns-dev/abnormalResistanceOfWholeOrganismToEntity.yaml">
        <rdfs:subClassOf rdf:resource="http://purl.obolibrary.org/obo/upheno/patterns-dev/abnormalAnatomicalEntityNotParts.yaml"/>
        <obo:IAO_0000115>abnormally changed resistance of organism to &apos;entity&apos;.</obo:IAO_0000115>
        <terms:title>abnormalResistanceOfWholeOrganismToEntity.yaml</terms:title>
        <oboInOwl:hasExactSynonym>abnormally changed  sensitivity of organism to &apos;entity&apos;</oboInOwl:hasExactSynonym>
        <rdfs:label>abnormally changed resistance of organism to &apos;entity&apos;</rdfs:label>
    </owl:Class>
    


    <!-- http://purl.obolibrary.org/obo/upheno/patterns-dev/abnormalShapeOfAnatomicalEntityByShapeType.yaml -->

    <owl:Class rdf:about="http://purl.obolibrary.org/obo/upheno/patterns-dev/abnormalShapeOfAnatomicalEntityByShapeType.yaml">
        <rdfs:subClassOf rdf:resource="http://purl.obolibrary.org/obo/upheno/patterns-dev/abnormalMorphologyOfAnatomicalEntity.yaml"/>
        <obo:IAO_0000115>Any structural anomaly that causes &apos;anatomical entity&apos; to be &apos;shape&apos; shaped.</obo:IAO_0000115>
        <terms:title>abnormalShapeOfAnatomicalEntityByShapeType</terms:title>
        <oboInOwl:hasExactSynonym>abnormal &apos;shape&apos; shape of &apos;anatomical entity&apos;</oboInOwl:hasExactSynonym>
        <rdfs:label>&apos;shape&apos; &apos;anatomical entity&apos;</rdfs:label>
    </owl:Class>
    


    <!-- http://purl.obolibrary.org/obo/upheno/patterns-dev/abnormalShapeOfAnatomicalEntityByShapeTypeInLocation.yaml -->

    <owl:Class rdf:about="http://purl.obolibrary.org/obo/upheno/patterns-dev/abnormalShapeOfAnatomicalEntityByShapeTypeInLocation.yaml">
        <rdfs:subClassOf rdf:resource="http://purl.obolibrary.org/obo/upheno/patterns-dev/abnormalMorphologyOfAnatomicalEntityInLocation.yaml"/>
        <rdfs:subClassOf rdf:resource="http://purl.obolibrary.org/obo/upheno/patterns-dev/abnormalShapeOfAnatomicalEntityByShapeType.yaml"/>
        <obo:IAO_0000115>Any structural anomaly that causes &apos;anatomical entity&apos; in the &apos;independent continuant&apos; to be &apos;shape&apos; shaped.</obo:IAO_0000115>
        <terms:title>abnormalShapeOfAnatomicalEntityByShapeTypeInLocation</terms:title>
        <oboInOwl:hasExactSynonym>abnormal &apos;shape&apos; shape of &apos;anatomical entity&apos; in &apos;independent continuant&apos;</oboInOwl:hasExactSynonym>
        <rdfs:label>&apos;shape&apos; &apos;anatomical entity&apos; in &apos;independent continuant&apos;</rdfs:label>
    </owl:Class>
    


    <!-- http://purl.obolibrary.org/obo/upheno/patterns-dev/abnormalShapeOfPhysicalEntity.yaml -->

    <owl:Class rdf:about="http://purl.obolibrary.org/obo/upheno/patterns-dev/abnormalShapeOfPhysicalEntity.yaml">
        <obo:IAO_0000115>Any structural anomaly in the shape of the &apos;entity&apos;.</obo:IAO_0000115>
        <terms:title>abnormalShapeOfPhysicalEntity</terms:title>
        <oboInOwl:hasExactSynonym>abnormally shaped &apos;entity&apos;</oboInOwl:hasExactSynonym>
        <rdfs:label>abnormal shape of &apos;entity&apos;</rdfs:label>
    </owl:Class>
    


    <!-- http://purl.obolibrary.org/obo/upheno/patterns-dev/abnormalShapeOfPhysicalEntityInLocation.yaml -->

    <owl:Class rdf:about="http://purl.obolibrary.org/obo/upheno/patterns-dev/abnormalShapeOfPhysicalEntityInLocation.yaml">
        <rdfs:subClassOf rdf:resource="http://purl.obolibrary.org/obo/upheno/patterns-dev/abnormalShapeOfPhysicalEntity.yaml"/>
        <obo:IAO_0000115>Any structural anomaly in the shape of the &apos;entity&apos; located in &apos;independent continuant&apos;.</obo:IAO_0000115>
        <terms:title>abnormalShapeOfPhysicalEntityInLocation</terms:title>
        <oboInOwl:hasExactSynonym>abnormally shaped &apos;entity&apos; in &apos;independent continuant&apos;</oboInOwl:hasExactSynonym>
        <rdfs:label>abnormal shape of &apos;entity&apos; in &apos;independent continuant&apos;</rdfs:label>
    </owl:Class>
    


    <!-- http://purl.obolibrary.org/obo/upheno/patterns-dev/abnormalSizeOfAnatomicalEntity.yaml -->

    <owl:Class rdf:about="http://purl.obolibrary.org/obo/upheno/patterns-dev/abnormalSizeOfAnatomicalEntity.yaml">
        <rdfs:subClassOf rdf:resource="http://purl.obolibrary.org/obo/upheno/patterns-dev/abnormalMorphologyOfAnatomicalEntity.yaml"/>
        <obo:IAO_0000115>A deviation from the normal size of the &apos;anatomical entity&apos;.</obo:IAO_0000115>
        <terms:title>abnormalSizeOfAnatomicalEntity</terms:title>
        <oboInOwl:hasExactSynonym>abnormal size of the &apos;anatomical entity&apos;</oboInOwl:hasExactSynonym>
        <rdfs:label>abnormal size of &apos;anatomical entity&apos;</rdfs:label>
    </owl:Class>
    


    <!-- http://purl.obolibrary.org/obo/upheno/patterns-dev/abnormalSizeOfCellularComponent.yaml -->

    <owl:Class rdf:about="http://purl.obolibrary.org/obo/upheno/patterns-dev/abnormalSizeOfCellularComponent.yaml">
        <rdfs:subClassOf rdf:resource="http://purl.obolibrary.org/obo/upheno/patterns-dev/abnormalMorphologyOfCellularComponent.yaml"/>
        <obo:IAO_0000115>A deviation from the normal size of the &apos;cellular component&apos;.</obo:IAO_0000115>
        <terms:title>abnormalSizeOfCellularComponent</terms:title>
        <oboInOwl:hasExactSynonym>abnormal size of the &apos;cellular component&apos;</oboInOwl:hasExactSynonym>
        <rdfs:label>abnormal size of &apos;cellular component&apos;</rdfs:label>
    </owl:Class>
    


    <!-- http://purl.obolibrary.org/obo/upheno/patterns-dev/abnormalSpatialPatternOfAnatomicalEntity.yaml -->

    <owl:Class rdf:about="http://purl.obolibrary.org/obo/upheno/patterns-dev/abnormalSpatialPatternOfAnatomicalEntity.yaml">
        <rdfs:subClassOf rdf:resource="http://purl.obolibrary.org/obo/upheno/patterns-dev/abnormalMorphologyOfAnatomicalEntity.yaml"/>
        <obo:IAO_0000115>Abnormal spatial pattern of &apos;anatomical entity&apos;.</obo:IAO_0000115>
        <terms:title>abnormalSpatialPatternOfAnatomicalEntity</terms:title>
        <oboInOwl:hasExactSynonym>abnormality of &apos;anatomical entity&apos; spatial pattern</oboInOwl:hasExactSynonym>
        <rdfs:label>abnormal spatial pattern of &apos;anatomical entity&apos;</rdfs:label>
    </owl:Class>
    


    <!-- http://purl.obolibrary.org/obo/upheno/patterns-dev/abnormalStabilityOfAnatomicalEntity.yaml -->

    <owl:Class rdf:about="http://purl.obolibrary.org/obo/upheno/patterns-dev/abnormalStabilityOfAnatomicalEntity.yaml">
        <rdfs:subClassOf rdf:resource="http://purl.obolibrary.org/obo/upheno/patterns-dev/abnormalMorphologyOfAnatomicalEntity.yaml"/>
        <obo:IAO_0000115>Any abnormality in the stability of the &apos;anatomical entity&apos;.</obo:IAO_0000115>
        <terms:title>abnormalStabilityOfAnatomicalEntity</terms:title>
        <rdfs:label>abnormal stability of &apos;anatomical entity&apos;</rdfs:label>
    </owl:Class>
    


    <!-- http://purl.obolibrary.org/obo/upheno/patterns-dev/abnormalThicknessOfAnatomicalEntity.yaml -->

    <owl:Class rdf:about="http://purl.obolibrary.org/obo/upheno/patterns-dev/abnormalThicknessOfAnatomicalEntity.yaml">
        <rdfs:subClassOf rdf:resource="http://purl.obolibrary.org/obo/upheno/patterns-dev/abnormalSizeOfAnatomicalEntity.yaml"/>
        <obo:IAO_0000115>Abnormal thickness of &apos;anatomical_entity&apos; in a dimension that is perpendicular to its length or width.</obo:IAO_0000115>
        <terms:title>abnormalThicknessOfAnatomicalEntity</terms:title>
        <oboInOwl:hasExactSynonym>&apos;anatomical_entity&apos; thickness abnormality</oboInOwl:hasExactSynonym>
        <rdfs:label>abnormal &apos;anatomical_entity&apos; thickness</rdfs:label>
    </owl:Class>
    


    <!-- http://purl.obolibrary.org/obo/upheno/patterns-dev/abnormalWeightOfAnatomicalEntity.yaml -->

    <owl:Class rdf:about="http://purl.obolibrary.org/obo/upheno/patterns-dev/abnormalWeightOfAnatomicalEntity.yaml">
        <rdfs:subClassOf rdf:resource="http://purl.obolibrary.org/obo/upheno/patterns-dev/abnormalAnatomicalEntityNotParts.yaml"/>
        <obo:IAO_0000115>An abnormality of mass in the &apos;anatomical entity&apos;.</obo:IAO_0000115>
        <terms:title>abnormalWeightOfAnatomicalEntity</terms:title>
        <oboInOwl:hasNarrowSynonym>abnormality of &apos;anatomical entity&apos; weight</oboInOwl:hasNarrowSynonym>
        <rdfs:label>abnormality of &apos;anatomical entity&apos; mass</rdfs:label>
    </owl:Class>
    


    <!-- http://purl.obolibrary.org/obo/upheno/patterns-dev/abnormallyApoptoticAnatomicalEntity.yaml -->

    <owl:Class rdf:about="http://purl.obolibrary.org/obo/upheno/patterns-dev/abnormallyApoptoticAnatomicalEntity.yaml">
        <rdfs:subClassOf rdf:resource="http://purl.obolibrary.org/obo/upheno/patterns-dev/abnormalMorphologyOfAnatomicalEntity.yaml"/>
        <obo:IAO_0000115>An abnormally apoptotic &apos;anatomical entity&apos;.</obo:IAO_0000115>
        <terms:title>abnormallyApoptoticAnatomicalEntity</terms:title>
        <oboInOwl:hasExactSynonym>&apos;anatomical entity&apos; with apoptosis</oboInOwl:hasExactSynonym>
        <rdfs:label>abnormally apoptotic &apos;anatomical entity&apos;</rdfs:label>
    </owl:Class>
    


    <!-- http://purl.obolibrary.org/obo/upheno/patterns-dev/abnormallyApoptoticAnatomicalEntityInLocation.yaml -->

    <owl:Class rdf:about="http://purl.obolibrary.org/obo/upheno/patterns-dev/abnormallyApoptoticAnatomicalEntityInLocation.yaml">
        <rdfs:subClassOf rdf:resource="http://purl.obolibrary.org/obo/upheno/patterns-dev/abnormalMorphologyOfAnatomicalEntityInLocation.yaml"/>
        <rdfs:subClassOf rdf:resource="http://purl.obolibrary.org/obo/upheno/patterns-dev/abnormallyApoptoticAnatomicalEntity.yaml"/>
        <obo:IAO_0000115>An abnormally apoptotic &apos;anatomical entity&apos; in &apos;independent continuant&apos;.</obo:IAO_0000115>
        <terms:title>abnormallyApoptoticAnatomicalEntityInLocation</terms:title>
        <oboInOwl:hasExactSynonym>&apos;independent continuant&apos; &apos;anatomical entity&apos; with apoptosis</oboInOwl:hasExactSynonym>
        <rdfs:label>abnormally apoptotic &apos;anatomical entity&apos; in &apos;independent continuant&apos;</rdfs:label>
    </owl:Class>
    


    <!-- http://purl.obolibrary.org/obo/upheno/patterns-dev/abnormallyArchedAnatomicalEntity.yaml -->

    <owl:Class rdf:about="http://purl.obolibrary.org/obo/upheno/patterns-dev/abnormallyArchedAnatomicalEntity.yaml">
        <rdfs:subClassOf rdf:resource="http://purl.obolibrary.org/obo/upheno/patterns-dev/abnormalShapeOfAnatomicalEntityByShapeType.yaml"/>
        <obo:IAO_0000115>An abnormally concave &apos;anatomical_entity&apos; which forms or resembles an arch.</obo:IAO_0000115>
        <terms:title>abnormallyArchedAnatomicalEntity</terms:title>
        <oboInOwl:hasExactSynonym>abnormally arched &apos;anatomical_entity&apos;</oboInOwl:hasExactSynonym>
        <rdfs:label>arched &apos;anatomical_entity&apos;</rdfs:label>
    </owl:Class>
    


    <!-- http://purl.obolibrary.org/obo/upheno/patterns-dev/abnormallyArrestedBiologicalProcess.yaml -->

    <owl:Class rdf:about="http://purl.obolibrary.org/obo/upheno/patterns-dev/abnormallyArrestedBiologicalProcess.yaml">
        <rdfs:subClassOf rdf:resource="http://purl.obolibrary.org/obo/upheno/patterns-dev/abnormallyDecreasedOccurrenceOfBiologicalProcess.yaml"/>
        <obo:IAO_0000115>Arrested &apos;biological_process&apos;.</obo:IAO_0000115>
        <terms:title>abnormallyArrestedBiologicalProcess</terms:title>
        <oboInOwl:hasExactSynonym>&apos;biological_process&apos; arrest</oboInOwl:hasExactSynonym>
        <oboInOwl:hasExactSynonym>failed &apos;biological_process&apos;</oboInOwl:hasExactSynonym>
        <oboInOwl:hasExactSynonym>failure to complete &apos;biological_process&apos;</oboInOwl:hasExactSynonym>
        <oboInOwl:hasExactSynonym>incomplete &apos;biological_process&apos;</oboInOwl:hasExactSynonym>
        <rdfs:label>arrested &apos;biological_process&apos;</rdfs:label>
    </owl:Class>
    


    <!-- http://purl.obolibrary.org/obo/upheno/patterns-dev/abnormallyArrestedBiologicalProcessInLocation.yaml -->

    <owl:Class rdf:about="http://purl.obolibrary.org/obo/upheno/patterns-dev/abnormallyArrestedBiologicalProcessInLocation.yaml">
        <rdfs:subClassOf rdf:resource="http://purl.obolibrary.org/obo/upheno/patterns-dev/abnormallyArrestedBiologicalProcess.yaml"/>
        <rdfs:subClassOf rdf:resource="http://purl.obolibrary.org/obo/upheno/patterns-dev/abnormallyDecreasedOccurrenceOfBiologicalProcessInLocation.yaml"/>
        <obo:IAO_0000115>Arrested &apos;biological_process&apos; in &apos;independent continuant&apos;.</obo:IAO_0000115>
        <terms:title>abnormallyArrestedBiologicalProcessInLocation</terms:title>
        <oboInOwl:hasExactSynonym>&apos;biological_process&apos; arrest in &apos;independent continuant&apos;</oboInOwl:hasExactSynonym>
        <oboInOwl:hasExactSynonym>failed &apos;biological_process&apos; in &apos;independent continuant&apos;</oboInOwl:hasExactSynonym>
        <oboInOwl:hasExactSynonym>failure to complete &apos;biological_process&apos; in &apos;independent continuant&apos;</oboInOwl:hasExactSynonym>
        <oboInOwl:hasExactSynonym>incomplete &apos;biological_process&apos; in &apos;independent continuant&apos;</oboInOwl:hasExactSynonym>
        <rdfs:label>arrested &apos;biological_process&apos; in &apos;independent continuant&apos;</rdfs:label>
    </owl:Class>
    


    <!-- http://purl.obolibrary.org/obo/upheno/patterns-dev/abnormallyAsymmetricalAnatomicalEntity.yaml -->

    <owl:Class rdf:about="http://purl.obolibrary.org/obo/upheno/patterns-dev/abnormallyAsymmetricalAnatomicalEntity.yaml">
        <rdfs:subClassOf rdf:resource="http://purl.obolibrary.org/obo/upheno/patterns-dev/abnormalSpatialPatternOfAnatomicalEntity.yaml"/>
        <obo:IAO_0000115>Abnormal morphological asymmetry of &apos;anatomical_entity&apos; (or a set of thereof) across an axis of symmetry.</obo:IAO_0000115>
        <terms:title>abnormallyAsymmetricalAnatomicalEntity</terms:title>
        <oboInOwl:hasExactSynonym>abnormally asymmetrical &apos;anatomical_entity&apos;</oboInOwl:hasExactSynonym>
        <oboInOwl:hasRelatedSynonym>&apos;anatomical_entity&apos; asymmetry</oboInOwl:hasRelatedSynonym>
        <oboInOwl:hasRelatedSynonym>asymmetry of &apos;anatomical_entity&apos;</oboInOwl:hasRelatedSynonym>
        <rdfs:label>abnormal asymmetry of &apos;anatomical_entity&apos;</rdfs:label>
    </owl:Class>
    


    <!-- http://purl.obolibrary.org/obo/upheno/patterns-dev/abnormallyBentAnatomicalEntity.yaml -->

    <owl:Class rdf:about="http://purl.obolibrary.org/obo/upheno/patterns-dev/abnormallyBentAnatomicalEntity.yaml">
        <rdfs:subClassOf rdf:resource="http://purl.obolibrary.org/obo/upheno/patterns-dev/abnormalShapeOfAnatomicalEntityByShapeType.yaml"/>
        <obo:IAO_0000115>Any abnormal bending of the &apos;anatomical entity&apos;.</obo:IAO_0000115>
        <terms:title>abnormallyBentAnatomicalEntity</terms:title>
        <oboInOwl:hasExactSynonym>abnormally bending &apos;anatomical entity&apos;</oboInOwl:hasExactSynonym>
        <rdfs:label>abnormal bending of &apos;anatomical entity&apos;</rdfs:label>
    </owl:Class>
    


    <!-- http://purl.obolibrary.org/obo/upheno/patterns-dev/abnormallyClosedAnatomicalEntity.yaml -->

    <owl:Class rdf:about="http://purl.obolibrary.org/obo/upheno/patterns-dev/abnormallyClosedAnatomicalEntity.yaml">
        <rdfs:subClassOf rdf:resource="http://purl.obolibrary.org/obo/upheno/patterns-dev/abnormalMorphologyOfAnatomicalEntity.yaml"/>
        <obo:IAO_0000115>Abnormally closed &apos;anatomical entity&apos;.</obo:IAO_0000115>
        <terms:title>abnormallyClosedAnatomicalEntity</terms:title>
        <oboInOwl:hasExactSynonym>abnormally closed &apos;anatomical entity&apos;</oboInOwl:hasExactSynonym>
        <rdfs:label>abnormal closing of the &apos;anatomical entity&apos;</rdfs:label>
    </owl:Class>
    


    <!-- http://purl.obolibrary.org/obo/upheno/patterns-dev/abnormallyCurledAnatomicalEntity.yaml -->

    <owl:Class rdf:about="http://purl.obolibrary.org/obo/upheno/patterns-dev/abnormallyCurledAnatomicalEntity.yaml">
        <rdfs:subClassOf rdf:resource="http://purl.obolibrary.org/obo/upheno/patterns-dev/abnormalShapeOfAnatomicalEntityByShapeType.yaml"/>
        <obo:IAO_0000115>A curled &apos;anatomical_entity&apos; that shows abnormal waves, coils or undulations.</obo:IAO_0000115>
        <terms:title>abnormallyCurledAnatomicalEntity</terms:title>
        <oboInOwl:hasExactSynonym>curled &apos;anatomical_entity&apos;</oboInOwl:hasExactSynonym>
        <oboInOwl:hasExactSynonym>curly &apos;anatomical_entity&apos;</oboInOwl:hasExactSynonym>
        <rdfs:label>abnormally curled &apos;anatomical_entity&apos;</rdfs:label>
    </owl:Class>
    


    <!-- http://purl.obolibrary.org/obo/upheno/patterns-dev/abnormallyCurvedAnatomicalEntityByOrientation.yaml -->

    <owl:Class rdf:about="http://purl.obolibrary.org/obo/upheno/patterns-dev/abnormallyCurvedAnatomicalEntityByOrientation.yaml">
        <rdfs:subClassOf rdf:resource="http://purl.obolibrary.org/obo/upheno/patterns-dev/abnormalShapeOfAnatomicalEntityByShapeType.yaml"/>
        <obo:IAO_0000115>Any abnormal &apos;anatomical entity&apos; that is &apos;curved&apos;ly.</obo:IAO_0000115>
        <terms:title>abnormallyCurvedAnatomicalEntityByOrientation</terms:title>
        <oboInOwl:hasExactSynonym>&apos;curved&apos; &apos;anatomical entity&apos;</oboInOwl:hasExactSynonym>
        <rdfs:label>abnormal &apos;anatomical entity&apos;, &apos;curved&apos;</rdfs:label>
    </owl:Class>
    


    <!-- http://purl.obolibrary.org/obo/upheno/patterns-dev/abnormallyDecreasedCoilingOfAnatomicalEntity.yaml -->

    <owl:Class rdf:about="http://purl.obolibrary.org/obo/upheno/patterns-dev/abnormallyDecreasedCoilingOfAnatomicalEntity.yaml">
        <rdfs:subClassOf rdf:resource="http://purl.obolibrary.org/obo/upheno/patterns-dev/abnormalCoilingOfAnatomicalEntity.yaml"/>
        <obo:IAO_0000115>Abnormally decreased coiling of the &apos;anatomical entity&apos;.</obo:IAO_0000115>
        <terms:title>abnormallyDecreasedCoilingOfAnatomicalEntity</terms:title>
        <oboInOwl:hasExactSynonym>abnormal decreased &apos;anatomical entity&apos; coiling</oboInOwl:hasExactSynonym>
        <rdfs:label>abnormally decreased coiling of &apos;anatomical entity&apos;</rdfs:label>
    </owl:Class>
    


    <!-- http://purl.obolibrary.org/obo/upheno/patterns-dev/abnormallyDecreasedDistanceBetweenAnatomicalEntities.yaml -->

    <owl:Class rdf:about="http://purl.obolibrary.org/obo/upheno/patterns-dev/abnormallyDecreasedDistanceBetweenAnatomicalEntities.yaml">
        <rdfs:subClassOf rdf:resource="http://purl.obolibrary.org/obo/upheno/patterns-dev/abnormalDistanceBetweenAnatomicalEntities.yaml"/>
        <obo:IAO_0000115>Decreased distance between &apos;anatomical entity1&apos; and &apos;anatomical entity2&apos;.</obo:IAO_0000115>
        <terms:title>abnormallyDecreasedDistanceBetweenAnatomicalEntities</terms:title>
        <oboInOwl:hasExactSynonym>distance decreased between &apos;anatomical entity1&apos; and &apos;anatomical entity2&apos;</oboInOwl:hasExactSynonym>
        <rdfs:label>decreased distance between &apos;anatomical entity1&apos; and &apos;anatomical entity2&apos;</rdfs:label>
    </owl:Class>
    


    <!-- http://purl.obolibrary.org/obo/upheno/patterns-dev/abnormallyDecreasedEfficacyOfBehavior.yaml -->

    <owl:Class rdf:about="http://purl.obolibrary.org/obo/upheno/patterns-dev/abnormallyDecreasedEfficacyOfBehavior.yaml">
        <rdfs:subClassOf rdf:resource="http://purl.obolibrary.org/obo/upheno/patterns-dev/abnormalBehavior.yaml"/>
        <obo:IAO_0000115>Decreased ability of &apos;behavior process&apos; to produce its output.</obo:IAO_0000115>
        <terms:title>abnormallyDecreasedEfficacyOfBehavior</terms:title>
        <rdfs:label>abnormally decreased efficacy of &apos;behavior process&apos;</rdfs:label>
    </owl:Class>
    


    <!-- http://purl.obolibrary.org/obo/upheno/patterns-dev/abnormallyDecreasedEfficacyOfProteinLocalizationInCellularComponent.yaml -->

    <owl:Class rdf:about="http://purl.obolibrary.org/obo/upheno/patterns-dev/abnormallyDecreasedEfficacyOfProteinLocalizationInCellularComponent.yaml">
        <rdfs:subClassOf rdf:resource="http://purl.obolibrary.org/obo/upheno/patterns-dev/abnormalEfficacyOfProteinLocalizationInCellularComponent.yaml"/>
        <rdfs:subClassOf rdf:resource="http://purl.obolibrary.org/obo/upheno/patterns-dev/abnormallyDecreasedQualityOfBiologicalProcess.yaml"/>
        <obo:IAO_0000115>Decreased protein localization &apos;cellular component&apos;.</obo:IAO_0000115>
        <terms:title>abnormallyDecreasedEfficacyOfProteinLocalizationInCellularComponent</terms:title>
        <rdfs:label>decreased protein localization in &apos;cellular component&apos;</rdfs:label>
    </owl:Class>
    


    <!-- http://purl.obolibrary.org/obo/upheno/patterns-dev/abnormallyDecreasedFunctionalityOfAnatomicalEntity.yaml -->

    <owl:Class rdf:about="http://purl.obolibrary.org/obo/upheno/patterns-dev/abnormallyDecreasedFunctionalityOfAnatomicalEntity.yaml">
        <rdfs:subClassOf rdf:resource="http://purl.obolibrary.org/obo/upheno/patterns-dev/abnormalFunctionalityOfAnatomicalEntity.yaml"/>
        <obo:IAO_0000115>An abnormally decreased functionality of the &apos;anatomical entity&apos;.</obo:IAO_0000115>
        <terms:title>abnormallyDecreasedFunctionalityOfAnatomicalEntity</terms:title>
        <rdfs:label>abnormally decreased functionality of the &apos;anatomical entity&apos;</rdfs:label>
    </owl:Class>
    


    <!-- http://purl.obolibrary.org/obo/upheno/patterns-dev/abnormallyDecreasedFunctionalityOfAnatomicalEntityInLocation.yaml -->

    <owl:Class rdf:about="http://purl.obolibrary.org/obo/upheno/patterns-dev/abnormallyDecreasedFunctionalityOfAnatomicalEntityInLocation.yaml">
        <rdfs:subClassOf rdf:resource="http://purl.obolibrary.org/obo/upheno/patterns-dev/abnormallyDecreasedFunctionalityOfAnatomicalEntity.yaml"/>
        <obo:IAO_0000115>A functional abnormality of the &apos;anatomical entity&apos; in &apos;independent continuant&apos;.</obo:IAO_0000115>
        <terms:title>abnormallyDecreasedFunctionalityOfAnatomicalEntityInLocation</terms:title>
        <rdfs:label>&apos;anatomical entity&apos; dysfunction in &apos;independent continuant&apos;</rdfs:label>
    </owl:Class>
    


    <!-- http://purl.obolibrary.org/obo/upheno/patterns-dev/abnormallyDecreasedHeightOfAnatomicalEntity.yaml -->

    <owl:Class rdf:about="http://purl.obolibrary.org/obo/upheno/patterns-dev/abnormallyDecreasedHeightOfAnatomicalEntity.yaml">
        <rdfs:subClassOf rdf:resource="http://purl.obolibrary.org/obo/upheno/patterns-dev/abnormalHeightOfAnatomicalEntity.yaml"/>
        <rdfs:subClassOf rdf:resource="http://purl.obolibrary.org/obo/upheno/patterns-dev/abnormallyDecreasedSizeOfAnatomicalEntity.yaml"/>
        <obo:IAO_0000115>A decrease in the height of the &apos;anatomical entity&apos;.</obo:IAO_0000115>
        <terms:title>abnormallyDecreasedHeightOfAnatomicalEntity</terms:title>
        <oboInOwl:hasExactSynonym>shorteer &apos;anatomical entity&apos;</oboInOwl:hasExactSynonym>
        <rdfs:label>decreased height of the &apos;anatomical entity&apos;</rdfs:label>
    </owl:Class>
    


    <!-- http://purl.obolibrary.org/obo/upheno/patterns-dev/abnormallyDecreasedLengthOfAnatomicalEntity.yaml -->

    <owl:Class rdf:about="http://purl.obolibrary.org/obo/upheno/patterns-dev/abnormallyDecreasedLengthOfAnatomicalEntity.yaml">
        <rdfs:subClassOf rdf:resource="http://purl.obolibrary.org/obo/upheno/patterns-dev/abnormalLengthOfAnatomicalEntity.yaml"/>
        <rdfs:subClassOf rdf:resource="http://purl.obolibrary.org/obo/upheno/patterns-dev/abnormallyDecreasedSizeOfAnatomicalEntity.yaml"/>
        <obo:IAO_0000115>Decreased length or shortening of the &apos;anatomical entity&apos;.</obo:IAO_0000115>
        <terms:title>abnormallyDecreasedLengthOfAnatomicalEntity</terms:title>
        <oboInOwl:hasExactSynonym>short &apos;anatomical entity&apos;</oboInOwl:hasExactSynonym>
        <rdfs:label>decreased length of &apos;anatomical entity&apos;</rdfs:label>
    </owl:Class>
    


    <!-- http://purl.obolibrary.org/obo/upheno/patterns-dev/abnormallyDecreasedLengthOfAnatomicalEntityAttachedToLocation.yaml -->

    <owl:Class rdf:about="http://purl.obolibrary.org/obo/upheno/patterns-dev/abnormallyDecreasedLengthOfAnatomicalEntityAttachedToLocation.yaml">
        <rdfs:subClassOf rdf:resource="http://purl.obolibrary.org/obo/upheno/patterns-dev/abnormallyDecreasedLengthOfAnatomicalEntity.yaml"/>
        <obo:IAO_0000115>Decreased length or shortening of the &apos;anatomical entity&apos; attached to the &apos;independent continuant&apos;.</obo:IAO_0000115>
        <terms:title>abnormallyDecreasedLengthOfAnatomicalEntityAttachedToLocation</terms:title>
        <oboInOwl:hasExactSynonym>short &apos;anatomical entity&apos; attached to &apos;independent continuant&apos;</oboInOwl:hasExactSynonym>
        <rdfs:label>decreased length of &apos;anatomical entity&apos; attached to &apos;independent continuant&apos;</rdfs:label>
    </owl:Class>
    


    <!-- http://purl.obolibrary.org/obo/upheno/patterns-dev/abnormallyDecreasedLengthOfAnatomicalEntityInLocation.yaml -->

    <owl:Class rdf:about="http://purl.obolibrary.org/obo/upheno/patterns-dev/abnormallyDecreasedLengthOfAnatomicalEntityInLocation.yaml">
        <rdfs:subClassOf rdf:resource="http://purl.obolibrary.org/obo/upheno/patterns-dev/abnormallyDecreasedLengthOfAnatomicalEntity.yaml"/>
        <rdfs:subClassOf rdf:resource="http://purl.obolibrary.org/obo/upheno/patterns-dev/abnormallyDecreasedSizeOfAnatomicalEntityInLocation.yaml"/>
        <obo:IAO_0000115>Decreased length or shortening of the &apos;anatomical entity&apos; in the &apos;independent continuant&apos;.</obo:IAO_0000115>
        <terms:title>abnormallyDecreasedLengthOfAnatomicalEntityInLocation</terms:title>
        <oboInOwl:hasExactSynonym>short &apos;anatomical entity&apos; in &apos;independent continuant&apos;</oboInOwl:hasExactSynonym>
        <rdfs:label>decreased length of &apos;anatomical entity&apos; in &apos;independent continuant&apos;</rdfs:label>
    </owl:Class>
    


    <!-- http://purl.obolibrary.org/obo/upheno/patterns-dev/abnormallyDecreasedLevelOfChemicalEntity.yaml -->

    <owl:Class rdf:about="http://purl.obolibrary.org/obo/upheno/patterns-dev/abnormallyDecreasedLevelOfChemicalEntity.yaml">
        <rdfs:subClassOf rdf:resource="http://purl.obolibrary.org/obo/upheno/patterns/abnormalLevelOfChemicalEntity.yaml"/>
        <obo:IAO_0000115>A decreased amount in the level of &apos;chemical entity&apos;.</obo:IAO_0000115>
        <terms:title>abnormallyDecreasedLevelOfChemicalEntity</terms:title>
        <rdfs:label>decreased level of &apos;chemical entity&apos;</rdfs:label>
    </owl:Class>
    


    <!-- http://purl.obolibrary.org/obo/upheno/patterns-dev/abnormallyDecreasedLevelOfChemicalEntityInLocation.yaml -->

    <owl:Class rdf:about="http://purl.obolibrary.org/obo/upheno/patterns-dev/abnormallyDecreasedLevelOfChemicalEntityInLocation.yaml">
        <rdfs:subClassOf rdf:resource="http://purl.obolibrary.org/obo/upheno/patterns-dev/abnormallyDecreasedLevelOfChemicalEntity.yaml"/>
        <rdfs:subClassOf rdf:resource="http://purl.obolibrary.org/obo/upheno/patterns/abnormalLevelOfChemicalEntityInLocation.yaml"/>
        <obo:IAO_0000115>A decrease in the level of &apos;chemical entity&apos; in &apos;independent continuant&apos;.</obo:IAO_0000115>
        <terms:title>abnormallyDecreasedLevelOfChemicalEntityInLocation</terms:title>
        <rdfs:label>decreased level of &apos;chemical entity&apos; in &apos;independent continuant&apos;</rdfs:label>
    </owl:Class>
    


    <!-- http://purl.obolibrary.org/obo/upheno/patterns-dev/abnormallyDecreasedLevelOfChemicalEntityWithRole.yaml -->

    <owl:Class rdf:about="http://purl.obolibrary.org/obo/upheno/patterns-dev/abnormallyDecreasedLevelOfChemicalEntityWithRole.yaml">
        <rdfs:subClassOf rdf:resource="http://purl.obolibrary.org/obo/upheno/patterns-dev/abnormalLevelOfChemicalEntityWithRole.yaml"/>
        <rdfs:subClassOf rdf:resource="http://purl.obolibrary.org/obo/upheno/patterns-dev/abnormallyDecreasedLevelOfChemicalEntity.yaml"/>
        <obo:IAO_0000115>An abnormally decreased level of role.</obo:IAO_0000115>
        <terms:title>abnormallyDecreasedLevelOfChemicalEntityWithRole</terms:title>
        <rdfs:label>decreased role level</rdfs:label>
    </owl:Class>
    


    <!-- http://purl.obolibrary.org/obo/upheno/patterns-dev/abnormallyDecreasedLevelOfChemicalEntityWithRoleInLocation.yaml -->

    <owl:Class rdf:about="http://purl.obolibrary.org/obo/upheno/patterns-dev/abnormallyDecreasedLevelOfChemicalEntityWithRoleInLocation.yaml">
        <rdfs:subClassOf rdf:resource="http://purl.obolibrary.org/obo/upheno/patterns-dev/abnormalLevelOfChemicalEntityWithRoleInLocation.yaml"/>
        <rdfs:subClassOf rdf:resource="http://purl.obolibrary.org/obo/upheno/patterns-dev/abnormallyDecreasedLevelOfChemicalEntityInLocation.yaml"/>
        <rdfs:subClassOf rdf:resource="http://purl.obolibrary.org/obo/upheno/patterns-dev/abnormallyDecreasedLevelOfChemicalEntityWithRole.yaml"/>
        <obo:IAO_0000115>An abnormally decreased level of role in the &apos;independent continuant&apos;.</obo:IAO_0000115>
        <terms:title>abnormallyDecreasedLevelOfChemicalEntityWithRoleInLocation</terms:title>
        <rdfs:label>decreased role &apos;independent continuant&apos; level</rdfs:label>
    </owl:Class>
    


    <!-- http://purl.obolibrary.org/obo/upheno/patterns-dev/abnormallyDecreasedMassDensityOfAnatomicalEntity -->

    <owl:Class rdf:about="http://purl.obolibrary.org/obo/upheno/patterns-dev/abnormallyDecreasedMassDensityOfAnatomicalEntity">
        <rdfs:subClassOf rdf:resource="http://purl.obolibrary.org/obo/upheno/patterns-dev/abnormalMassDensityOfAnatomicalEntity.yaml"/>
        <obo:IAO_0000115>Reduced or decreased mass density of &apos;anatomical entity&apos;.</obo:IAO_0000115>
        <terms:title>abnormallyDecreasedMassDensityOfAnatomicalEntity</terms:title>
        <rdfs:label>Decreased &apos;anatomical entity&apos; mass density</rdfs:label>
    </owl:Class>
    


    <!-- http://purl.obolibrary.org/obo/upheno/patterns-dev/abnormallyDecreasedMassOfAnatomicalEntity.yaml -->

    <owl:Class rdf:about="http://purl.obolibrary.org/obo/upheno/patterns-dev/abnormallyDecreasedMassOfAnatomicalEntity.yaml">
        <rdfs:subClassOf rdf:resource="http://purl.obolibrary.org/obo/upheno/patterns-dev/abnormalWeightOfAnatomicalEntity.yaml"/>
        <obo:IAO_0000115>Reduced or decreased mass of &apos;anatomical entity&apos;.</obo:IAO_0000115>
        <terms:title>abnormallyDecreasedMassOfAnatomicalEntity</terms:title>
        <rdfs:label>Decreased &apos;anatomical entity&apos; mass</rdfs:label>
    </owl:Class>
    


    <!-- http://purl.obolibrary.org/obo/upheno/patterns-dev/abnormallyDecreasedMobilityOfAnatomicalEntity.yaml -->

    <owl:Class rdf:about="http://purl.obolibrary.org/obo/upheno/patterns-dev/abnormallyDecreasedMobilityOfAnatomicalEntity.yaml">
        <rdfs:subClassOf rdf:resource="http://purl.obolibrary.org/obo/upheno/patterns-dev/abnormalMobilityOfAnatomicalEntity.yaml"/>
        <obo:IAO_0000115>Decreased or reduced ability to move &apos;anatomical entity&apos;.</obo:IAO_0000115>
        <terms:title>abnormallyDecreasedMobilityOfAnatomicalEntity</terms:title>
        <rdfs:label>decreased &apos;anatomical entity&apos; mobility</rdfs:label>
    </owl:Class>
    


    <!-- http://purl.obolibrary.org/obo/upheno/patterns-dev/abnormallyDecreasedMotilityOfCellularComponentInLocation.yaml -->

    <owl:Class rdf:about="http://purl.obolibrary.org/obo/upheno/patterns-dev/abnormallyDecreasedMotilityOfCellularComponentInLocation.yaml">
        <rdfs:subClassOf rdf:resource="http://purl.obolibrary.org/obo/upheno/patterns-dev/abnormalMotilityOfCellularComponent.yaml"/>
        <obo:IAO_0000115>Decreased ability to move &apos;cellular component&apos; in &apos;independent continuant&apos;.</obo:IAO_0000115>
        <terms:title>abnormallyDecreasedMotilityOfCellularComponentInLocation</terms:title>
        <rdfs:label>decreased &apos;cellular component&apos; motility in &apos;independent continuant&apos;</rdfs:label>
    </owl:Class>
    


    <!-- http://purl.obolibrary.org/obo/upheno/patterns-dev/abnormallyDecreasedNumberOfAnatomicalEntity.yaml -->

    <owl:Class rdf:about="http://purl.obolibrary.org/obo/upheno/patterns-dev/abnormallyDecreasedNumberOfAnatomicalEntity.yaml">
        <rdfs:subClassOf rdf:resource="http://purl.obolibrary.org/obo/upheno/patterns-dev/abnormalNumberOfAnatomicalEntity.yaml"/>
        <obo:IAO_0000115>The presence of a reduced number of &apos;anatomical entity&apos;.</obo:IAO_0000115>
        <terms:title>abnormallyDecreasedNumberOfAnatomicalEntity</terms:title>
        <oboInOwl:hasExactSynonym>Reduced number of &apos;anatomical entity&apos;</oboInOwl:hasExactSynonym>
        <rdfs:label>abnormally decreased number of &apos;anatomical entity&apos;</rdfs:label>
    </owl:Class>
    


    <!-- http://purl.obolibrary.org/obo/upheno/patterns-dev/abnormallyDecreasedNumberOfAnatomicalEntityInLocation.yaml -->

    <owl:Class rdf:about="http://purl.obolibrary.org/obo/upheno/patterns-dev/abnormallyDecreasedNumberOfAnatomicalEntityInLocation.yaml">
        <rdfs:subClassOf rdf:resource="http://purl.obolibrary.org/obo/upheno/patterns-dev/abnormalNumberOfAnatomicalEntityInLocation.yaml"/>
        <rdfs:subClassOf rdf:resource="http://purl.obolibrary.org/obo/upheno/patterns-dev/abnormallyDecreasedNumberOfAnatomicalEntity.yaml"/>
        <obo:IAO_0000115>The presence of a reduced number of &apos;anatomical entity&apos; in the &apos;independent continuant&apos;.</obo:IAO_0000115>
        <terms:title>abnormallyDecreasedNumberOfAnatomicalEntityInLocation</terms:title>
        <oboInOwl:hasExactSynonym>Reduced number of &apos;anatomical entity&apos; in the &apos;independent continuant&apos;</oboInOwl:hasExactSynonym>
        <rdfs:label>abnormally decreased number of &apos;anatomical entity&apos; in the &apos;independent continuant&apos;</rdfs:label>
    </owl:Class>
    


    <!-- http://purl.obolibrary.org/obo/upheno/patterns-dev/abnormallyDecreasedNumberOfCellularComponent.yaml -->

    <owl:Class rdf:about="http://purl.obolibrary.org/obo/upheno/patterns-dev/abnormallyDecreasedNumberOfCellularComponent.yaml">
        <rdfs:subClassOf rdf:resource="http://purl.obolibrary.org/obo/upheno/patterns-dev/abnormalNumberOfCellularComponent.yaml"/>
        <obo:IAO_0000115>The presence of a reduced number of &apos;cellular component&apos;.</obo:IAO_0000115>
        <terms:title>abnormallyDecreasedNumberOfCellularComponent</terms:title>
        <oboInOwl:hasExactSynonym>Reduced number of &apos;cellular component&apos;</oboInOwl:hasExactSynonym>
        <rdfs:label>abnormally decreased number of &apos;cellular component&apos;</rdfs:label>
    </owl:Class>
    


    <!-- http://purl.obolibrary.org/obo/upheno/patterns-dev/abnormallyDecreasedOccurrenceOfBiologicalProcess.yaml -->

    <owl:Class rdf:about="http://purl.obolibrary.org/obo/upheno/patterns-dev/abnormallyDecreasedOccurrenceOfBiologicalProcess.yaml">
        <rdfs:subClassOf rdf:resource="http://purl.obolibrary.org/obo/upheno/patterns-dev/abnormallyDecreasedQualityOfBiologicalProcess.yaml"/>
        <obo:IAO_0000115>A decreased occurrence of &apos;biological_process&apos;.</obo:IAO_0000115>
        <terms:title>abnormallyDecreasedOccurrenceOfBiologicalProcess</terms:title>
        <rdfs:label>decreased occurrence of &apos;biological_process&apos;</rdfs:label>
    </owl:Class>
    


    <!-- http://purl.obolibrary.org/obo/upheno/patterns-dev/abnormallyDecreasedOccurrenceOfBiologicalProcessInLocation.yaml -->

    <owl:Class rdf:about="http://purl.obolibrary.org/obo/upheno/patterns-dev/abnormallyDecreasedOccurrenceOfBiologicalProcessInLocation.yaml">
        <rdfs:subClassOf rdf:resource="http://purl.obolibrary.org/obo/upheno/patterns-dev/abnormallyDecreasedOccurrenceOfBiologicalProcess.yaml"/>
        <rdfs:subClassOf rdf:resource="http://purl.obolibrary.org/obo/upheno/patterns-dev/abnormallyDecreasedQualityOfBiologicalProcessInLocation.yaml"/>
        <obo:IAO_0000115>A decreased occurrence of &apos;biological process&apos; in &apos;independent continuant&apos;.</obo:IAO_0000115>
        <terms:title>abnormallyDecreasedOccurrenceOfBiologicalProcessInLocation</terms:title>
        <rdfs:label>decreased occurrence of &apos;biological process&apos; in &apos;independent continuant&apos;</rdfs:label>
    </owl:Class>
    


    <!-- http://purl.obolibrary.org/obo/upheno/patterns-dev/abnormallyDecreasedPigmentationOfAnatomicalEntity.yaml -->

    <owl:Class rdf:about="http://purl.obolibrary.org/obo/upheno/patterns-dev/abnormallyDecreasedPigmentationOfAnatomicalEntity.yaml">
        <rdfs:subClassOf rdf:resource="http://purl.obolibrary.org/obo/upheno/patterns-dev/abnormalPigmentationOfAnatomicalEntity.yaml"/>
        <obo:IAO_0000115>Decreased or loss of pigmentation of &apos;anatomical entity&apos;.</obo:IAO_0000115>
        <terms:title>abnormallyDecreasedPigmentationOfAnatomicalEntity</terms:title>
        <oboInOwl:hasExactSynonym>&apos;anatomical entity&apos; hypopigmentation</oboInOwl:hasExactSynonym>
        <oboInOwl:hasExactSynonym>loss of pigment in the &apos;anatomical entity&apos;</oboInOwl:hasExactSynonym>
        <rdfs:label>decreased pigmentation in the &apos;anatomical entity&apos;</rdfs:label>
    </owl:Class>
    


    <!-- http://purl.obolibrary.org/obo/upheno/patterns-dev/abnormallyDecreasedPositionOfAnatomicalEntity.yaml -->

    <owl:Class rdf:about="http://purl.obolibrary.org/obo/upheno/patterns-dev/abnormallyDecreasedPositionOfAnatomicalEntity.yaml">
        <rdfs:subClassOf rdf:resource="http://purl.obolibrary.org/obo/upheno/patterns-dev/abnormalPositionOfAnatomicalEntity.yaml"/>
        <obo:IAO_0000115>Lowered position or placement of &apos;anatomical entity&apos;.</obo:IAO_0000115>
        <terms:title>abnormallyDecreasedPositionOfAnatomicalEntity</terms:title>
        <oboInOwl:hasExactSynonym>Lowered &apos;anatomical entity&apos; position</oboInOwl:hasExactSynonym>
        <rdfs:label>Decreased &apos;anatomical entity&apos; position</rdfs:label>
    </owl:Class>
    


    <!-- http://purl.obolibrary.org/obo/upheno/patterns-dev/abnormallyDecreasedQualityOfBiologicalProcess.yaml -->

    <owl:Class rdf:about="http://purl.obolibrary.org/obo/upheno/patterns-dev/abnormallyDecreasedQualityOfBiologicalProcess.yaml">
        <rdfs:subClassOf rdf:resource="http://purl.obolibrary.org/obo/upheno/patterns-dev/abnormalBiologicalProcess.yaml"/>
        <obo:IAO_0000115>Decreased qualitatively &apos;biological process&apos;.</obo:IAO_0000115>
        <terms:title>abnormallyDecreasedQualityOfBiologicalProcess</terms:title>
        <rdfs:label>decreased qualitatively &apos;biological process&apos;</rdfs:label>
    </owl:Class>
    


    <!-- http://purl.obolibrary.org/obo/upheno/patterns-dev/abnormallyDecreasedQualityOfBiologicalProcessInLocation.yaml -->

    <owl:Class rdf:about="http://purl.obolibrary.org/obo/upheno/patterns-dev/abnormallyDecreasedQualityOfBiologicalProcessInLocation.yaml">
        <rdfs:subClassOf rdf:resource="http://purl.obolibrary.org/obo/upheno/patterns-dev/abnormalBiologicalProcessInLocation.yaml"/>
        <rdfs:subClassOf rdf:resource="http://purl.obolibrary.org/obo/upheno/patterns-dev/abnormallyDecreasedQualityOfBiologicalProcess.yaml"/>
        <obo:IAO_0000115>Decreased qualitatively &apos;biological process&apos; in &apos;independent continuant&apos;.</obo:IAO_0000115>
        <terms:title>abnormallyDecreasedQualityOfBiologicalProcessInLocation</terms:title>
        <rdfs:label>decreased qualitatively &apos;biological process&apos; in &apos;independent continuant&apos;</rdfs:label>
    </owl:Class>
    


    <!-- http://purl.obolibrary.org/obo/upheno/patterns-dev/abnormallyDecreasedRateOfBehavior.yaml -->

    <owl:Class rdf:about="http://purl.obolibrary.org/obo/upheno/patterns-dev/abnormallyDecreasedRateOfBehavior.yaml">
        <rdfs:subClassOf rdf:resource="http://purl.obolibrary.org/obo/upheno/patterns-dev/abnormalBehavior.yaml"/>
        <obo:IAO_0000115>Decrease in rate (amount or occurrence per unit of time) of &apos;behavior process&apos;.</obo:IAO_0000115>
        <terms:title>abnormallyDecreasedRateOfBehavior</terms:title>
        <rdfs:label>abnormally decreased rate of &apos;behavior process&apos;</rdfs:label>
    </owl:Class>
    


    <!-- http://purl.obolibrary.org/obo/upheno/patterns-dev/abnormallyDecreasedRateOfBiologicalProcess.yaml -->

    <owl:Class rdf:about="http://purl.obolibrary.org/obo/upheno/patterns-dev/abnormallyDecreasedRateOfBiologicalProcess.yaml">
        <rdfs:subClassOf rdf:resource="http://purl.obolibrary.org/obo/upheno/patterns-dev/abnormalRateOfBiologicalProcess.yaml"/>
        <rdfs:subClassOf rdf:resource="http://purl.obolibrary.org/obo/upheno/patterns-dev/abnormallyDecreasedQualityOfBiologicalProcess.yaml"/>
        <obo:IAO_0000115>decreased &apos;biological_process&apos;.</obo:IAO_0000115>
        <terms:title>abnormallyDecreasedRateOfBiologicalProcess</terms:title>
        <rdfs:label>decreased &apos;biological_process&apos;</rdfs:label>
    </owl:Class>
    


    <!-- http://purl.obolibrary.org/obo/upheno/patterns-dev/abnormallyDecreasedRateOfBiologicalProcessInLocation.yaml -->

    <owl:Class rdf:about="http://purl.obolibrary.org/obo/upheno/patterns-dev/abnormallyDecreasedRateOfBiologicalProcessInLocation.yaml">
        <rdfs:subClassOf rdf:resource="http://purl.obolibrary.org/obo/upheno/patterns-dev/abnormalRateOfBiologicalProcessInLocation.yaml"/>
        <rdfs:subClassOf rdf:resource="http://purl.obolibrary.org/obo/upheno/patterns-dev/abnormallyDecreasedQualityOfBiologicalProcessInLocation.yaml"/>
        <rdfs:subClassOf rdf:resource="http://purl.obolibrary.org/obo/upheno/patterns-dev/abnormallyDecreasedRateOfBiologicalProcess.yaml"/>
        <obo:IAO_0000115>decreased &apos;biological_process&apos; in &apos;independent continuant&apos;.</obo:IAO_0000115>
        <terms:title>abnormallyDecreasedRateOfBiologicalProcessInLocation</terms:title>
        <rdfs:label>decreased &apos;biological_process&apos; in &apos;independent continuant&apos;</rdfs:label>
    </owl:Class>
    


    <!-- http://purl.obolibrary.org/obo/upheno/patterns-dev/abnormallyDecreasedRateOfContinuousBiologicalProcess.yaml -->

    <owl:Class rdf:about="http://purl.obolibrary.org/obo/upheno/patterns-dev/abnormallyDecreasedRateOfContinuousBiologicalProcess.yaml">
        <rdfs:subClassOf rdf:resource="http://purl.obolibrary.org/obo/upheno/patterns-dev/abnormalRateOfContinuousBiologicalProcess.yaml"/>
        <rdfs:subClassOf rdf:resource="http://purl.obolibrary.org/obo/upheno/patterns-dev/abnormallyDecreasedRateOfBiologicalProcess.yaml"/>
        <obo:IAO_0000115>Decreased continuous rate of &apos;biological_process&apos;, i.e. &apos;biological_process&apos; has a reduced amount of output per unit time while it is occurring.</obo:IAO_0000115>
        <terms:title>abnormallyDecreasedRateOfContinuousBiologicalProcess</terms:title>
        <oboInOwl:hasExactSynonym>decreased &apos;biological_process&apos; velocity</oboInOwl:hasExactSynonym>
        <oboInOwl:hasExactSynonym>decreased speed of &apos;biological_process&apos;</oboInOwl:hasExactSynonym>
        <oboInOwl:hasExactSynonym>reduced continuous rate of &apos;biological_process&apos;</oboInOwl:hasExactSynonym>
        <oboInOwl:hasExactSynonym>reduced speed of &apos;biological_process&apos;</oboInOwl:hasExactSynonym>
        <rdfs:label>decreased continuous rate of &apos;biological_process&apos;</rdfs:label>
    </owl:Class>
    


    <!-- http://purl.obolibrary.org/obo/upheno/patterns-dev/abnormallyDecreasedRateOfMolecularFunction.yaml -->

    <owl:Class rdf:about="http://purl.obolibrary.org/obo/upheno/patterns-dev/abnormallyDecreasedRateOfMolecularFunction.yaml">
        <rdfs:subClassOf rdf:resource="http://purl.obolibrary.org/obo/upheno/patterns-dev/abnormalMolecularFunction.yaml"/>
        <obo:IAO_0000115>Abnormally reduced functionality of &apos;molecular function&apos;.</obo:IAO_0000115>
        <terms:title>abnormallyDecreasedRateOfMolecularFunction</terms:title>
        <rdfs:label>decreased &apos;molecular function&apos;</rdfs:label>
    </owl:Class>
    


    <!-- http://purl.obolibrary.org/obo/upheno/patterns-dev/abnormallyDecreasedResistanceOfWholeOrganismToChemicalEntity.yaml -->

    <owl:Class rdf:about="http://purl.obolibrary.org/obo/upheno/patterns-dev/abnormallyDecreasedResistanceOfWholeOrganismToChemicalEntity.yaml">
        <rdfs:subClassOf rdf:resource="http://purl.obolibrary.org/obo/upheno/patterns-dev/abnormalAnatomicalEntityNotParts.yaml"/>
        <obo:IAO_0000115>Decreased resistance of organism to &apos;chemical entity&apos;.</obo:IAO_0000115>
        <terms:title>abnormallyDecreasedResistanceOfWholeOrganismToChemicalEntity.yaml</terms:title>
        <oboInOwl:hasExactSynonym>increased sensitivity of organism to &apos;chemical entity&apos;</oboInOwl:hasExactSynonym>
        <rdfs:label>decreased resistance of organism to &apos;chemical entity&apos;</rdfs:label>
    </owl:Class>
    


    <!-- http://purl.obolibrary.org/obo/upheno/patterns-dev/abnormallyDecreasedResistanceOfWholeOrganismToEntity.yaml -->

    <owl:Class rdf:about="http://purl.obolibrary.org/obo/upheno/patterns-dev/abnormallyDecreasedResistanceOfWholeOrganismToEntity.yaml">
        <rdfs:subClassOf rdf:resource="http://purl.obolibrary.org/obo/upheno/patterns-dev/abnormalResistanceOfWholeOrganismToEntity.yaml"/>
        <obo:IAO_0000115>Decreased resistance of organism to &apos;entity&apos;.</obo:IAO_0000115>
        <terms:title>abnormallyDecreasedResistanceOfWholeOrganismToEntity.yaml</terms:title>
        <oboInOwl:hasExactSynonym>increased sensitivity of organism to &apos;entity&apos;</oboInOwl:hasExactSynonym>
        <rdfs:label>decreased resistance of organism to &apos;entity&apos;</rdfs:label>
    </owl:Class>
    


    <!-- http://purl.obolibrary.org/obo/upheno/patterns-dev/abnormallyDecreasedSizeOfAnatomicalEntity.yaml -->

    <owl:Class rdf:about="http://purl.obolibrary.org/obo/upheno/patterns-dev/abnormallyDecreasedSizeOfAnatomicalEntity.yaml">
        <rdfs:subClassOf rdf:resource="http://purl.obolibrary.org/obo/upheno/patterns-dev/abnormalSizeOfAnatomicalEntity.yaml"/>
        <obo:IAO_0000115>An abnormal reduction in the size of the &apos;anatomical entity&apos;.</obo:IAO_0000115>
        <terms:title>abnormallyDecreasedSizeOfAnatomicalEntity</terms:title>
        <oboInOwl:hasExactSynonym>abnormally small &apos;anatomical entity&apos;</oboInOwl:hasExactSynonym>
        <rdfs:label>decreased size of the &apos;anatomical entity&apos;</rdfs:label>
    </owl:Class>
    


    <!-- http://purl.obolibrary.org/obo/upheno/patterns-dev/abnormallyDecreasedSizeOfAnatomicalEntityInLocation.yaml -->

    <owl:Class rdf:about="http://purl.obolibrary.org/obo/upheno/patterns-dev/abnormallyDecreasedSizeOfAnatomicalEntityInLocation.yaml">
        <rdfs:subClassOf rdf:resource="http://purl.obolibrary.org/obo/upheno/patterns-dev/abnormalMorphologyOfAnatomicalEntityInLocation.yaml"/>
        <rdfs:subClassOf rdf:resource="http://purl.obolibrary.org/obo/upheno/patterns-dev/abnormallyDecreasedSizeOfAnatomicalEntity.yaml"/>
        <obo:IAO_0000115>An abnormal reduction in the size of the &apos;anatomical entity&apos; in the &apos;independent continuant&apos;.</obo:IAO_0000115>
        <terms:title>abnormallyDecreasedSizeOfAnatomicalEntityInLocation</terms:title>
        <oboInOwl:hasExactSynonym>abnormally small &apos;anatomical entity&apos; in &apos;independent continuant&apos;</oboInOwl:hasExactSynonym>
        <rdfs:label>decreased size of the &apos;anatomical entity&apos; in the &apos;independent continuant&apos;</rdfs:label>
    </owl:Class>
    


    <!-- http://purl.obolibrary.org/obo/upheno/patterns-dev/abnormallyDecreasedSizeOfCellularComponent.yaml -->

    <owl:Class rdf:about="http://purl.obolibrary.org/obo/upheno/patterns-dev/abnormallyDecreasedSizeOfCellularComponent.yaml">
        <rdfs:subClassOf rdf:resource="http://purl.obolibrary.org/obo/upheno/patterns-dev/abnormalSizeOfCellularComponent.yaml"/>
        <obo:IAO_0000115>An abnormal reduction in the size of the &apos;cellular component&apos;.</obo:IAO_0000115>
        <terms:title>abnormallyDecreasedSizeOfCellularComponent</terms:title>
        <oboInOwl:hasExactSynonym>abnormally small &apos;cellular component&apos;</oboInOwl:hasExactSynonym>
        <rdfs:label>decreased size of the &apos;cellular component&apos;</rdfs:label>
    </owl:Class>
    


    <!-- http://purl.obolibrary.org/obo/upheno/patterns-dev/abnormallyDecreasedSpeedOfAnatomicalEntity.yaml -->

    <owl:Class rdf:about="http://purl.obolibrary.org/obo/upheno/patterns-dev/abnormallyDecreasedSpeedOfAnatomicalEntity.yaml">
        <rdfs:subClassOf rdf:resource="http://purl.obolibrary.org/obo/upheno/patterns-dev/abnormalAnatomicalEntityNotParts.yaml"/>
        <obo:IAO_0000115>slower, decreased speed of &apos;anatomical entity&apos;</obo:IAO_0000115>
        <terms:title>abnormallyDecreasedSpeedOfAnatomicalEntity</terms:title>
        <oboInOwl:hasExactSynonym>slow moving &apos;anatomical entity&apos;</oboInOwl:hasExactSynonym>
        <rdfs:label>decreased speed of the &apos;anatomical entity&apos;</rdfs:label>
    </owl:Class>
    


    <!-- http://purl.obolibrary.org/obo/upheno/patterns-dev/abnormallyDecreasedStabilityOfAnatomicalEntity.yaml -->

    <owl:Class rdf:about="http://purl.obolibrary.org/obo/upheno/patterns-dev/abnormallyDecreasedStabilityOfAnatomicalEntity.yaml">
        <rdfs:subClassOf rdf:resource="http://purl.obolibrary.org/obo/upheno/patterns-dev/abnormalStabilityOfAnatomicalEntity.yaml"/>
        <obo:IAO_0000115>An abnormally decreased stability of the &apos;anatomical entity&apos;.</obo:IAO_0000115>
        <terms:title>abnormallyDecreasedStabilityOfAnatomicalEntity</terms:title>
        <rdfs:label>abnormally decreased &apos;anatomical entity&apos; stability</rdfs:label>
    </owl:Class>
    


    <!-- http://purl.obolibrary.org/obo/upheno/patterns-dev/abnormallyDecreasedStrengthOfAnatomicalEntity.yaml -->

    <owl:Class rdf:about="http://purl.obolibrary.org/obo/upheno/patterns-dev/abnormallyDecreasedStrengthOfAnatomicalEntity.yaml">
        <rdfs:subClassOf rdf:resource="http://purl.obolibrary.org/obo/upheno/patterns-dev/abnormalAnatomicalEntityNotParts.yaml"/>
        <obo:IAO_0000115>Decreased tonicity of &apos;anatomical entity&apos;.</obo:IAO_0000115>
        <obo:IAO_0000115>Weakness or decreased strength of &apos;anatomical entity&apos;.</obo:IAO_0000115>
        <terms:title>abnormallyDecreasedStrengthOfAnatomicalEntity</terms:title>
        <terms:title>abnormallyDecreasedTonicityOfAnatomicalEntity</terms:title>
        <oboInOwl:hasExactSynonym>&apos;anatomical entity&apos; weakness</oboInOwl:hasExactSynonym>
        <oboInOwl:hasExactSynonym>decreased strength of &apos;anatomical entity&apos;</oboInOwl:hasExactSynonym>
        <rdfs:label>decreased &apos;anatomical entity&apos; strength</rdfs:label>
        <rdfs:label>decreased &apos;anatomical entity&apos; tone</rdfs:label>
    </owl:Class>
    


    <!-- http://purl.obolibrary.org/obo/upheno/patterns-dev/abnormallyDecreasedThicknessOfAnatomicalEntity.yaml -->

    <owl:Class rdf:about="http://purl.obolibrary.org/obo/upheno/patterns-dev/abnormallyDecreasedThicknessOfAnatomicalEntity.yaml">
        <rdfs:subClassOf rdf:resource="http://purl.obolibrary.org/obo/upheno/patterns-dev/abnormalThicknessOfAnatomicalEntity.yaml"/>
        <rdfs:subClassOf rdf:resource="http://purl.obolibrary.org/obo/upheno/patterns-dev/abnormallyDecreasedSizeOfAnatomicalEntity.yaml"/>
        <obo:IAO_0000115>A decrease in the thickness of the &apos;anatomical entity&apos;.</obo:IAO_0000115>
        <terms:title>abnormallyDecreasedThicknessOfAnatomicalEntity</terms:title>
        <oboInOwl:hasExactSynonym>thinned &apos;anatomical entity&apos;</oboInOwl:hasExactSynonym>
        <rdfs:label>decreased thickness of the &apos;anatomical entity&apos;</rdfs:label>
    </owl:Class>
    


    <!-- http://purl.obolibrary.org/obo/upheno/patterns-dev/abnormallyDecreasedVolumeOfAnatomicalEntity.yaml -->

    <owl:Class rdf:about="http://purl.obolibrary.org/obo/upheno/patterns-dev/abnormallyDecreasedVolumeOfAnatomicalEntity.yaml">
        <rdfs:subClassOf rdf:resource="http://purl.obolibrary.org/obo/upheno/patterns-dev/abnormallyDecreasedSizeOfAnatomicalEntity.yaml"/>
        <obo:IAO_0000115>An abnormal reduction in the volume of the &apos;anatomical entity&apos;.</obo:IAO_0000115>
        <terms:title>abnormallyDecreasedVolumeOfAnatomicalEntity</terms:title>
        <rdfs:label>decreased volume of the &apos;anatomical entity&apos;</rdfs:label>
    </owl:Class>
    


    <!-- http://purl.obolibrary.org/obo/upheno/patterns-dev/abnormallyDecreasedWeightOfAnatomicalEntity.yaml -->

    <owl:Class rdf:about="http://purl.obolibrary.org/obo/upheno/patterns-dev/abnormallyDecreasedWeightOfAnatomicalEntity.yaml">
        <rdfs:subClassOf rdf:resource="http://purl.obolibrary.org/obo/upheno/patterns-dev/abnormalWeightOfAnatomicalEntity.yaml"/>
        <obo:IAO_0000115>An abnormal decrease in mass in the &apos;anatomical entity&apos;.</obo:IAO_0000115>
        <terms:title>abnormallyDecreasedWeightOfAnatomicalEntity</terms:title>
        <oboInOwl:hasExactSynonym>low &apos;anatomical entity&apos; mass</oboInOwl:hasExactSynonym>
        <oboInOwl:hasExactSynonym>small &apos;anatomical entity&apos; mass</oboInOwl:hasExactSynonym>
        <oboInOwl:hasNarrowSynonym>decreased &apos;anatomical entity&apos; weight</oboInOwl:hasNarrowSynonym>
        <rdfs:label>decreased &apos;anatomical entity&apos; mass</rdfs:label>
    </owl:Class>
    


    <!-- http://purl.obolibrary.org/obo/upheno/patterns-dev/abnormallyDecreasedWetnessOfAnatomicalEntity.yaml -->

    <owl:Class rdf:about="http://purl.obolibrary.org/obo/upheno/patterns-dev/abnormallyDecreasedWetnessOfAnatomicalEntity.yaml">
        <rdfs:subClassOf rdf:resource="http://purl.obolibrary.org/obo/upheno/patterns-dev/abnormalAnatomicalEntityNotParts.yaml"/>
        <obo:IAO_0000115>A relatively low wetness on the surface of &apos;anatomical_entity&apos;.</obo:IAO_0000115>
        <terms:title>abnormallyDecreasedWetnessOfAnatomicalEntity</terms:title>
        <oboInOwl:hasExactSynonym>decreased &apos;anatomical_entity&apos; surface wetness</oboInOwl:hasExactSynonym>
        <oboInOwl:hasExactSynonym>decreased &apos;anatomical_entity&apos; wetness</oboInOwl:hasExactSynonym>
        <oboInOwl:hasExactSynonym>decreased wetness of &apos;anatomical_entity&apos;</oboInOwl:hasExactSynonym>
        <oboInOwl:hasRelatedSynonym>&apos;anatomical_entity&apos; dryness</oboInOwl:hasRelatedSynonym>
        <oboInOwl:hasRelatedSynonym>dry &apos;anatomical_entity&apos;</oboInOwl:hasRelatedSynonym>
        <rdfs:label>decreased surface wetness of &apos;anatomical_entity&apos;</rdfs:label>
    </owl:Class>
    


    <!-- http://purl.obolibrary.org/obo/upheno/patterns-dev/abnormallyDecreasedWidthOfAnatomicalEntity.yaml -->

    <owl:Class rdf:about="http://purl.obolibrary.org/obo/upheno/patterns-dev/abnormallyDecreasedWidthOfAnatomicalEntity.yaml">
        <rdfs:subClassOf rdf:resource="http://purl.obolibrary.org/obo/upheno/patterns-dev/abnormallyDecreasedSizeOfAnatomicalEntity.yaml"/>
        <obo:IAO_0000115>skinny or decreased width of the &apos;anatomical entity&apos;.</obo:IAO_0000115>
        <terms:title>abnormallyDecreasedWidthOfAnatomicalEntity</terms:title>
        <oboInOwl:hasExactSynonym>skinny &apos;anatomical entity&apos;</oboInOwl:hasExactSynonym>
        <rdfs:label>decreased width of the &apos;anatomical entity&apos;</rdfs:label>
    </owl:Class>
    


    <!-- http://purl.obolibrary.org/obo/upheno/patterns-dev/abnormallyDecreasedWidthOfAnatomicalEntityInLocation.yaml -->

    <owl:Class rdf:about="http://purl.obolibrary.org/obo/upheno/patterns-dev/abnormallyDecreasedWidthOfAnatomicalEntityInLocation.yaml">
        <rdfs:subClassOf rdf:resource="http://purl.obolibrary.org/obo/upheno/patterns-dev/abnormallyDecreasedSizeOfAnatomicalEntityInLocation.yaml"/>
        <rdfs:subClassOf rdf:resource="http://purl.obolibrary.org/obo/upheno/patterns-dev/abnormallyDecreasedWidthOfAnatomicalEntity.yaml"/>
        <obo:IAO_0000115>skinny or decreased width of the &apos;anatomical entity&apos; in &apos;independent continuant&apos;.</obo:IAO_0000115>
        <terms:title>abnormallyDecreasedWidthOfAnatomicalEntityInLocation</terms:title>
        <oboInOwl:hasExactSynonym>skinny &apos;anatomical entity&apos; in &apos;independent continuant&apos;</oboInOwl:hasExactSynonym>
        <rdfs:label>decreased width of the &apos;anatomical entity&apos; in &apos;independent continuant&apos;</rdfs:label>
    </owl:Class>
    


    <!-- http://purl.obolibrary.org/obo/upheno/patterns-dev/abnormallyDelayedBiologicalProcess.yaml -->

    <owl:Class rdf:about="http://purl.obolibrary.org/obo/upheno/patterns-dev/abnormallyDelayedBiologicalProcess.yaml">
        <rdfs:subClassOf rdf:resource="http://purl.obolibrary.org/obo/upheno/patterns-dev/abnormalBiologicalProcess.yaml"/>
        <obo:IAO_0000115>Delayed &apos;biological process&apos;.</obo:IAO_0000115>
        <terms:title>abnormallyDelayedBiologicalProcess</terms:title>
        <rdfs:label>delayed &apos;biological process&apos;</rdfs:label>
    </owl:Class>
    


    <!-- http://purl.obolibrary.org/obo/upheno/patterns-dev/abnormallyDelayedBiologicalProcessInLocation.yaml -->

    <owl:Class rdf:about="http://purl.obolibrary.org/obo/upheno/patterns-dev/abnormallyDelayedBiologicalProcessInLocation.yaml">
        <rdfs:subClassOf rdf:resource="http://purl.obolibrary.org/obo/upheno/patterns-dev/abnormalBiologicalProcessInLocation.yaml"/>
        <rdfs:subClassOf rdf:resource="http://purl.obolibrary.org/obo/upheno/patterns-dev/abnormallyDelayedBiologicalProcess.yaml"/>
        <obo:IAO_0000115>Delayed &apos;biological process&apos; in &apos;independent continuant&apos;.</obo:IAO_0000115>
        <terms:title>abnormallyDelayedBiologicalProcessInLocation</terms:title>
        <rdfs:label>delayed &apos;biological process&apos; in &apos;independent continuant&apos;</rdfs:label>
    </owl:Class>
    


    <!-- http://purl.obolibrary.org/obo/upheno/patterns-dev/abnormallyDetachedAnatomicalEntities.yaml -->

    <owl:Class rdf:about="http://purl.obolibrary.org/obo/upheno/patterns-dev/abnormallyDetachedAnatomicalEntities.yaml">
        <rdfs:subClassOf rdf:resource="http://purl.obolibrary.org/obo/upheno/patterns-dev/abnormalMorphologyOfAnatomicalEntity.yaml"/>
        <obo:IAO_0000115>Detachment of the &apos;anatomical entity&apos; and from the &apos;anatomical entity&apos;.</obo:IAO_0000115>
        <terms:title>abnormallyDetachedAnatomicalEntities</terms:title>
        <rdfs:label>detached &apos;anatomical entity&apos; from &apos;anatomical entity&apos;</rdfs:label>
    </owl:Class>
    


    <!-- http://purl.obolibrary.org/obo/upheno/patterns-dev/abnormallyDilatedAnatomicalEntity.yaml -->

    <owl:Class rdf:about="http://purl.obolibrary.org/obo/upheno/patterns-dev/abnormallyDilatedAnatomicalEntity.yaml">
        <rdfs:subClassOf rdf:resource="http://purl.obolibrary.org/obo/upheno/patterns-dev/abnormallyIncreasedSizeOfAnatomicalEntity.yaml"/>
        <obo:IAO_0000115>Abnormal dilation of &apos;anatomical_entity&apos;.</obo:IAO_0000115>
        <terms:title>abnormallyDilatedAnatomicalEntity</terms:title>
        <oboInOwl:hasExactSynonym>abnormal &apos;anatomical_entity&apos; dilation</oboInOwl:hasExactSynonym>
        <oboInOwl:hasExactSynonym>dilated &apos;anatomical_entity&apos;</oboInOwl:hasExactSynonym>
        <rdfs:label>abnormally dilated &apos;anatomical_entity&apos;</rdfs:label>
    </owl:Class>
    


    <!-- http://purl.obolibrary.org/obo/upheno/patterns-dev/abnormallyDuplicatedAnatomicalEntity.yaml -->

    <owl:Class rdf:about="http://purl.obolibrary.org/obo/upheno/patterns-dev/abnormallyDuplicatedAnatomicalEntity.yaml">
        <rdfs:subClassOf rdf:resource="http://purl.obolibrary.org/obo/upheno/patterns-dev/abnormallyIncreasedNumberOfAnatomicalEntity.yaml"/>
        <obo:IAO_0000115>Any abnormal duplication of the &apos;anatomical entity&apos;.</obo:IAO_0000115>
        <terms:title>abnormallyDuplicatedAnatomicalEntity</terms:title>
        <oboInOwl:hasExactSynonym>abnormal duplication of &apos;anatomical entity&apos;</oboInOwl:hasExactSynonym>
        <oboInOwl:hasExactSynonym>abnormally duplicated &apos;anatomical entity&apos;</oboInOwl:hasExactSynonym>
        <rdfs:label>abnormal duplication of &apos;anatomical entity&apos;</rdfs:label>
    </owl:Class>
    


    <!-- http://purl.obolibrary.org/obo/upheno/patterns-dev/abnormallyDuplicatedAnatomicalEntityInLocation.yaml -->

    <owl:Class rdf:about="http://purl.obolibrary.org/obo/upheno/patterns-dev/abnormallyDuplicatedAnatomicalEntityInLocation.yaml">
        <rdfs:subClassOf rdf:resource="http://purl.obolibrary.org/obo/upheno/patterns-dev/abnormallyDuplicatedAnatomicalEntity.yaml"/>
        <rdfs:subClassOf rdf:resource="http://purl.obolibrary.org/obo/upheno/patterns-dev/abnormallyIncreasedNumberOfAnatomicalEntityInLocation.yaml"/>
        <obo:IAO_0000115>Any abnormal duplication of the &apos;anatomical entity&apos; in &apos;independent continuant&apos;.</obo:IAO_0000115>
        <terms:title>abnormallyDuplicatedAnatomicalEntityInLocation</terms:title>
        <oboInOwl:hasExactSynonym>abnormally duplicated &apos;anatomical entity&apos; in &apos;independent continuant&apos;</oboInOwl:hasExactSynonym>
        <rdfs:label>abnormal duplication of &apos;anatomical entity&apos; in &apos;independent continuant&apos;</rdfs:label>
    </owl:Class>
    


    <!-- http://purl.obolibrary.org/obo/upheno/patterns-dev/abnormallyEvertedAnatomicalEntity.yaml -->

    <owl:Class rdf:about="http://purl.obolibrary.org/obo/upheno/patterns-dev/abnormallyEvertedAnatomicalEntity.yaml">
        <rdfs:subClassOf rdf:resource="http://purl.obolibrary.org/obo/upheno/patterns-dev/abnormalSpatialPatternOfAnatomicalEntity.yaml"/>
        <obo:IAO_0000115>An abnormal configuration of the &apos;anatomical entity&apos; such that it is turned outward i.e., everted,.</obo:IAO_0000115>
        <terms:title>abnormallyEvertedAnatomicalEntity</terms:title>
        <rdfs:label>everted &apos;anatomical entity&apos;</rdfs:label>
    </owl:Class>
    


    <!-- http://purl.obolibrary.org/obo/upheno/patterns-dev/abnormallyFusedAnatomicalEntities.yaml -->

    <owl:Class rdf:about="http://purl.obolibrary.org/obo/upheno/patterns-dev/abnormallyFusedAnatomicalEntities.yaml">
        <rdfs:subClassOf rdf:resource="http://purl.obolibrary.org/obo/upheno/patterns-dev/abnormalMorphologyOfAnatomicalEntity.yaml"/>
        <obo:IAO_0000115>Any abnormal fusion of the &apos;anatomical entity&apos; and the &apos;anatomical entity&apos;.</obo:IAO_0000115>
        <terms:title>abnormallyFusedAnatomicalEntities</terms:title>
        <oboInOwl:hasExactSynonym>abnormal fusion of &apos;anatomical entity&apos; and &apos;anatomical entity&apos;</oboInOwl:hasExactSynonym>
        <rdfs:label>abnormally fused &apos;anatomical entity&apos; and &apos;anatomical entity&apos;</rdfs:label>
    </owl:Class>
    


    <!-- http://purl.obolibrary.org/obo/upheno/patterns-dev/abnormallyFusedAnatomicalEntitiesInLocation.yaml -->

    <owl:Class rdf:about="http://purl.obolibrary.org/obo/upheno/patterns-dev/abnormallyFusedAnatomicalEntitiesInLocation.yaml">
        <rdfs:subClassOf rdf:resource="http://purl.obolibrary.org/obo/upheno/patterns-dev/abnormalMorphologyOfAnatomicalEntityInLocation.yaml"/>
        <rdfs:subClassOf rdf:resource="http://purl.obolibrary.org/obo/upheno/patterns-dev/abnormallyFusedAnatomicalEntities.yaml"/>
        <obo:IAO_0000115>Any abnormal fusion of the &apos;anatomical entity&apos; in the &apos;independent continuant&apos; and the &apos;anatomical entity&apos; in the &apos;independent continuant&apos;.</obo:IAO_0000115>
        <terms:title>abnormallyFusedAnatomicalEntitiesInLocation</terms:title>
        <oboInOwl:hasExactSynonym>abnormal fusion of &apos;anatomical entity&apos; in &apos;independent continuant&apos; and &apos;anatomical entity&apos; in &apos;independent continuant&apos;</oboInOwl:hasExactSynonym>
        <rdfs:label>abnormally fused &apos;anatomical entity&apos; in &apos;independent continuant&apos; with &apos;anatomical entity&apos; in &apos;independent continuant&apos;</rdfs:label>
    </owl:Class>
    


    <!-- http://purl.obolibrary.org/obo/upheno/patterns-dev/abnormallyGlisteningAnatomicalEntity.yaml -->

    <owl:Class rdf:about="http://purl.obolibrary.org/obo/upheno/patterns-dev/abnormallyGlisteningAnatomicalEntity.yaml">
        <rdfs:subClassOf rdf:resource="http://purl.obolibrary.org/obo/upheno/patterns-dev/abnormalAnatomicalEntityNotParts.yaml"/>
        <obo:IAO_0000115>Abnormally shiny, glossy or glistening appearance of &apos;anatomical_entity&apos;.</obo:IAO_0000115>
        <terms:title>abnormallyGlisteningAnatomicalEntity</terms:title>
        <oboInOwl:hasExactSynonym>shiny &apos;anatomical_entity&apos;</oboInOwl:hasExactSynonym>
        <rdfs:label>glistening &apos;anatomical_entity&apos;</rdfs:label>
    </owl:Class>
    


    <!-- http://purl.obolibrary.org/obo/upheno/patterns-dev/abnormallyGreasyAnatomicalEntity.yaml -->

    <owl:Class rdf:about="http://purl.obolibrary.org/obo/upheno/patterns-dev/abnormallyGreasyAnatomicalEntity.yaml">
        <rdfs:subClassOf rdf:resource="http://purl.obolibrary.org/obo/upheno/patterns-dev/abnormalMorphologyOfAnatomicalEntity.yaml"/>
        <obo:IAO_0000115>An abnormal coating of &apos;anatomical_entity&apos; which is oily and slippery.</obo:IAO_0000115>
        <terms:title>abnormallyGreasyAnatomicalEntity</terms:title>
        <oboInOwl:hasExactSynonym>oily &apos;anatomical_entity&apos;</oboInOwl:hasExactSynonym>
        <rdfs:label>greasy &apos;anatomical_entity&apos;</rdfs:label>
    </owl:Class>
    


    <!-- http://purl.obolibrary.org/obo/upheno/patterns-dev/abnormallyImmobileAnatomicalEntity.yaml -->

    <owl:Class rdf:about="http://purl.obolibrary.org/obo/upheno/patterns-dev/abnormallyImmobileAnatomicalEntity.yaml">
        <rdfs:subClassOf rdf:resource="http://purl.obolibrary.org/obo/upheno/patterns-dev/abnormalMobilityOfAnatomicalEntity.yaml"/>
        <obo:IAO_0000115>complete lack of mobility of the &apos;anatomical entity&apos;.</obo:IAO_0000115>
        <terms:title>abnormallyImmobileAnatomicalEntity</terms:title>
        <rdfs:label>abnormally immobile &apos;anatomical entity&apos;</rdfs:label>
    </owl:Class>
    


    <!-- http://purl.obolibrary.org/obo/upheno/patterns-dev/abnormallyIncreasedCoilingOfAnatomicalEntity.yaml -->

    <owl:Class rdf:about="http://purl.obolibrary.org/obo/upheno/patterns-dev/abnormallyIncreasedCoilingOfAnatomicalEntity.yaml">
        <rdfs:subClassOf rdf:resource="http://purl.obolibrary.org/obo/upheno/patterns-dev/abnormalCoilingOfAnatomicalEntity.yaml"/>
        <obo:IAO_0000115>Abnormally increased coiling of the &apos;anatomical entity&apos;.</obo:IAO_0000115>
        <terms:title>abnormallyIncreasedCoilingOfAnatomicalEntity</terms:title>
        <oboInOwl:hasExactSynonym>abnormal increased &apos;anatomical entity&apos; coiling</oboInOwl:hasExactSynonym>
        <rdfs:label>abnormally increased coiling of &apos;anatomical entity&apos;</rdfs:label>
    </owl:Class>
    


    <!-- http://purl.obolibrary.org/obo/upheno/patterns-dev/abnormallyIncreasedDistanceBetweenAnatomicalEntities.yaml -->

    <owl:Class rdf:about="http://purl.obolibrary.org/obo/upheno/patterns-dev/abnormallyIncreasedDistanceBetweenAnatomicalEntities.yaml">
        <rdfs:subClassOf rdf:resource="http://purl.obolibrary.org/obo/upheno/patterns-dev/abnormalDistanceBetweenAnatomicalEntities.yaml"/>
        <obo:IAO_0000115>Increased distance between &apos;entity1&apos; and &apos;entity2&apos;.</obo:IAO_0000115>
        <terms:title>abnormallyIncreasedDistanceBetweenAnatomicalEntities</terms:title>
        <oboInOwl:hasExactSynonym>distance increased between &apos;entity1&apos; and &apos;entity2&apos;</oboInOwl:hasExactSynonym>
        <rdfs:label>increased distance between &apos;entity1&apos; and &apos;entity2&apos;</rdfs:label>
    </owl:Class>
    


    <!-- http://purl.obolibrary.org/obo/upheno/patterns-dev/abnormallyIncreasedEfficacyOfBehavior.yaml -->

    <owl:Class rdf:about="http://purl.obolibrary.org/obo/upheno/patterns-dev/abnormallyIncreasedEfficacyOfBehavior.yaml">
        <rdfs:subClassOf rdf:resource="http://purl.obolibrary.org/obo/upheno/patterns-dev/abnormalBehavior.yaml"/>
        <obo:IAO_0000115>Increased ability of &apos;behavior process&apos; to produce its output.</obo:IAO_0000115>
        <terms:title>abnormallyIncreasedEfficacyOfBehavior</terms:title>
        <rdfs:label>abnormally increased efficacy of &apos;behavior process&apos;</rdfs:label>
    </owl:Class>
    


    <!-- http://purl.obolibrary.org/obo/upheno/patterns-dev/abnormallyIncreasedEfficacyOfProteinLocalizationInCellularComponent.yaml -->

    <owl:Class rdf:about="http://purl.obolibrary.org/obo/upheno/patterns-dev/abnormallyIncreasedEfficacyOfProteinLocalizationInCellularComponent.yaml">
        <rdfs:subClassOf rdf:resource="http://purl.obolibrary.org/obo/upheno/patterns-dev/abnormalEfficacyOfProteinLocalizationInCellularComponent.yaml"/>
        <rdfs:subClassOf rdf:resource="http://purl.obolibrary.org/obo/upheno/patterns-dev/abnormallyIncreasedQualityOfBiologicalProcess.yaml"/>
        <obo:IAO_0000115>Increased protein localization &apos;cellular component&apos;.</obo:IAO_0000115>
        <terms:title>abnormallyIncreasedEfficacyOfProteinLocalizationInCellularComponent</terms:title>
        <rdfs:label>increased protein localization in &apos;cellular component&apos;</rdfs:label>
    </owl:Class>
    


    <!-- http://purl.obolibrary.org/obo/upheno/patterns-dev/abnormallyIncreasedFunctionalityOfAnatomicalEntityInLocation.yaml -->

    <owl:Class rdf:about="http://purl.obolibrary.org/obo/upheno/patterns-dev/abnormallyIncreasedFunctionalityOfAnatomicalEntityInLocation.yaml">
        <rdfs:subClassOf rdf:resource="http://purl.obolibrary.org/obo/upheno/patterns-dev/abnormalFunctionalityOfAnatomicalEntity.yaml"/>
        <obo:IAO_0000115>A hyperactivity of the &apos;anatomical entity&apos; in the &apos;independent continuant&apos;.</obo:IAO_0000115>
        <terms:title>abnormallyIncreasedFunctionalityOfAnatomicalEntityInLocation</terms:title>
        <rdfs:label>&apos;anatomical entity&apos; hyperactivity in &apos;independent continuant&apos;</rdfs:label>
    </owl:Class>
    


    <!-- http://purl.obolibrary.org/obo/upheno/patterns-dev/abnormallyIncreasedHeightOfAnatomicalEntity.yaml -->

    <owl:Class rdf:about="http://purl.obolibrary.org/obo/upheno/patterns-dev/abnormallyIncreasedHeightOfAnatomicalEntity.yaml">
        <rdfs:subClassOf rdf:resource="http://purl.obolibrary.org/obo/upheno/patterns-dev/abnormalHeightOfAnatomicalEntity.yaml"/>
        <rdfs:subClassOf rdf:resource="http://purl.obolibrary.org/obo/upheno/patterns-dev/abnormallyIncreasedSizeOfAnatomicalEntity.yaml"/>
        <obo:IAO_0000115>An increase in the height of the &apos;anatomical entity&apos;.</obo:IAO_0000115>
        <terms:title>abnormallyIncreasedHeightOfAnatomicalEntity</terms:title>
        <oboInOwl:hasExactSynonym>higher &apos;anatomical entity&apos;</oboInOwl:hasExactSynonym>
        <rdfs:label>increased height of the &apos;anatomical entity&apos;</rdfs:label>
    </owl:Class>
    


    <!-- http://purl.obolibrary.org/obo/upheno/patterns-dev/abnormallyIncreasedHeightOfAnatomicalEntityInLocation.yaml -->

    <owl:Class rdf:about="http://purl.obolibrary.org/obo/upheno/patterns-dev/abnormallyIncreasedHeightOfAnatomicalEntityInLocation.yaml">
        <rdfs:subClassOf rdf:resource="http://purl.obolibrary.org/obo/upheno/patterns-dev/abnormallyIncreasedHeightOfAnatomicalEntity.yaml"/>
        <rdfs:subClassOf rdf:resource="http://purl.obolibrary.org/obo/upheno/patterns-dev/abnormallyIncreasedSizeOfAnatomicalEntityInLocation.yaml"/>
        <obo:IAO_0000115>An increase in the height of the &apos;anatomical entity&apos; in the &apos;independent continuant&apos;.</obo:IAO_0000115>
        <terms:title>abnormallyIncreasedHeightOfAnatomicalEntityInLocation</terms:title>
        <oboInOwl:hasExactSynonym>higher &apos;anatomical entity&apos; in &apos;independent continuant&apos;</oboInOwl:hasExactSynonym>
        <rdfs:label>increased height of &apos;anatomical entity&apos; in &apos;independent continuant&apos;</rdfs:label>
    </owl:Class>
    


    <!-- http://purl.obolibrary.org/obo/upheno/patterns-dev/abnormallyIncreasedLengthOfAnatomicalEntity.yaml -->

    <owl:Class rdf:about="http://purl.obolibrary.org/obo/upheno/patterns-dev/abnormallyIncreasedLengthOfAnatomicalEntity.yaml">
        <rdfs:subClassOf rdf:resource="http://purl.obolibrary.org/obo/upheno/patterns-dev/abnormalLengthOfAnatomicalEntity.yaml"/>
        <rdfs:subClassOf rdf:resource="http://purl.obolibrary.org/obo/upheno/patterns-dev/abnormallyIncreasedSizeOfAnatomicalEntity.yaml"/>
        <obo:IAO_0000115>longer, increased length of, &apos;anatomical entity&apos;</obo:IAO_0000115>
        <terms:title>abnormallyIncreasedLengthOfAnatomicalEntity</terms:title>
        <oboInOwl:hasExactSynonym>longer &apos;anatomical entity&apos;</oboInOwl:hasExactSynonym>
        <rdfs:label>increased length of the &apos;anatomical entity&apos;</rdfs:label>
    </owl:Class>
    


    <!-- http://purl.obolibrary.org/obo/upheno/patterns-dev/abnormallyIncreasedLengthOfAnatomicalEntityInLocation.yaml -->

    <owl:Class rdf:about="http://purl.obolibrary.org/obo/upheno/patterns-dev/abnormallyIncreasedLengthOfAnatomicalEntityInLocation.yaml">
        <rdfs:subClassOf rdf:resource="http://purl.obolibrary.org/obo/upheno/patterns-dev/abnormallyIncreasedLengthOfAnatomicalEntity.yaml"/>
        <rdfs:subClassOf rdf:resource="http://purl.obolibrary.org/obo/upheno/patterns-dev/abnormallyIncreasedSizeOfAnatomicalEntityInLocation.yaml"/>
        <obo:IAO_0000115>An abnormal increase in length in &apos;anatomical entity&apos; in location &apos;independent continuant&apos;.</obo:IAO_0000115>
        <terms:title>abnormallyIncreasedLengthOfAnatomicalEntityInLocation</terms:title>
        <rdfs:label>increased &apos;anatomical entity&apos; length in &apos;independent continuant&apos;</rdfs:label>
    </owl:Class>
    


    <!-- http://purl.obolibrary.org/obo/upheno/patterns-dev/abnormallyIncreasedLevelOfChemicalEntity.yaml -->

    <owl:Class rdf:about="http://purl.obolibrary.org/obo/upheno/patterns-dev/abnormallyIncreasedLevelOfChemicalEntity.yaml">
        <rdfs:subClassOf rdf:resource="http://purl.obolibrary.org/obo/upheno/patterns/abnormalLevelOfChemicalEntity.yaml"/>
        <obo:IAO_0000115>An increased amount in the level of &apos;chemical entity&apos;.</obo:IAO_0000115>
        <terms:title>abnormallyIncreasedLevelOfChemicalEntity</terms:title>
        <oboInOwl:hasExactSynonym>increased &apos;chemical entity&apos; level</oboInOwl:hasExactSynonym>
        <rdfs:label>increased level of &apos;chemical entity&apos;</rdfs:label>
    </owl:Class>
    


    <!-- http://purl.obolibrary.org/obo/upheno/patterns-dev/abnormallyIncreasedLevelOfChemicalEntityInLocation.yaml -->

    <owl:Class rdf:about="http://purl.obolibrary.org/obo/upheno/patterns-dev/abnormallyIncreasedLevelOfChemicalEntityInLocation.yaml">
        <rdfs:subClassOf rdf:resource="http://purl.obolibrary.org/obo/upheno/patterns-dev/abnormallyIncreasedLevelOfChemicalEntity.yaml"/>
        <rdfs:subClassOf rdf:resource="http://purl.obolibrary.org/obo/upheno/patterns/abnormalLevelOfChemicalEntityInLocation.yaml"/>
        <obo:IAO_0000115>An increase in the level of &apos;chemical entity&apos; in &apos;independent continuant&apos;.</obo:IAO_0000115>
        <terms:title>abnormallyIncreasedLevelOfChemicalEntityInLocation</terms:title>
        <oboInOwl:hasExactSynonym>increased level of &apos;chemical entity&apos; in &apos;independent continuant&apos;</oboInOwl:hasExactSynonym>
        <rdfs:label>increased level of &apos;chemical entity&apos; in &apos;independent continuant&apos;</rdfs:label>
    </owl:Class>
    


    <!-- http://purl.obolibrary.org/obo/upheno/patterns-dev/abnormallyIncreasedLevelOfChemicalEntityWithRole.yaml -->

    <owl:Class rdf:about="http://purl.obolibrary.org/obo/upheno/patterns-dev/abnormallyIncreasedLevelOfChemicalEntityWithRole.yaml">
        <rdfs:subClassOf rdf:resource="http://purl.obolibrary.org/obo/upheno/patterns-dev/abnormalLevelOfChemicalEntityWithRole.yaml"/>
        <rdfs:subClassOf rdf:resource="http://purl.obolibrary.org/obo/upheno/patterns-dev/abnormallyIncreasedLevelOfChemicalEntity.yaml"/>
        <obo:IAO_0000115>An abnormally increased amount of role.</obo:IAO_0000115>
        <terms:title>abnormallyIncreasedLevelOfChemicalEntityWithRole</terms:title>
        <rdfs:label>increased role level</rdfs:label>
    </owl:Class>
    


    <!-- http://purl.obolibrary.org/obo/upheno/patterns-dev/abnormallyIncreasedLevelOfChemicalEntityWithRoleInLocation.yaml -->

    <owl:Class rdf:about="http://purl.obolibrary.org/obo/upheno/patterns-dev/abnormallyIncreasedLevelOfChemicalEntityWithRoleInLocation.yaml">
        <rdfs:subClassOf rdf:resource="http://purl.obolibrary.org/obo/upheno/patterns-dev/abnormalLevelOfChemicalEntityWithRoleInLocation.yaml"/>
        <rdfs:subClassOf rdf:resource="http://purl.obolibrary.org/obo/upheno/patterns-dev/abnormallyIncreasedLevelOfChemicalEntityInLocation.yaml"/>
        <rdfs:subClassOf rdf:resource="http://purl.obolibrary.org/obo/upheno/patterns-dev/abnormallyIncreasedLevelOfChemicalEntityWithRole.yaml"/>
        <obo:IAO_0000115>An abnormally increased level of role in the &apos;independent continuant&apos;.</obo:IAO_0000115>
        <terms:title>abnormallyIncreasedLevelOfChemicalEntityWithRoleInLocation</terms:title>
        <rdfs:label>increased &apos;independent continuant&apos; role level</rdfs:label>
    </owl:Class>
    


    <!-- http://purl.obolibrary.org/obo/upheno/patterns-dev/abnormallyIncreasedMassDensityOfAnatomicalEntity.yaml -->

    <owl:Class rdf:about="http://purl.obolibrary.org/obo/upheno/patterns-dev/abnormallyIncreasedMassDensityOfAnatomicalEntity.yaml">
        <rdfs:subClassOf rdf:resource="http://purl.obolibrary.org/obo/upheno/patterns-dev/abnormalMassDensityOfAnatomicalEntity.yaml"/>
        <obo:IAO_0000115>Abnormally increased mass density (mass per unit volume) of &apos;anatomical_entity&apos;.</obo:IAO_0000115>
        <terms:title>abnormallyIncreasedMassDensityOfAnatomicalEntity.yaml</terms:title>
        <oboInOwl:hasExactSynonym>abnormally increased mass density of &apos;anatomical_entity&apos;</oboInOwl:hasExactSynonym>
        <rdfs:label>abnormally increased &apos;anatomical_entity&apos; mass density</rdfs:label>
    </owl:Class>
    


    <!-- http://purl.obolibrary.org/obo/upheno/patterns-dev/abnormallyIncreasedMassDensityOfAnatomicalEntityInLocation.yaml -->

    <owl:Class rdf:about="http://purl.obolibrary.org/obo/upheno/patterns-dev/abnormallyIncreasedMassDensityOfAnatomicalEntityInLocation.yaml">
        <rdfs:subClassOf rdf:resource="http://purl.obolibrary.org/obo/upheno/patterns-dev/abnormalMassDensityOfAnatomicalEntityInLocation.yaml"/>
        <rdfs:subClassOf rdf:resource="http://purl.obolibrary.org/obo/upheno/patterns-dev/abnormallyIncreasedMassDensityOfAnatomicalEntity.yaml"/>
        <obo:IAO_0000115>Abnormally increased mass density (mass per unit volume) of &apos;anatomical_entity&apos; of &apos;independent_continuant&apos;.</obo:IAO_0000115>
        <terms:title>abnormallyIncreasedMassDensityOfAnatomicalEntityInLocation</terms:title>
        <oboInOwl:hasExactSynonym>abnormally increased mass density of &apos;anatomical_entity&apos; of &apos;independent_continuant&apos;</oboInOwl:hasExactSynonym>
        <rdfs:label>abnormally increased &apos;anatomical_entity&apos; of &apos;independent_continuant&apos; mass density</rdfs:label>
    </owl:Class>
    


    <!-- http://purl.obolibrary.org/obo/upheno/patterns-dev/abnormallyIncreasedMobilityOfAnatomicalEntity.yaml -->

    <owl:Class rdf:about="http://purl.obolibrary.org/obo/upheno/patterns-dev/abnormallyIncreasedMobilityOfAnatomicalEntity.yaml">
        <rdfs:subClassOf rdf:resource="http://purl.obolibrary.org/obo/upheno/patterns-dev/abnormalMobilityOfAnatomicalEntity.yaml"/>
        <obo:IAO_0000115>Increased or enhanced ability to move &apos;anatomical entity&apos;.</obo:IAO_0000115>
        <terms:title>abnormallyIncreasedMobilityOfAnatomicalEntity</terms:title>
        <rdfs:label>increased &apos;anatomical entity&apos; mobility</rdfs:label>
    </owl:Class>
    


    <!-- http://purl.obolibrary.org/obo/upheno/patterns-dev/abnormallyIncreasedMotilityOfCellularComponentInLocation.yaml -->

    <owl:Class rdf:about="http://purl.obolibrary.org/obo/upheno/patterns-dev/abnormallyIncreasedMotilityOfCellularComponentInLocation.yaml">
        <rdfs:subClassOf rdf:resource="http://purl.obolibrary.org/obo/upheno/patterns-dev/abnormalMotilityOfCellularComponent.yaml"/>
        <obo:IAO_0000115>Increased ability to move &apos;cellular component&apos; in &apos;independent continuant&apos;.</obo:IAO_0000115>
        <terms:title>abnormallyIncreasedMotilityOfCellularComponentInLocation</terms:title>
        <rdfs:label>increased &apos;cellular component&apos; motility in &apos;independent continuant&apos;</rdfs:label>
    </owl:Class>
    


    <!-- http://purl.obolibrary.org/obo/upheno/patterns-dev/abnormallyIncreasedNumberOfAnatomicalEntity.yaml -->

    <owl:Class rdf:about="http://purl.obolibrary.org/obo/upheno/patterns-dev/abnormallyIncreasedNumberOfAnatomicalEntity.yaml">
        <rdfs:subClassOf rdf:resource="http://purl.obolibrary.org/obo/upheno/patterns-dev/abnormalNumberOfAnatomicalEntity.yaml"/>
        <obo:IAO_0000115>The presence of an increased number of &apos;anatomical entity&apos;.</obo:IAO_0000115>
        <terms:title>abnormallyIncreasedNumberOfAnatomicalEntity</terms:title>
        <oboInOwl:hasExactSynonym>Extra &apos;anatomical entity&apos;</oboInOwl:hasExactSynonym>
        <rdfs:label>abnormally increased number of &apos;anatomical entity&apos;</rdfs:label>
    </owl:Class>
    


    <!-- http://purl.obolibrary.org/obo/upheno/patterns-dev/abnormallyIncreasedNumberOfAnatomicalEntityInLocation.yaml -->

    <owl:Class rdf:about="http://purl.obolibrary.org/obo/upheno/patterns-dev/abnormallyIncreasedNumberOfAnatomicalEntityInLocation.yaml">
        <rdfs:subClassOf rdf:resource="http://purl.obolibrary.org/obo/upheno/patterns-dev/abnormalNumberOfAnatomicalEntityInLocation.yaml"/>
        <rdfs:subClassOf rdf:resource="http://purl.obolibrary.org/obo/upheno/patterns-dev/abnormallyIncreasedNumberOfAnatomicalEntity.yaml"/>
        <obo:IAO_0000115>The presence of an increased number of &apos;anatomical entity&apos; in the &apos;independent continuant&apos;.</obo:IAO_0000115>
        <terms:title>abnormallyIncreasedNumberOfAnatomicalEntityInLocation</terms:title>
        <oboInOwl:hasExactSynonym>Extra &apos;anatomical entity&apos; in the &apos;independent continuant&apos;</oboInOwl:hasExactSynonym>
        <rdfs:label>abnormally increased number of &apos;anatomical entity&apos; in the &apos;independent continuant&apos;</rdfs:label>
    </owl:Class>
    


    <!-- http://purl.obolibrary.org/obo/upheno/patterns-dev/abnormallyIncreasedNumberOfCellularComponent.yaml -->

    <owl:Class rdf:about="http://purl.obolibrary.org/obo/upheno/patterns-dev/abnormallyIncreasedNumberOfCellularComponent.yaml">
        <rdfs:subClassOf rdf:resource="http://purl.obolibrary.org/obo/upheno/patterns-dev/abnormalNumberOfCellularComponent.yaml"/>
        <obo:IAO_0000115>The presence of an increased number of &apos;cellular component&apos;.</obo:IAO_0000115>
        <terms:title>abnormallyIncreasedNumberOfCellularComponent</terms:title>
        <oboInOwl:hasExactSynonym>Extra &apos;cellular component&apos;</oboInOwl:hasExactSynonym>
        <rdfs:label>increased number of &apos;cellular component&apos;</rdfs:label>
    </owl:Class>
    


    <!-- http://purl.obolibrary.org/obo/upheno/patterns-dev/abnormallyIncreasedOccurrenceOfBiologicalProcess.yaml -->

    <owl:Class rdf:about="http://purl.obolibrary.org/obo/upheno/patterns-dev/abnormallyIncreasedOccurrenceOfBiologicalProcess.yaml">
        <rdfs:subClassOf rdf:resource="http://purl.obolibrary.org/obo/upheno/patterns-dev/abnormallyIncreasedQualityOfBiologicalProcess.yaml"/>
        <obo:IAO_0000115>An increased occurrence of &apos;biological_process&apos;.</obo:IAO_0000115>
        <terms:title>abnormallyIncreasedOccurrenceOfBiologicalProcess</terms:title>
        <rdfs:label>increased occurrence of &apos;biological_process&apos;</rdfs:label>
    </owl:Class>
    


    <!-- http://purl.obolibrary.org/obo/upheno/patterns-dev/abnormallyIncreasedOccurrenceOfBiologicalProcessInLocation.yaml -->

    <owl:Class rdf:about="http://purl.obolibrary.org/obo/upheno/patterns-dev/abnormallyIncreasedOccurrenceOfBiologicalProcessInLocation.yaml">
        <rdfs:subClassOf rdf:resource="http://purl.obolibrary.org/obo/upheno/patterns-dev/abnormallyIncreasedOccurrenceOfBiologicalProcess.yaml"/>
        <rdfs:subClassOf rdf:resource="http://purl.obolibrary.org/obo/upheno/patterns-dev/abnormallyIncreasedQualityOfBiologicalProcessInLocation.yaml"/>
        <obo:IAO_0000115>An increased occurrence of &apos;biological process&apos; in &apos;independent continuant&apos;.</obo:IAO_0000115>
        <terms:title>abnormallyIncreasedOccurrenceOfBiologicalProcessInLocation</terms:title>
        <rdfs:label>increased occurrence of &apos;biological process&apos; in &apos;independent continuant&apos;</rdfs:label>
    </owl:Class>
    


    <!-- http://purl.obolibrary.org/obo/upheno/patterns-dev/abnormallyIncreasedPigmentationOfAnatomicalEntity.yaml -->

    <owl:Class rdf:about="http://purl.obolibrary.org/obo/upheno/patterns-dev/abnormallyIncreasedPigmentationOfAnatomicalEntity.yaml">
        <rdfs:subClassOf rdf:resource="http://purl.obolibrary.org/obo/upheno/patterns-dev/abnormalPigmentationOfAnatomicalEntity.yaml"/>
        <obo:IAO_0000115>Increased or increasing of pigmentation of &apos;anatomical entity&apos;.</obo:IAO_0000115>
        <terms:title>abnormallyIncreasedPigmentationOfAnatomicalEntity</terms:title>
        <oboInOwl:hasExactSynonym>&apos;anatomical entity&apos; hyperpigmentation</oboInOwl:hasExactSynonym>
        <oboInOwl:hasExactSynonym>increasing of pigment in the &apos;anatomical entity&apos;</oboInOwl:hasExactSynonym>
        <rdfs:label>increased pigmentation in the &apos;anatomical entity&apos;</rdfs:label>
    </owl:Class>
    


    <!-- http://purl.obolibrary.org/obo/upheno/patterns-dev/abnormallyIncreasedQualityOfBiologicalProcess.yaml -->

    <owl:Class rdf:about="http://purl.obolibrary.org/obo/upheno/patterns-dev/abnormallyIncreasedQualityOfBiologicalProcess.yaml">
        <rdfs:subClassOf rdf:resource="http://purl.obolibrary.org/obo/upheno/patterns-dev/abnormalBiologicalProcess.yaml"/>
        <obo:IAO_0000115>Increased qualitatively &apos;biological process&apos;.</obo:IAO_0000115>
        <terms:title>abnormallyIncreasedQualityOfBiologicalProcess</terms:title>
        <rdfs:label>increased qualitatively &apos;biological process&apos;</rdfs:label>
    </owl:Class>
    


    <!-- http://purl.obolibrary.org/obo/upheno/patterns-dev/abnormallyIncreasedQualityOfBiologicalProcessInLocation.yaml -->

    <owl:Class rdf:about="http://purl.obolibrary.org/obo/upheno/patterns-dev/abnormallyIncreasedQualityOfBiologicalProcessInLocation.yaml">
        <rdfs:subClassOf rdf:resource="http://purl.obolibrary.org/obo/upheno/patterns-dev/abnormalBiologicalProcessInLocation.yaml"/>
        <rdfs:subClassOf rdf:resource="http://purl.obolibrary.org/obo/upheno/patterns-dev/abnormallyIncreasedQualityOfBiologicalProcess.yaml"/>
        <obo:IAO_0000115>Increased qualitatively &apos;biological process&apos; in &apos;independent continuant&apos;.</obo:IAO_0000115>
        <terms:title>abnormallyIncreasedQualityOfBiologicalProcessInLocation</terms:title>
        <rdfs:label>increased qualitatively &apos;biological process&apos; in &apos;independent continuant&apos;</rdfs:label>
    </owl:Class>
    


    <!-- http://purl.obolibrary.org/obo/upheno/patterns-dev/abnormallyIncreasedRateOfBehavior.yaml -->

    <owl:Class rdf:about="http://purl.obolibrary.org/obo/upheno/patterns-dev/abnormallyIncreasedRateOfBehavior.yaml">
        <rdfs:subClassOf rdf:resource="http://purl.obolibrary.org/obo/upheno/patterns-dev/abnormalBehavior.yaml"/>
        <obo:IAO_0000115>Increase in rate (amount or occurrence per unit of time) of &apos;behavior process&apos;.</obo:IAO_0000115>
        <terms:title>abnormallyIncreasedRateOfBehavior</terms:title>
        <rdfs:label>abnormally increased rate of &apos;behavior process&apos;</rdfs:label>
    </owl:Class>
    


    <!-- http://purl.obolibrary.org/obo/upheno/patterns-dev/abnormallyIncreasedRateOfBiologicalProcess.yaml -->

    <owl:Class rdf:about="http://purl.obolibrary.org/obo/upheno/patterns-dev/abnormallyIncreasedRateOfBiologicalProcess.yaml">
        <rdfs:subClassOf rdf:resource="http://purl.obolibrary.org/obo/upheno/patterns-dev/abnormalRateOfBiologicalProcess.yaml"/>
        <rdfs:subClassOf rdf:resource="http://purl.obolibrary.org/obo/upheno/patterns-dev/abnormallyIncreasedQualityOfBiologicalProcess.yaml"/>
        <obo:IAO_0000115>Increased &apos;biological_process&apos;.</obo:IAO_0000115>
        <terms:title>abnormallyIncreasedRateOfBiologicalProcess</terms:title>
        <rdfs:label>increased &apos;biological_process&apos;</rdfs:label>
    </owl:Class>
    


    <!-- http://purl.obolibrary.org/obo/upheno/patterns-dev/abnormallyIncreasedRateOfBiologicalProcessInLocation.yaml -->

    <owl:Class rdf:about="http://purl.obolibrary.org/obo/upheno/patterns-dev/abnormallyIncreasedRateOfBiologicalProcessInLocation.yaml">
        <rdfs:subClassOf rdf:resource="http://purl.obolibrary.org/obo/upheno/patterns-dev/abnormalRateOfBiologicalProcessInLocation.yaml"/>
        <rdfs:subClassOf rdf:resource="http://purl.obolibrary.org/obo/upheno/patterns-dev/abnormallyIncreasedQualityOfBiologicalProcessInLocation.yaml"/>
        <rdfs:subClassOf rdf:resource="http://purl.obolibrary.org/obo/upheno/patterns-dev/abnormallyIncreasedRateOfBiologicalProcess.yaml"/>
        <obo:IAO_0000115>Increased &apos;biological process&apos; in &apos;independent continuant&apos;.</obo:IAO_0000115>
        <terms:title>abnormallyIncreasedRateOfBiologicalProcessInLocation</terms:title>
        <rdfs:label>increased &apos;biological process&apos; in &apos;independent continuant&apos;</rdfs:label>
    </owl:Class>
    


    <!-- http://purl.obolibrary.org/obo/upheno/patterns-dev/abnormallyIncreasedRateOfContinuousBiologicalProcess.yaml -->

    <owl:Class rdf:about="http://purl.obolibrary.org/obo/upheno/patterns-dev/abnormallyIncreasedRateOfContinuousBiologicalProcess.yaml">
        <rdfs:subClassOf rdf:resource="http://purl.obolibrary.org/obo/upheno/patterns-dev/abnormalRateOfContinuousBiologicalProcess.yaml"/>
        <rdfs:subClassOf rdf:resource="http://purl.obolibrary.org/obo/upheno/patterns-dev/abnormallyIncreasedRateOfBiologicalProcess.yaml"/>
        <obo:IAO_0000115>Increased continuous rate of &apos;biological_process&apos;, i.e. &apos;biological_process&apos; has an increased amount of output per unit time while it is occurring.</obo:IAO_0000115>
        <terms:title>abnormallyIncreasedRateOfContinuousBiologicalProcess</terms:title>
        <oboInOwl:hasExactSynonym>increased &apos;biological_process&apos; velocity</oboInOwl:hasExactSynonym>
        <oboInOwl:hasExactSynonym>increased speed of &apos;biological_process&apos;</oboInOwl:hasExactSynonym>
        <rdfs:label>increased continuous rate of &apos;biological_process&apos;</rdfs:label>
    </owl:Class>
    


    <!-- http://purl.obolibrary.org/obo/upheno/patterns-dev/abnormallyIncreasedRateOfMolecularFunction.yaml -->

    <owl:Class rdf:about="http://purl.obolibrary.org/obo/upheno/patterns-dev/abnormallyIncreasedRateOfMolecularFunction.yaml">
        <rdfs:subClassOf rdf:resource="http://purl.obolibrary.org/obo/upheno/patterns-dev/abnormalMolecularFunction.yaml"/>
        <obo:IAO_0000115>Increased &apos;molecular function&apos;.</obo:IAO_0000115>
        <terms:title>abnormallyIncreasedRateOfMolecularFunction</terms:title>
        <rdfs:label>increased &apos;molecular function&apos;</rdfs:label>
    </owl:Class>
    


    <!-- http://purl.obolibrary.org/obo/upheno/patterns-dev/abnormallyIncreasedResistanceOfWholeOrganismToChemicalEntity.yaml -->

    <owl:Class rdf:about="http://purl.obolibrary.org/obo/upheno/patterns-dev/abnormallyIncreasedResistanceOfWholeOrganismToChemicalEntity.yaml">
        <rdfs:subClassOf rdf:resource="http://purl.obolibrary.org/obo/upheno/patterns-dev/abnormalAnatomicalEntityNotParts.yaml"/>
        <obo:IAO_0000115>Increased resistance of organism to &apos;chemical entity&apos;.</obo:IAO_0000115>
        <terms:title>abnormallyIncreasedResistanceOfWholeOrganismToChemicalEntity.yaml</terms:title>
        <oboInOwl:hasExactSynonym>decreased sensitivity of organism to &apos;chemical entity&apos;</oboInOwl:hasExactSynonym>
        <rdfs:label>increased resistance of organism to &apos;chemical entity&apos;</rdfs:label>
    </owl:Class>
    


    <!-- http://purl.obolibrary.org/obo/upheno/patterns-dev/abnormallyIncreasedResistanceOfWholeOrganismToEntity.yaml -->

    <owl:Class rdf:about="http://purl.obolibrary.org/obo/upheno/patterns-dev/abnormallyIncreasedResistanceOfWholeOrganismToEntity.yaml">
        <rdfs:subClassOf rdf:resource="http://purl.obolibrary.org/obo/upheno/patterns-dev/abnormalResistanceOfWholeOrganismToEntity.yaml"/>
        <obo:IAO_0000115>Increased resistance of organism to &apos;entity&apos;.</obo:IAO_0000115>
        <terms:title>abnormallyIncreasedResistanceOfWholeOrganismToEntity.yaml</terms:title>
        <oboInOwl:hasExactSynonym>decreased sensitivity of organism to &apos;entity&apos;</oboInOwl:hasExactSynonym>
        <rdfs:label>increased resistance of organism to &apos;entity&apos;</rdfs:label>
    </owl:Class>
    


    <!-- http://purl.obolibrary.org/obo/upheno/patterns-dev/abnormallyIncreasedSizeOfAnatomicalEntity.yaml -->

    <owl:Class rdf:about="http://purl.obolibrary.org/obo/upheno/patterns-dev/abnormallyIncreasedSizeOfAnatomicalEntity.yaml">
        <rdfs:subClassOf rdf:resource="http://purl.obolibrary.org/obo/upheno/patterns-dev/abnormalSizeOfAnatomicalEntity.yaml"/>
        <obo:IAO_0000115>An increase in the size of the &apos;anatomical entity&apos;.</obo:IAO_0000115>
        <terms:title>abnormallyIncreasedSizeOfAnatomicalEntity</terms:title>
        <oboInOwl:hasExactSynonym>enlarged &apos;anatomical entity&apos;</oboInOwl:hasExactSynonym>
        <rdfs:label>increased size of the &apos;anatomical entity&apos;</rdfs:label>
    </owl:Class>
    


    <!-- http://purl.obolibrary.org/obo/upheno/patterns-dev/abnormallyIncreasedSizeOfAnatomicalEntityInLocation.yaml -->

    <owl:Class rdf:about="http://purl.obolibrary.org/obo/upheno/patterns-dev/abnormallyIncreasedSizeOfAnatomicalEntityInLocation.yaml">
        <rdfs:subClassOf rdf:resource="http://purl.obolibrary.org/obo/upheno/patterns-dev/abnormalMorphologyOfAnatomicalEntityInLocation.yaml"/>
        <rdfs:subClassOf rdf:resource="http://purl.obolibrary.org/obo/upheno/patterns-dev/abnormallyIncreasedSizeOfAnatomicalEntity.yaml"/>
        <obo:IAO_0000115>An increase in the size of the &apos;anatomical entity&apos; in the &apos;independent continuant&apos;.</obo:IAO_0000115>
        <terms:title>abnormallyIncreasedSizeOfAnatomicalEntityInLocation</terms:title>
        <oboInOwl:hasExactSynonym>enlarged &apos;anatomical entity&apos; in &apos;independent continuant&apos;</oboInOwl:hasExactSynonym>
        <rdfs:label>increased size of the &apos;anatomical entity&apos; in &apos;independent continuant&apos;</rdfs:label>
    </owl:Class>
    


    <!-- http://purl.obolibrary.org/obo/upheno/patterns-dev/abnormallyIncreasedSizeOfCellularComponent.yaml -->

    <owl:Class rdf:about="http://purl.obolibrary.org/obo/upheno/patterns-dev/abnormallyIncreasedSizeOfCellularComponent.yaml">
        <rdfs:subClassOf rdf:resource="http://purl.obolibrary.org/obo/upheno/patterns-dev/abnormalSizeOfCellularComponent.yaml"/>
        <obo:IAO_0000115>An increase in the size of the &apos;cellular component&apos;.</obo:IAO_0000115>
        <terms:title>abnormallyIncreasedSizeOfCellularComponent</terms:title>
        <oboInOwl:hasExactSynonym>enlarged &apos;cellular component&apos;</oboInOwl:hasExactSynonym>
        <rdfs:label>increased size of the &apos;cellular component&apos;</rdfs:label>
    </owl:Class>
    


    <!-- http://purl.obolibrary.org/obo/upheno/patterns-dev/abnormallyIncreasedSpeedOfAnatomicalEntity.yaml -->

    <owl:Class rdf:about="http://purl.obolibrary.org/obo/upheno/patterns-dev/abnormallyIncreasedSpeedOfAnatomicalEntity.yaml">
        <rdfs:subClassOf rdf:resource="http://purl.obolibrary.org/obo/upheno/patterns-dev/abnormalAnatomicalEntityNotParts.yaml"/>
        <obo:IAO_0000115>faster, increased speed of &apos;anatomical entity&apos;</obo:IAO_0000115>
        <terms:title>abnormallyIncreasedSpeedOfAnatomicalEntity</terms:title>
        <oboInOwl:hasExactSynonym>fast moving &apos;anatomical entity&apos;</oboInOwl:hasExactSynonym>
        <rdfs:label>increased speed of the &apos;anatomical entity&apos;</rdfs:label>
    </owl:Class>
    


    <!-- http://purl.obolibrary.org/obo/upheno/patterns-dev/abnormallyIncreasedStabilityOfAnatomicalEntity.yaml -->

    <owl:Class rdf:about="http://purl.obolibrary.org/obo/upheno/patterns-dev/abnormallyIncreasedStabilityOfAnatomicalEntity.yaml">
        <rdfs:subClassOf rdf:resource="http://purl.obolibrary.org/obo/upheno/patterns-dev/abnormalStabilityOfAnatomicalEntity.yaml"/>
        <obo:IAO_0000115>An abnormally increased stability of the &apos;anatomical entity&apos;.</obo:IAO_0000115>
        <terms:title>abnormallyIncreasedStabilityOfAnatomicalEntity</terms:title>
        <rdfs:label>abnormally increased &apos;anatomical entity&apos; stability</rdfs:label>
    </owl:Class>
    


    <!-- http://purl.obolibrary.org/obo/upheno/patterns-dev/abnormallyIncreasedThicknessOfAnatomicalEntity.yaml -->

    <owl:Class rdf:about="http://purl.obolibrary.org/obo/upheno/patterns-dev/abnormallyIncreasedThicknessOfAnatomicalEntity.yaml">
        <rdfs:subClassOf rdf:resource="http://purl.obolibrary.org/obo/upheno/patterns-dev/abnormalThicknessOfAnatomicalEntity.yaml"/>
        <rdfs:subClassOf rdf:resource="http://purl.obolibrary.org/obo/upheno/patterns-dev/abnormallyIncreasedSizeOfAnatomicalEntity.yaml"/>
        <obo:IAO_0000115>An increase in the thickness of the &apos;anatomical entity&apos;.</obo:IAO_0000115>
        <terms:title>abnormallyIncreasedThicknessOfAnatomicalEntity</terms:title>
        <oboInOwl:hasExactSynonym>thickened &apos;anatomical entity&apos;</oboInOwl:hasExactSynonym>
        <rdfs:label>increased thickness of the &apos;anatomical entity&apos;</rdfs:label>
    </owl:Class>
    


    <!-- http://purl.obolibrary.org/obo/upheno/patterns-dev/abnormallyIncreasedThicknessOfAnatomicalEntityInLocation.yaml -->

    <owl:Class rdf:about="http://purl.obolibrary.org/obo/upheno/patterns-dev/abnormallyIncreasedThicknessOfAnatomicalEntityInLocation.yaml">
        <rdfs:subClassOf rdf:resource="http://purl.obolibrary.org/obo/upheno/patterns-dev/abnormallyIncreasedSizeOfAnatomicalEntityInLocation.yaml"/>
        <rdfs:subClassOf rdf:resource="http://purl.obolibrary.org/obo/upheno/patterns-dev/abnormallyIncreasedThicknessOfAnatomicalEntity.yaml"/>
        <obo:IAO_0000115>An increase in the thickness of the &apos;anatomical entity&apos; in the &apos;independent continuant&apos;.</obo:IAO_0000115>
        <terms:title>abnormallyIncreasedThicknessOfAnatomicalEntityInLocation</terms:title>
        <oboInOwl:hasExactSynonym>thickened &apos;anatomical entity&apos; in &apos;independent continuant&apos;</oboInOwl:hasExactSynonym>
        <rdfs:label>increased thickness of the &apos;anatomical entity&apos; in &apos;independent continuant&apos;</rdfs:label>
    </owl:Class>
    


    <!-- http://purl.obolibrary.org/obo/upheno/patterns-dev/abnormallyIncreasedVolumeOfAnatomicalEntity.yaml -->

    <owl:Class rdf:about="http://purl.obolibrary.org/obo/upheno/patterns-dev/abnormallyIncreasedVolumeOfAnatomicalEntity.yaml">
        <rdfs:subClassOf rdf:resource="http://purl.obolibrary.org/obo/upheno/patterns-dev/abnormallyIncreasedSizeOfAnatomicalEntity.yaml"/>
        <obo:IAO_0000115>An abnormal increase in the volume of &apos;anatomical_entity&apos;.</obo:IAO_0000115>
        <terms:title>abnormallyIncreasedVolumeOfAnatomicalEntity</terms:title>
        <oboInOwl:hasExactSynonym>increased volume of &apos;anatomical_entity&apos;</oboInOwl:hasExactSynonym>
        <rdfs:label>abnormally increased volume of &apos;anatomical_entity&apos;</rdfs:label>
    </owl:Class>
    


    <!-- http://purl.obolibrary.org/obo/upheno/patterns-dev/abnormallyIncreasedWeightOfAnatomicalEntity.yaml -->

    <owl:Class rdf:about="http://purl.obolibrary.org/obo/upheno/patterns-dev/abnormallyIncreasedWeightOfAnatomicalEntity.yaml">
        <rdfs:subClassOf rdf:resource="http://purl.obolibrary.org/obo/upheno/patterns-dev/abnormalWeightOfAnatomicalEntity.yaml"/>
        <obo:IAO_0000115>An abnormal increase in mass in the &apos;anatomical entity&apos;.</obo:IAO_0000115>
        <terms:title>abnormallyIncreasedWeightOfAnatomicalEntity</terms:title>
        <oboInOwl:hasExactSynonym>high &apos;anatomical entity&apos; mass</oboInOwl:hasExactSynonym>
        <oboInOwl:hasExactSynonym>large &apos;anatomical entity&apos; mass</oboInOwl:hasExactSynonym>
        <oboInOwl:hasNarrowSynonym>increased &apos;anatomical entity&apos; weight</oboInOwl:hasNarrowSynonym>
        <rdfs:label>increased &apos;anatomical entity&apos; mass</rdfs:label>
    </owl:Class>
    


    <!-- http://purl.obolibrary.org/obo/upheno/patterns-dev/abnormallyIncreasedWidthOfAnatomicalEntity.yaml -->

    <owl:Class rdf:about="http://purl.obolibrary.org/obo/upheno/patterns-dev/abnormallyIncreasedWidthOfAnatomicalEntity.yaml">
        <rdfs:subClassOf rdf:resource="http://purl.obolibrary.org/obo/upheno/patterns-dev/abnormallyIncreasedSizeOfAnatomicalEntity.yaml"/>
        <obo:IAO_0000115>Increased width of &apos;anatomical entity&apos;.</obo:IAO_0000115>
        <terms:title>abnormallyIncreasedWidthOfAnatomicalEntity</terms:title>
        <oboInOwl:hasExactSynonym>wider &apos;anatomical entity&apos;</oboInOwl:hasExactSynonym>
        <rdfs:label>increased width of &apos;anatomical entity&apos;</rdfs:label>
    </owl:Class>
    


    <!-- http://purl.obolibrary.org/obo/upheno/patterns-dev/abnormallyIncreasedWidthOfAnatomicalEntityInLocation.yaml -->

    <owl:Class rdf:about="http://purl.obolibrary.org/obo/upheno/patterns-dev/abnormallyIncreasedWidthOfAnatomicalEntityInLocation.yaml">
        <rdfs:subClassOf rdf:resource="http://purl.obolibrary.org/obo/upheno/patterns-dev/abnormallyIncreasedSizeOfAnatomicalEntityInLocation.yaml"/>
        <rdfs:subClassOf rdf:resource="http://purl.obolibrary.org/obo/upheno/patterns-dev/abnormallyIncreasedWidthOfAnatomicalEntity.yaml"/>
        <obo:IAO_0000115>Wide or increased width of the &apos;anatomical entity&apos; in &apos;independent continuant&apos;.</obo:IAO_0000115>
        <terms:title>abnormallyIncreasedWidthOfAnatomicalEntityInLocation</terms:title>
        <oboInOwl:hasExactSynonym>wide &apos;anatomical entity&apos; in &apos;independent continuant&apos;</oboInOwl:hasExactSynonym>
        <rdfs:label>increased width of the &apos;anatomical entity&apos; in &apos;independent continuant&apos;</rdfs:label>
    </owl:Class>
    


    <!-- http://purl.obolibrary.org/obo/upheno/patterns-dev/abnormallyInvertedAnatomicalEntityInLocation.yaml -->

    <owl:Class rdf:about="http://purl.obolibrary.org/obo/upheno/patterns-dev/abnormallyInvertedAnatomicalEntityInLocation.yaml">
        <rdfs:subClassOf rdf:resource="http://purl.obolibrary.org/obo/upheno/patterns-dev/abnormalMorphologyOfAnatomicalEntityInLocation.yaml"/>
        <rdfs:subClassOf rdf:resource="http://purl.obolibrary.org/obo/upheno/patterns-dev/abnormalSpatialPatternOfAnatomicalEntity.yaml"/>
        <obo:IAO_0000115>An abnormal configuration of the &apos;anatomical entity&apos; such that it is reversed in position, order, or condition in in &apos;independent continuant&apos;.</obo:IAO_0000115>
        <terms:title>abnormallyInvertedAnatomicalEntityInLocation</terms:title>
        <oboInOwl:hasExactSynonym>reversed &apos;anatomical entity&apos; in &apos;independent continuant&apos;</oboInOwl:hasExactSynonym>
        <rdfs:label>inverted &apos;anatomical entity&apos; in &apos;independent continuant&apos;</rdfs:label>
    </owl:Class>
    


    <!-- http://purl.obolibrary.org/obo/upheno/patterns-dev/abnormallyIvoryAnatomicalEntityInLocation.yaml -->

    <owl:Class rdf:about="http://purl.obolibrary.org/obo/upheno/patterns-dev/abnormallyIvoryAnatomicalEntityInLocation.yaml">
        <rdfs:subClassOf rdf:resource="http://purl.obolibrary.org/obo/upheno/patterns-dev/abnormallyIncreasedMassDensityOfAnatomicalEntityInLocation.yaml"/>
        <rdfs:subClassOf rdf:resource="http://purl.obolibrary.org/obo/upheno/patterns-dev/ivoryAnatomicalEntity.yaml"/>
        <obo:IAO_0000115>An abnormal increase in the density of &apos;anatomical_entity&apos; of &apos;independent_continuant&apos; resulting in increased degree of radiopacity (in X-rays).</obo:IAO_0000115>
        <terms:title>abnormallyIvoryAnatomicalEntityInLocation</terms:title>
        <oboInOwl:hasExactSynonym>abnormal radiographic density of &apos;anatomical_entity&apos; of &apos;independent_continuant&apos;</oboInOwl:hasExactSynonym>
        <rdfs:label>ivory &apos;anatomical_entity&apos; or &apos;independent_continuant&apos;</rdfs:label>
    </owl:Class>
    


    <!-- http://purl.obolibrary.org/obo/upheno/patterns-dev/abnormallyOpaqueAnatomicalEntity.yaml -->

    <owl:Class rdf:about="http://purl.obolibrary.org/obo/upheno/patterns-dev/abnormallyOpaqueAnatomicalEntity.yaml">
        <rdfs:subClassOf rdf:resource="http://purl.obolibrary.org/obo/upheno/patterns-dev/abnormalAnatomicalEntityNotParts.yaml"/>
        <obo:IAO_0000115>Impaired ability or inability of light to pass through &apos;anatomical_entity&apos;.</obo:IAO_0000115>
        <terms:title>abnormallyOpaqueAnatomicalEntity</terms:title>
        <oboInOwl:hasExactSynonym>cloudy &apos;anatomical_entity&apos;</oboInOwl:hasExactSynonym>
        <oboInOwl:hasExactSynonym>opacity of &apos;anatomical_entity&apos;</oboInOwl:hasExactSynonym>
        <rdfs:label>opaque &apos;anatomical_entity&apos;</rdfs:label>
    </owl:Class>
    


    <!-- http://purl.obolibrary.org/obo/upheno/patterns-dev/abnormallyOpenAnatomicalEntity.yaml -->

    <owl:Class rdf:about="http://purl.obolibrary.org/obo/upheno/patterns-dev/abnormallyOpenAnatomicalEntity.yaml">
        <rdfs:subClassOf rdf:resource="http://purl.obolibrary.org/obo/upheno/patterns-dev/abnormalMorphologyOfAnatomicalEntity.yaml"/>
        <obo:IAO_0000115>Abnormally open &apos;anatomical entity&apos;.</obo:IAO_0000115>
        <terms:title>abnormallyOpenAnatomicalEntity</terms:title>
        <oboInOwl:hasExactSynonym>abnormally open &apos;anatomical entity&apos;</oboInOwl:hasExactSynonym>
        <rdfs:label>abnormal opening of the &apos;anatomical entity&apos;</rdfs:label>
    </owl:Class>
    


    <!-- http://purl.obolibrary.org/obo/upheno/patterns-dev/abnormallyPatchyPigmentationOfAnatomicalEntity.yaml -->

    <owl:Class rdf:about="http://purl.obolibrary.org/obo/upheno/patterns-dev/abnormallyPatchyPigmentationOfAnatomicalEntity.yaml">
        <rdfs:subClassOf rdf:resource="http://purl.obolibrary.org/obo/upheno/patterns-dev/abnormalPigmentationOfAnatomicalEntity.yaml"/>
        <obo:IAO_0000115>&apos;anatomical entity&apos; with a degree of pigmentation quality that is diversified with patches, or irregularity.</obo:IAO_0000115>
        <terms:title>abnormallyPatchyPigmentationOfAnatomicalEntity</terms:title>
        <oboInOwl:hasExactSynonym>irregular pigment in the &apos;anatomical entity&apos;</oboInOwl:hasExactSynonym>
        <rdfs:label>patchy pigmentation in the &apos;anatomical entity&apos;</rdfs:label>
    </owl:Class>
    


    <!-- http://purl.obolibrary.org/obo/upheno/patterns-dev/abnormallyPrematureBiologicalProcess.yaml -->

    <owl:Class rdf:about="http://purl.obolibrary.org/obo/upheno/patterns-dev/abnormallyPrematureBiologicalProcess.yaml">
        <rdfs:subClassOf rdf:resource="http://purl.obolibrary.org/obo/upheno/patterns-dev/abnormalBiologicalProcess.yaml"/>
        <obo:IAO_0000115>An abnormally early start time of &apos;biological process&apos;.</obo:IAO_0000115>
        <terms:title>abnormallyPrematureBiologicalProcess</terms:title>
        <rdfs:label>premature &apos;biological process&apos;</rdfs:label>
    </owl:Class>
    


    <!-- http://purl.obolibrary.org/obo/upheno/patterns-dev/abnormallyPrematureBiologicalProcessInLocation.yaml -->

    <owl:Class rdf:about="http://purl.obolibrary.org/obo/upheno/patterns-dev/abnormallyPrematureBiologicalProcessInLocation.yaml">
        <rdfs:subClassOf rdf:resource="http://purl.obolibrary.org/obo/upheno/patterns-dev/abnormalBiologicalProcessInLocation.yaml"/>
        <rdfs:subClassOf rdf:resource="http://purl.obolibrary.org/obo/upheno/patterns-dev/abnormallyPrematureBiologicalProcess.yaml"/>
        <obo:IAO_0000115>An abnormally early start time of &apos;biological process&apos; in &apos;independent continuant&apos;.</obo:IAO_0000115>
        <terms:title>abnormallyPrematureBiologicalProcessInLocation</terms:title>
        <rdfs:label>premature &apos;biological process&apos; in &apos;independent continuant&apos;</rdfs:label>
    </owl:Class>
    


    <!-- http://purl.obolibrary.org/obo/upheno/patterns-dev/abnormallyProminentAnatomicalEntity.yaml -->

    <owl:Class rdf:about="http://purl.obolibrary.org/obo/upheno/patterns-dev/abnormallyProminentAnatomicalEntity.yaml">
        <rdfs:subClassOf rdf:resource="http://purl.obolibrary.org/obo/upheno/patterns-dev/abnormallyProtrudingAnatomicalEntity.yaml"/>
        <obo:IAO_0000115>Abnormal prominence of the &apos;anatomical entity&apos;.</obo:IAO_0000115>
        <terms:title>abnormallyProminentAnatomicalEntity</terms:title>
        <rdfs:label>prominent &apos;anatomical entity&apos;</rdfs:label>
    </owl:Class>
    


    <!-- http://purl.obolibrary.org/obo/upheno/patterns-dev/abnormallyProtrudingAnatomicalEntity.yaml -->

    <owl:Class rdf:about="http://purl.obolibrary.org/obo/upheno/patterns-dev/abnormallyProtrudingAnatomicalEntity.yaml">
        <rdfs:subClassOf rdf:resource="http://purl.obolibrary.org/obo/upheno/patterns-dev/abnormalAnatomicalEntityNotParts.yaml"/>
        <obo:IAO_0000115>An abnormally protruding &apos;anatomical_entity&apos; that extends out above or beyond an anatomical surface or boundary.</obo:IAO_0000115>
        <terms:title>abnormallyProtrudingAnatomicalEntity</terms:title>
        <oboInOwl:hasExactSynonym>abnormal &apos;anatomical_entity&apos; protrusion</oboInOwl:hasExactSynonym>
        <oboInOwl:hasExactSynonym>protruding &apos;anatomical_entity&apos;</oboInOwl:hasExactSynonym>
        <rdfs:label>abnormally protruding &apos;anatomical_entity&apos;</rdfs:label>
    </owl:Class>
    


    <!-- http://purl.obolibrary.org/obo/upheno/patterns-dev/abnormallyProtrudingAnatomicalEntityInLocation.yaml -->

    <owl:Class rdf:about="http://purl.obolibrary.org/obo/upheno/patterns-dev/abnormallyProtrudingAnatomicalEntityInLocation.yaml">
        <rdfs:subClassOf rdf:resource="http://purl.obolibrary.org/obo/upheno/patterns-dev/abnormallyProtrudingAnatomicalEntity.yaml"/>
        <obo:IAO_0000115>hernial protrusion of the &apos;anatomical entity&apos; through an opening or defect in the &apos;independent continuant&apos;.</obo:IAO_0000115>
        <terms:title>abnormallyProtrudingAnatomicalEntityInLocation</terms:title>
        <oboInOwl:hasExactSynonym>protruding &apos;anatomical entity&apos; in &apos;independent continuant&apos;</oboInOwl:hasExactSynonym>
        <rdfs:label>abnormal protrusion of &apos;anatomical entity&apos; through &apos;independent continuant&apos;</rdfs:label>
    </owl:Class>
    


    <!-- http://purl.obolibrary.org/obo/upheno/patterns-dev/abnormallyPunctateAnatomicalEntity.yaml -->

    <owl:Class rdf:about="http://purl.obolibrary.org/obo/upheno/patterns-dev/abnormallyPunctateAnatomicalEntity.yaml">
        <rdfs:subClassOf rdf:resource="http://purl.obolibrary.org/obo/upheno/patterns-dev/abnormalSpatialPatternOfAnatomicalEntity.yaml"/>
        <obo:IAO_0000115>The presence of abnormal dots, punctures, points or pits in &apos;anatomical_entity&apos;.</obo:IAO_0000115>
        <terms:title>abnormallyPunctateAnatomicalEntity</terms:title>
        <oboInOwl:hasRelatedSynonym>abnormally stippled &apos;anatomical_entity&apos;</oboInOwl:hasRelatedSynonym>
        <rdfs:label>abnormally punctate &apos;anatomical_entity&apos;</rdfs:label>
    </owl:Class>
    


    <!-- http://purl.obolibrary.org/obo/upheno/patterns-dev/abnormallyPunctateAnatomicalEntityInLocation.yaml -->

    <owl:Class rdf:about="http://purl.obolibrary.org/obo/upheno/patterns-dev/abnormallyPunctateAnatomicalEntityInLocation.yaml">
        <rdfs:subClassOf rdf:resource="http://purl.obolibrary.org/obo/upheno/patterns-dev/abnormalMorphologyOfAnatomicalEntityInLocation.yaml"/>
        <rdfs:subClassOf rdf:resource="http://purl.obolibrary.org/obo/upheno/patterns-dev/abnormallyPunctateAnatomicalEntity.yaml"/>
        <obo:IAO_0000115>The presence of abnormal dots, punctures, points or pits in &apos;anatomical_entity&apos; of &apos;independent_continuant&apos;.</obo:IAO_0000115>
        <terms:title>abnormallyPunctateAnatomicalEntityInLocation</terms:title>
        <oboInOwl:hasRelatedSynonym>abnormally stippled &apos;anatomical_entity&apos; of &apos;independent_continuant&apos;</oboInOwl:hasRelatedSynonym>
        <rdfs:label>abnormally punctate &apos;anatomical_entity&apos; of &apos;independent_continuant&apos;</rdfs:label>
    </owl:Class>
    


    <!-- http://purl.obolibrary.org/obo/upheno/patterns-dev/abnormallyRotatedAnatomicalEntity.yaml -->

    <owl:Class rdf:about="http://purl.obolibrary.org/obo/upheno/patterns-dev/abnormallyRotatedAnatomicalEntity.yaml">
        <rdfs:subClassOf rdf:resource="http://purl.obolibrary.org/obo/upheno/patterns-dev/abnormalSpatialPatternOfAnatomicalEntity.yaml"/>
        <obo:IAO_0000115>Abnormal rotation of the &apos;anatomical entity&apos;.</obo:IAO_0000115>
        <terms:title>abnormallyRotatedAnatomicalEntity</terms:title>
        <rdfs:label>rotated &apos;anatomical entity&apos;</rdfs:label>
    </owl:Class>
    


    <!-- http://purl.obolibrary.org/obo/upheno/patterns-dev/abnormallySegmentedAnatomicalEntityInLocation.yaml -->

    <owl:Class rdf:about="http://purl.obolibrary.org/obo/upheno/patterns-dev/abnormallySegmentedAnatomicalEntityInLocation.yaml">
        <rdfs:subClassOf rdf:resource="http://purl.obolibrary.org/obo/upheno/patterns-dev/abnormalMorphologyOfAnatomicalEntityInLocation.yaml"/>
        <obo:IAO_0000115>Abnormal segmentation of the &apos;anatomical entity&apos; in &apos;independent continuant&apos;.</obo:IAO_0000115>
        <terms:title>abnormallySegmentedAnatomicalEntityInLocation</terms:title>
        <oboInOwl:hasExactSynonym>segmented &apos;anatomical entity&apos; in &apos;independent continuant&apos;</oboInOwl:hasExactSynonym>
        <rdfs:label>abnormal segmentation of &apos;anatomical entity&apos; in &apos;independent continuant&apos;</rdfs:label>
    </owl:Class>
    


    <!-- http://purl.obolibrary.org/obo/upheno/patterns-dev/abscessInLocation.yaml -->

    <owl:Class rdf:about="http://purl.obolibrary.org/obo/upheno/patterns-dev/abscessInLocation.yaml">
        <rdfs:subClassOf rdf:resource="http://purl.obolibrary.org/obo/upheno/patterns/abnormalAnatomicalEntity.yaml"/>
        <obo:IAO_0000115>The presence of an abscess of the &apos;anatomical entity&apos;.</obo:IAO_0000115>
        <terms:title>abscessInLocation</terms:title>
        <rdfs:label>&apos;anatomical entity&apos; abscess</rdfs:label>
    </owl:Class>
    


    <!-- http://purl.obolibrary.org/obo/upheno/patterns-dev/aplasticAnatomicalEntity.yaml -->

    <owl:Class rdf:about="http://purl.obolibrary.org/obo/upheno/patterns-dev/aplasticAnatomicalEntity.yaml">
        <rdfs:subClassOf rdf:resource="http://purl.obolibrary.org/obo/upheno/patterns-dev/abnormalAgenesisOfAnatomicalEntity.yaml"/>
        <rdfs:subClassOf rdf:resource="http://purl.obolibrary.org/obo/upheno/patterns-dev/aplasticHypoplasticAnatomicalEntity.yaml"/>
        <obo:IAO_0000115>Congenital absence of the &apos;anatomical entity&apos;.</obo:IAO_0000115>
        <terms:title>aplasticAnatomicalEntity</terms:title>
        <oboInOwl:hasExactSynonym>aplasia of the &apos;anatomical entity&apos;</oboInOwl:hasExactSynonym>
        <rdfs:label>aplastic &apos;anatomical entity&apos;</rdfs:label>
    </owl:Class>
    


    <!-- http://purl.obolibrary.org/obo/upheno/patterns-dev/aplasticHypoplasticAnatomicalEntity.yaml -->

    <owl:Class rdf:about="http://purl.obolibrary.org/obo/upheno/patterns-dev/aplasticHypoplasticAnatomicalEntity.yaml">
        <rdfs:subClassOf rdf:resource="http://purl.obolibrary.org/obo/upheno/patterns-dev/abnormalAnatomicalEntityNotParts.yaml"/>
        <obo:IAO_0000115>Absence or underdevelopment of the &apos;anatomical entity&apos;.</obo:IAO_0000115>
        <terms:title>aplasticHypoplasticAnatomicalEntity</terms:title>
        <oboInOwl:hasExactSynonym>aplasia or hypoplasia affecting the &apos;anatomical entity&apos;</oboInOwl:hasExactSynonym>
        <rdfs:label>aplasia or hypoplasia of &apos;anatomical entity&apos;</rdfs:label>
    </owl:Class>
    


    <!-- http://purl.obolibrary.org/obo/upheno/patterns-dev/atreticAnatomicalEntity.yaml -->

    <owl:Class rdf:about="http://purl.obolibrary.org/obo/upheno/patterns-dev/atreticAnatomicalEntity.yaml">
        <rdfs:subClassOf rdf:resource="http://purl.obolibrary.org/obo/upheno/patterns-dev/abnormallyClosedAnatomicalEntity.yaml"/>
        <obo:IAO_0000115>A developmental defect resulting in complete obliteration of the lumen of the &apos;anatomical entity&apos;.</obo:IAO_0000115>
        <terms:title>atreticAnatomicalEntity</terms:title>
        <oboInOwl:hasExactSynonym>atresia of the &apos;anatomical entity&apos;</oboInOwl:hasExactSynonym>
        <rdfs:label>&apos;anatomical entity&apos; atresia</rdfs:label>
    </owl:Class>
    


    <!-- http://purl.obolibrary.org/obo/upheno/patterns-dev/atrophiedAnatomicalEntity.yaml -->

    <owl:Class rdf:about="http://purl.obolibrary.org/obo/upheno/patterns-dev/atrophiedAnatomicalEntity.yaml">
        <rdfs:subClassOf rdf:resource="http://purl.obolibrary.org/obo/upheno/patterns-dev/abnormallyDecreasedSizeOfAnatomicalEntity.yaml"/>
        <obo:IAO_0000115>Partial or complete wasting (loss) of &apos;anatomical entity&apos; tissue that was once present.</obo:IAO_0000115>
        <terms:title>atrophiedAnatomicalEntity</terms:title>
        <oboInOwl:hasExactSynonym>atrophy of the &apos;anatomical entity&apos;</oboInOwl:hasExactSynonym>
        <rdfs:label>&apos;anatomical entity&apos; atrophy</rdfs:label>
    </owl:Class>
    


    <!-- http://purl.obolibrary.org/obo/upheno/patterns-dev/blisteredAnatomicalEntity.yaml -->

    <owl:Class rdf:about="http://purl.obolibrary.org/obo/upheno/patterns-dev/blisteredAnatomicalEntity.yaml">
        <rdfs:subClassOf rdf:resource="http://purl.obolibrary.org/obo/upheno/patterns-dev/abnormalMorphologyOfAnatomicalEntity.yaml"/>
        <obo:IAO_0000115>Abnormal local accumulation of fluid underneath the surface causing a blistered &apos;anatomical entity&apos;.</obo:IAO_0000115>
        <terms:title>blisteredAnatomicalEntity</terms:title>
        <oboInOwl:hasExactSynonym>&apos;anatomical entity&apos; with blister</oboInOwl:hasExactSynonym>
        <rdfs:label>abnormally blistered &apos;anatomical entity&apos;</rdfs:label>
    </owl:Class>
    


    <!-- http://purl.obolibrary.org/obo/upheno/patterns-dev/blisteredAnatomicalEntityInLocation.yaml -->

    <owl:Class rdf:about="http://purl.obolibrary.org/obo/upheno/patterns-dev/blisteredAnatomicalEntityInLocation.yaml">
        <rdfs:subClassOf rdf:resource="http://purl.obolibrary.org/obo/upheno/patterns-dev/abnormalMorphologyOfAnatomicalEntityInLocation.yaml"/>
        <rdfs:subClassOf rdf:resource="http://purl.obolibrary.org/obo/upheno/patterns-dev/blisteredAnatomicalEntity.yaml"/>
        <obo:IAO_0000115>Abnormal local accumulation of fluid underneath the surface causing a blistered &apos;anatomical entity&apos; in &apos;independent continuant&apos;.</obo:IAO_0000115>
        <terms:title>blisteredAnatomicalEntityInLocation</terms:title>
        <oboInOwl:hasExactSynonym>&apos;independent continuant&apos; &apos;anatomical entity&apos; with blister</oboInOwl:hasExactSynonym>
        <rdfs:label>abnormally blistered &apos;anatomical entity&apos; in &apos;independent continuant&apos;</rdfs:label>
    </owl:Class>
    


    <!-- http://purl.obolibrary.org/obo/upheno/patterns-dev/brokenAnatomicalEntity.yaml -->

    <owl:Class rdf:about="http://purl.obolibrary.org/obo/upheno/patterns-dev/brokenAnatomicalEntity.yaml">
        <rdfs:subClassOf rdf:resource="http://purl.obolibrary.org/obo/upheno/patterns-dev/abnormalMorphologyOfAnatomicalEntity.yaml"/>
        <obo:IAO_0000115>A partial or complete breakage of the &apos;anatomical entity&apos;.</obo:IAO_0000115>
        <terms:title>brokenAnatomicalEntity</terms:title>
        <oboInOwl:hasExactSynonym>bone &apos;anatomical entity&apos;</oboInOwl:hasExactSynonym>
        <rdfs:label>broken &apos;anatomical entity&apos;</rdfs:label>
    </owl:Class>
    


    <!-- http://purl.obolibrary.org/obo/upheno/patterns-dev/calcifiedAnatomicalEntity.yaml -->

    <owl:Class rdf:about="http://purl.obolibrary.org/obo/upheno/patterns-dev/calcifiedAnatomicalEntity.yaml">
        <rdfs:subClassOf rdf:resource="http://purl.obolibrary.org/obo/upheno/patterns-dev/abnormalMorphologyOfAnatomicalEntity.yaml"/>
        <obo:IAO_0000115>Calcification of the &apos;anatomical entity&apos;.</obo:IAO_0000115>
        <terms:title>calcifiedAnatomicalEntity</terms:title>
        <oboInOwl:hasExactSynonym>calcified &apos;anatomical entity&apos;</oboInOwl:hasExactSynonym>
        <rdfs:label>&apos;anatomical entity&apos; calcification</rdfs:label>
    </owl:Class>
    


    <!-- http://purl.obolibrary.org/obo/upheno/patterns-dev/collapsedAnatomicalEntity.yaml -->

    <owl:Class rdf:about="http://purl.obolibrary.org/obo/upheno/patterns-dev/collapsedAnatomicalEntity.yaml">
        <rdfs:subClassOf rdf:resource="http://purl.obolibrary.org/obo/upheno/patterns-dev/abnormalMorphologyOfAnatomicalEntity.yaml"/>
        <obo:IAO_0000115>A structural failure that affects &apos;anatomical_entity&apos; so that it becomes flat or caved in.</obo:IAO_0000115>
        <terms:title>collapsedAnatomicalEntity</terms:title>
        <rdfs:label>collapsed &apos;anatomical_entity&apos;</rdfs:label>
    </owl:Class>
    


    <!-- http://purl.obolibrary.org/obo/upheno/patterns-dev/cystInLocation.yaml -->

    <owl:Class rdf:about="http://purl.obolibrary.org/obo/upheno/patterns-dev/cystInLocation.yaml">
        <rdfs:subClassOf rdf:resource="http://purl.obolibrary.org/obo/upheno/patterns-dev/abnormalMorphologyOfPartOfAnatomicalEntity.yaml"/>
        <obo:IAO_0000115>The presence of a cyst in the &apos;anatomical entity&apos;.</obo:IAO_0000115>
        <terms:title>cystInLocation</terms:title>
        <rdfs:label>&apos;anatomical entity&apos; cyst</rdfs:label>
    </owl:Class>
    


    <!-- http://purl.obolibrary.org/obo/upheno/patterns-dev/damagedAnatomicalEntityInLocation.yaml -->

    <owl:Class rdf:about="http://purl.obolibrary.org/obo/upheno/patterns-dev/damagedAnatomicalEntityInLocation.yaml">
        <rdfs:subClassOf rdf:resource="http://purl.obolibrary.org/obo/upheno/patterns-dev/abnormalMorphologyOfAnatomicalEntityInLocation.yaml"/>
        <obo:IAO_0000115>A damaged or injured &apos;anatomical entity&apos; in the &apos;independent continuant&apos;, that may lead to impaired function.</obo:IAO_0000115>
        <terms:title>damagedAnatomicalEntityInLocation</terms:title>
        <rdfs:label>damaged &apos;anatomical entity&apos; in the &apos;independent continuant&apos;</rdfs:label>
    </owl:Class>
    


    <!-- http://purl.obolibrary.org/obo/upheno/patterns-dev/decreasedProportionOfCellTypeInLocation.yaml -->

    <owl:Class rdf:about="http://purl.obolibrary.org/obo/upheno/patterns-dev/decreasedProportionOfCellTypeInLocation.yaml">
        <rdfs:subClassOf rdf:resource="http://purl.obolibrary.org/obo/upheno/patterns-dev/abnormalProportionOfCellTypeInLocation.yaml"/>
        <rdfs:subClassOf rdf:resource="http://purl.obolibrary.org/obo/upheno/patterns-dev/abnormalProportionOfCellTypeTowardsCellTypeInLocation.yaml"/>
        <obo:IAO_0000115>A decreased proportion of cell in the &apos;independent continuant&apos;.</obo:IAO_0000115>
        <terms:title>decreasedProportionOfCellTypeInLocation</terms:title>
        <rdfs:label>decreased proportion of cell in &apos;independent continuant&apos;</rdfs:label>
    </owl:Class>
    


    <!-- http://purl.obolibrary.org/obo/upheno/patterns-dev/decreasedProportionOfCellTypeTowardsCellTypeInLocation.yaml -->

    <owl:Class rdf:about="http://purl.obolibrary.org/obo/upheno/patterns-dev/decreasedProportionOfCellTypeTowardsCellTypeInLocation.yaml">
        <rdfs:subClassOf rdf:resource="http://purl.obolibrary.org/obo/upheno/patterns-dev/abnormalProportionOfCellTypeInLocation.yaml"/>
        <rdfs:subClassOf rdf:resource="http://purl.obolibrary.org/obo/upheno/patterns-dev/abnormalProportionOfCellTypeTowardsCellTypeInLocation.yaml"/>
        <obo:IAO_0000115>A decreased proportion of &apos;cell&apos; relative to &apos;cell&apos; in the &apos;independent continuant&apos;.</obo:IAO_0000115>
        <terms:title>decreasedProportionOfCellTypeTowardsCellTypeInLocation</terms:title>
        <rdfs:label>decreased proportion of &apos;cell&apos; relative to &apos;cell&apos; in &apos;independent continuant&apos;</rdfs:label>
    </owl:Class>
    


    <!-- http://purl.obolibrary.org/obo/upheno/patterns-dev/delaminatedAnatomicalEntity.yaml -->

    <owl:Class rdf:about="http://purl.obolibrary.org/obo/upheno/patterns-dev/delaminatedAnatomicalEntity.yaml">
        <rdfs:subClassOf rdf:resource="http://purl.obolibrary.org/obo/upheno/patterns-dev/abnormalMorphologyOfAnatomicalEntity.yaml"/>
        <obo:IAO_0000115>Separation of &apos;anatomical_entity&apos;, or its layers or sheets into constituent layers.</obo:IAO_0000115>
        <terms:title>delaminatedAnatomicalEntity</terms:title>
        <rdfs:label>delaminated &apos;anatomical_entity&apos;</rdfs:label>
    </owl:Class>
    


    <!-- http://purl.obolibrary.org/obo/upheno/patterns-dev/deviationTowardsLateralSideOfAnatomicalEntity.yaml -->

    <owl:Class rdf:about="http://purl.obolibrary.org/obo/upheno/patterns-dev/deviationTowardsLateralSideOfAnatomicalEntity.yaml">
        <rdfs:subClassOf rdf:resource="http://purl.obolibrary.org/obo/upheno/patterns-dev/spatialDeviationOfAnatomicalEntity.yaml"/>
        <obo:IAO_0000115>A changed direction of position or shift towards the side of &apos;anatomical_entity&apos;.</obo:IAO_0000115>
        <terms:title>deviationTowardsLateralSideOfAnatomicalEntity</terms:title>
        <oboInOwl:hasExactSynonym>&apos;anatomical_entity&apos; lateral deviation</oboInOwl:hasExactSynonym>
        <rdfs:label>lateral deviation of &apos;anatomical_entity&apos;</rdfs:label>
    </owl:Class>
    


    <!-- http://purl.obolibrary.org/obo/upheno/patterns-dev/deviationTowardsTheMedialSideOfAnatomicalEntity.yaml -->

    <owl:Class rdf:about="http://purl.obolibrary.org/obo/upheno/patterns-dev/deviationTowardsTheMedialSideOfAnatomicalEntity.yaml">
        <rdfs:subClassOf rdf:resource="http://purl.obolibrary.org/obo/upheno/patterns-dev/spatialDeviationOfAnatomicalEntity.yaml"/>
        <obo:IAO_0000115>A changed direction of position or shift towards the middle of &apos;anatomical_entity&apos;.</obo:IAO_0000115>
        <terms:title>deviationTowardsTheMedialSideOfAnatomicalEntity</terms:title>
        <oboInOwl:hasBroadSynonym>permanent bending of &apos;anatomical_entity&apos;</oboInOwl:hasBroadSynonym>
        <oboInOwl:hasBroadSynonym>shift of &apos;anatomical_entity&apos; towards the middle</oboInOwl:hasBroadSynonym>
        <rdfs:label>deviation of &apos;anatomical_entity&apos; towards the middle</rdfs:label>
    </owl:Class>
    


    <!-- http://purl.obolibrary.org/obo/upheno/patterns-dev/dislocatedAnatomicalEntity.yaml -->

    <owl:Class rdf:about="http://purl.obolibrary.org/obo/upheno/patterns-dev/dislocatedAnatomicalEntity.yaml">
        <rdfs:subClassOf rdf:resource="http://purl.obolibrary.org/obo/upheno/patterns-dev/abnormalPositionOfAnatomicalEntity.yaml"/>
        <obo:IAO_0000115>Dislocation or displacement of &apos;anatomical_entity&apos; from the place or position where it developed.</obo:IAO_0000115>
        <terms:title>dislocatedAnatomicalEntity</terms:title>
        <oboInOwl:hasExactSynonym>dislocation of &apos;anatomical_entity&apos;</oboInOwl:hasExactSynonym>
        <rdfs:label>&apos;anatomical_entity&apos; dislocation</rdfs:label>
    </owl:Class>
    


    <!-- http://purl.obolibrary.org/obo/upheno/patterns-dev/disorganizedAnatomicalEntity.yaml -->

    <owl:Class rdf:about="http://purl.obolibrary.org/obo/upheno/patterns-dev/disorganizedAnatomicalEntity.yaml">
        <rdfs:subClassOf rdf:resource="http://purl.obolibrary.org/obo/upheno/patterns-dev/abnormalMorphologyOfAnatomicalEntity.yaml"/>
        <obo:IAO_0000115>Disorganization of &apos;anatomical_entity&apos;.</obo:IAO_0000115>
        <terms:title>disorganizedAnatomicalEntity</terms:title>
        <oboInOwl:hasExactSynonym>&apos;anatomical_entity&apos; disarray</oboInOwl:hasExactSynonym>
        <rdfs:label>disorganized &apos;anatomical_entity&apos;</rdfs:label>
    </owl:Class>
    


    <!-- http://purl.obolibrary.org/obo/upheno/patterns-dev/dysplasticAnatomicalEntity.yaml -->

    <owl:Class rdf:about="http://purl.obolibrary.org/obo/upheno/patterns-dev/dysplasticAnatomicalEntity.yaml">
        <rdfs:subClassOf rdf:resource="http://purl.obolibrary.org/obo/upheno/patterns-dev/abnormalMorphologyOfAnatomicalEntity.yaml"/>
        <obo:IAO_0000115>Defective development of the &apos;anatomical entity&apos;.</obo:IAO_0000115>
        <terms:title>dysplasticAnatomicalEntity</terms:title>
        <oboInOwl:hasExactSynonym>&apos;anatomical entity&apos; dysgenesis</oboInOwl:hasExactSynonym>
        <rdfs:label>dysgenesis of the &apos;anatomical entity&apos;</rdfs:label>
    </owl:Class>
    


    <!-- http://purl.obolibrary.org/obo/upheno/patterns-dev/edematousAnatomicalEntity.yaml -->

    <owl:Class rdf:about="http://purl.obolibrary.org/obo/upheno/patterns-dev/edematousAnatomicalEntity.yaml">
        <rdfs:subClassOf rdf:resource="http://purl.obolibrary.org/obo/upheno/patterns-dev/abnormalMorphologyOfAnatomicalEntity.yaml"/>
        <obo:IAO_0000115>Abnormal accumulation of fluid in &apos;anatomical_entity&apos;.</obo:IAO_0000115>
        <terms:title>edematousAnatomicalEntity</terms:title>
        <oboInOwl:hasExactSynonym>edema in &apos;anatomical_entity&apos;</oboInOwl:hasExactSynonym>
        <oboInOwl:hasExactSynonym>oedema in &apos;anatomical_entity&apos;</oboInOwl:hasExactSynonym>
        <rdfs:label>edematous &apos;anatomical_entity&apos;</rdfs:label>
    </owl:Class>
    


    <!-- http://purl.obolibrary.org/obo/upheno/patterns-dev/exsertedAnatomicalEntity.yaml -->

    <owl:Class rdf:about="http://purl.obolibrary.org/obo/upheno/patterns-dev/exsertedAnatomicalEntity.yaml">
        <rdfs:subClassOf rdf:resource="http://purl.obolibrary.org/obo/upheno/patterns-dev/abnormallyProtrudingAnatomicalEntity.yaml"/>
        <obo:IAO_0000115>An exserted &apos;anatomical_entity&apos; is protruding or projecting from the body abnormally.</obo:IAO_0000115>
        <terms:title>exsertedAnatomicalEntity</terms:title>
        <oboInOwl:hasExactSynonym>protuberant &apos;anatomical_entity&apos;</oboInOwl:hasExactSynonym>
        <oboInOwl:hasNarrowSynonym>&apos;anatomical_entity&apos; prolapse</oboInOwl:hasNarrowSynonym>
        <oboInOwl:hasNarrowSynonym>prolapsed &apos;anatomical_entity&apos;</oboInOwl:hasNarrowSynonym>
        <rdfs:label>exserted &apos;anatomical_entity&apos;</rdfs:label>
    </owl:Class>
    


    <!-- http://purl.obolibrary.org/obo/upheno/patterns-dev/fibroticAnatomicalEntity.yaml -->

    <owl:Class rdf:about="http://purl.obolibrary.org/obo/upheno/patterns-dev/fibroticAnatomicalEntity.yaml">
        <rdfs:subClassOf rdf:resource="http://purl.obolibrary.org/obo/upheno/patterns-dev/abnormalMorphologyOfAnatomicalEntity.yaml"/>
        <obo:IAO_0000115>The presence of excessive fibrous connective tissue in the &apos;anatomical entity&apos;.</obo:IAO_0000115>
        <terms:title>fibroticAnatomicalEntity</terms:title>
        <oboInOwl:hasExactSynonym>Fibrosis of the &apos;anatomical entity&apos;</oboInOwl:hasExactSynonym>
        <rdfs:label>&apos;anatomical entity&apos; fibrosis</rdfs:label>
    </owl:Class>
    


    <!-- http://purl.obolibrary.org/obo/upheno/patterns-dev/foldedAnatomicalEntity.yaml -->

    <owl:Class rdf:about="http://purl.obolibrary.org/obo/upheno/patterns-dev/foldedAnatomicalEntity.yaml">
        <rdfs:subClassOf rdf:resource="http://purl.obolibrary.org/obo/upheno/patterns-dev/abnormalShapeOfAnatomicalEntityByShapeType.yaml"/>
        <obo:IAO_0000115>A morphological anomaly that involves folding all or any part of &apos;anatomical_entity&apos; over another connected part.</obo:IAO_0000115>
        <terms:title>foldedAnatomicalEntity</terms:title>
        <oboInOwl:hasExactSynonym>abnormally folded &apos;anatomical_entity&apos;</oboInOwl:hasExactSynonym>
        <rdfs:label>folded &apos;anatomical_entity&apos;</rdfs:label>
    </owl:Class>
    


    <!-- http://purl.obolibrary.org/obo/upheno/patterns-dev/fracturedAnatomicalEntity.yaml -->

    <owl:Class rdf:about="http://purl.obolibrary.org/obo/upheno/patterns-dev/fracturedAnatomicalEntity.yaml">
        <rdfs:subClassOf rdf:resource="http://purl.obolibrary.org/obo/upheno/patterns-dev/brokenAnatomicalEntity.yaml"/>
        <obo:IAO_0000115>A partial or complete fracture of the &apos;anatomical entity&apos;.</obo:IAO_0000115>
        <terms:title>fracturedAnatomicalEntity</terms:title>
        <oboInOwl:hasExactSynonym>bone &apos;anatomical entity&apos;</oboInOwl:hasExactSynonym>
        <rdfs:label>fractured &apos;anatomical entity&apos;</rdfs:label>
    </owl:Class>
    


    <!-- http://purl.obolibrary.org/obo/upheno/patterns-dev/fracturedAnatomicalEntityByFractureType.yaml -->

    <owl:Class rdf:about="http://purl.obolibrary.org/obo/upheno/patterns-dev/fracturedAnatomicalEntityByFractureType.yaml">
        <rdfs:subClassOf rdf:resource="http://purl.obolibrary.org/obo/upheno/patterns-dev/brokenAnatomicalEntity.yaml"/>
        <obo:IAO_0000115>A &apos;anatomical entity&apos; that is fractured.</obo:IAO_0000115>
        <terms:title>fracturedAnatomicalEntityByFractureType</terms:title>
        <rdfs:label>fractured &apos;anatomical entity&apos;</rdfs:label>
    </owl:Class>
    


    <!-- http://purl.obolibrary.org/obo/upheno/patterns-dev/herniatedAnatomicalEntity.yaml -->

    <owl:Class rdf:about="http://purl.obolibrary.org/obo/upheno/patterns-dev/herniatedAnatomicalEntity.yaml">
        <rdfs:subClassOf rdf:resource="http://purl.obolibrary.org/obo/upheno/patterns-dev/abnormallyProtrudingAnatomicalEntity.yaml"/>
        <obo:IAO_0000115>A herniated &apos;anatomical_entity&apos; which protrudes through an abnormal opening in the wall or tissue layer that contains it.</obo:IAO_0000115>
        <terms:title>herniatedAnatomicalEntity</terms:title>
        <oboInOwl:hasExactSynonym>&apos;anatomical_entity&apos; hernia</oboInOwl:hasExactSynonym>
        <oboInOwl:hasExactSynonym>hernia of &apos;anatomical_entity&apos;</oboInOwl:hasExactSynonym>
        <rdfs:label>herniated &apos;anatomical_entity&apos;</rdfs:label>
    </owl:Class>
    


    <!-- http://purl.obolibrary.org/obo/upheno/patterns-dev/hyperplasticAnatomicalEntity.yaml -->

    <owl:Class rdf:about="http://purl.obolibrary.org/obo/upheno/patterns-dev/hyperplasticAnatomicalEntity.yaml">
        <rdfs:subClassOf rdf:resource="http://purl.obolibrary.org/obo/upheno/patterns-dev/abnormalAnatomicalEntityNotParts.yaml"/>
        <obo:IAO_0000115>&apos;anatomical_entity&apos; shows abnormally increased number of cells in a tissue (hyperplasia) typically resulting in increased size.</obo:IAO_0000115>
        <terms:title>hyperplasticAnatomicalEntity.yaml</terms:title>
        <oboInOwl:hasExactSynonym>hyperplastic &apos;anatomical_entity&apos;</oboInOwl:hasExactSynonym>
        <rdfs:label>&apos;anatomical_entity&apos; hyperplasia</rdfs:label>
    </owl:Class>
    


    <!-- http://purl.obolibrary.org/obo/upheno/patterns-dev/hypertrophicAnatomicalEntity.yaml -->

    <owl:Class rdf:about="http://purl.obolibrary.org/obo/upheno/patterns-dev/hypertrophicAnatomicalEntity.yaml">
        <rdfs:subClassOf rdf:resource="http://purl.obolibrary.org/obo/upheno/patterns-dev/abnormallyIncreasedVolumeOfAnatomicalEntity.yaml"/>
        <obo:IAO_0000115>Increased size of &apos;multicellular_anatomical_structure&apos; due to overgrowth and enlargement of its constituent cells.</obo:IAO_0000115>
        <terms:title>hypertrophicAnatomicalEntity</terms:title>
        <oboInOwl:hasExactSynonym>&apos;multicellular_anatomical_structure&apos; hypertrophy</oboInOwl:hasExactSynonym>
        <rdfs:label>hypertrophic &apos;multicellular_anatomical_structure&apos;</rdfs:label>
    </owl:Class>
    


    <!-- http://purl.obolibrary.org/obo/upheno/patterns-dev/hypoplasticAnatomicalEntity.yaml -->

    <owl:Class rdf:about="http://purl.obolibrary.org/obo/upheno/patterns-dev/hypoplasticAnatomicalEntity.yaml">
        <rdfs:subClassOf rdf:resource="http://purl.obolibrary.org/obo/upheno/patterns-dev/aplasticHypoplasticAnatomicalEntity.yaml"/>
        <obo:IAO_0000115>Small, underdeveloped &apos;anatomical entity&apos;.</obo:IAO_0000115>
        <terms:title>hypoplasticAnatomicalEntity</terms:title>
        <oboInOwl:hasExactSynonym>hypoplastic &apos;anatomical entity&apos;</oboInOwl:hasExactSynonym>
        <rdfs:label>&apos;anatomical entity&apos; hypoplasia</rdfs:label>
    </owl:Class>
    


    <!-- http://purl.obolibrary.org/obo/upheno/patterns-dev/hypoplasticAnatomicalEntityInLocation.yaml -->

    <owl:Class rdf:about="http://purl.obolibrary.org/obo/upheno/patterns-dev/hypoplasticAnatomicalEntityInLocation.yaml">
        <rdfs:subClassOf rdf:resource="http://purl.obolibrary.org/obo/upheno/patterns-dev/hypoplasticAnatomicalEntity.yaml"/>
        <obo:IAO_0000115>Small, underdeveloped &apos;anatomical entity&apos; in &apos;independent continuant&apos;.</obo:IAO_0000115>
        <terms:title>hypoplasticAnatomicalEntityInLocation</terms:title>
        <oboInOwl:hasExactSynonym>&apos;independent continuant&apos; with hypoplastic &apos;anatomical entity&apos;</oboInOwl:hasExactSynonym>
        <rdfs:label>&apos;anatomical entity&apos; hypoplasia in &apos;independent continuant&apos;</rdfs:label>
    </owl:Class>
    


    <!-- http://purl.obolibrary.org/obo/upheno/patterns-dev/increasedProportionOfCellTypeInLocation.yaml -->

    <owl:Class rdf:about="http://purl.obolibrary.org/obo/upheno/patterns-dev/increasedProportionOfCellTypeInLocation.yaml">
        <rdfs:subClassOf rdf:resource="http://purl.obolibrary.org/obo/upheno/patterns-dev/abnormalProportionOfCellTypeInLocation.yaml"/>
        <rdfs:subClassOf rdf:resource="http://purl.obolibrary.org/obo/upheno/patterns-dev/abnormalProportionOfCellTypeTowardsCellTypeInLocation.yaml"/>
        <obo:IAO_0000115>An increased proportion of &apos;cell&apos; in the &apos;independent continuant&apos;.</obo:IAO_0000115>
        <terms:title>increasedProportionOfCellTypeInLocation</terms:title>
        <rdfs:label>increased proportion of &apos;cell&apos; in &apos;independent continuant&apos;</rdfs:label>
    </owl:Class>
    


    <!-- http://purl.obolibrary.org/obo/upheno/patterns-dev/increasedProportionOfCellTypeTowardsCellTypeInLocation.yaml -->

    <owl:Class rdf:about="http://purl.obolibrary.org/obo/upheno/patterns-dev/increasedProportionOfCellTypeTowardsCellTypeInLocation.yaml">
        <rdfs:subClassOf rdf:resource="http://purl.obolibrary.org/obo/upheno/patterns-dev/abnormalProportionOfCellTypeInLocation.yaml"/>
        <rdfs:subClassOf rdf:resource="http://purl.obolibrary.org/obo/upheno/patterns-dev/abnormalProportionOfCellTypeTowardsCellTypeInLocation.yaml"/>
        <obo:IAO_0000115>An increased proportion of &apos;cell&apos; relative to &apos;cell&apos; in the &apos;independent continuant&apos;.</obo:IAO_0000115>
        <terms:title>increasedProportionOfCellTypeTowardsCellTypeInLocation</terms:title>
        <rdfs:label>increased proportion of &apos;cell&apos; relative to &apos;cell&apos; in &apos;independent continuant&apos;</rdfs:label>
    </owl:Class>
    


    <!-- http://purl.obolibrary.org/obo/upheno/patterns-dev/irregularMassDensityOfAnatomicalEntity.yaml -->

    <owl:Class rdf:about="http://purl.obolibrary.org/obo/upheno/patterns-dev/irregularMassDensityOfAnatomicalEntity.yaml">
        <rdfs:subClassOf rdf:resource="http://purl.obolibrary.org/obo/upheno/patterns-dev/abnormalMassDensityOfAnatomicalEntity.yaml"/>
        <obo:IAO_0000115>An irregularity in the mass density of &apos;anatomical_entity&apos;.</obo:IAO_0000115>
        <terms:title>irregularMassDensityOfAnatomicalEntity</terms:title>
        <oboInOwl:hasExactSynonym>irregularity of &apos;anatomical_entity&apos; mass density</oboInOwl:hasExactSynonym>
        <rdfs:label>irregular mass density of &apos;anatomical_entity&apos;</rdfs:label>
    </owl:Class>
    


    <!-- http://purl.obolibrary.org/obo/upheno/patterns-dev/ivoryAnatomicalEntity.yaml -->

    <owl:Class rdf:about="http://purl.obolibrary.org/obo/upheno/patterns-dev/ivoryAnatomicalEntity.yaml">
        <rdfs:subClassOf rdf:resource="http://purl.obolibrary.org/obo/upheno/patterns-dev/abnormallyIncreasedMassDensityOfAnatomicalEntity.yaml"/>
        <obo:IAO_0000115>An abnormal increase in the density of &apos;anatomical_entity&apos; resulting in increased degree of radiopacity (in X-rays).</obo:IAO_0000115>
        <terms:title>ivoryAnatomicalEntity</terms:title>
        <oboInOwl:hasExactSynonym>abnormal radiographic density of &apos;anatomical_entity&apos;</oboInOwl:hasExactSynonym>
        <rdfs:label>ivory &apos;anatomical_entity&apos;</rdfs:label>
    </owl:Class>
    


    <!-- http://purl.obolibrary.org/obo/upheno/patterns-dev/lesionedAnatomicalEntity.yaml -->

    <owl:Class rdf:about="http://purl.obolibrary.org/obo/upheno/patterns-dev/lesionedAnatomicalEntity.yaml">
        <rdfs:subClassOf rdf:resource="http://purl.obolibrary.org/obo/upheno/patterns-dev/abnormalMorphologyOfAnatomicalEntity.yaml"/>
        <obo:IAO_0000115>An abnormal &apos;anatomical entity&apos; with one or more lesions.</obo:IAO_0000115>
        <terms:title>lesionedAnatomicalEntity</terms:title>
        <oboInOwl:hasExactSynonym>&apos;anatomical entity&apos; with lesion(s)</oboInOwl:hasExactSynonym>
        <rdfs:label>lesion in &apos;anatomical entity&apos;</rdfs:label>
    </owl:Class>
    


    <!-- http://purl.obolibrary.org/obo/upheno/patterns-dev/lysedAnatomicalEntity.yaml -->

    <owl:Class rdf:about="http://purl.obolibrary.org/obo/upheno/patterns-dev/lysedAnatomicalEntity.yaml">
        <rdfs:subClassOf rdf:resource="http://purl.obolibrary.org/obo/upheno/patterns-dev/abnormalMorphologyOfAnatomicalEntity.yaml"/>
        <obo:IAO_0000115>&apos;anatomical entity&apos; with extensive cellular membrane destruction.</obo:IAO_0000115>
        <terms:title>lysedAnatomicalEntity</terms:title>
        <rdfs:label>abnormally lysed &apos;anatomical entity&apos;</rdfs:label>
    </owl:Class>
    


    <!-- http://purl.obolibrary.org/obo/upheno/patterns-dev/malformedAnatomicalEntity.yaml -->

    <owl:Class rdf:about="http://purl.obolibrary.org/obo/upheno/patterns-dev/malformedAnatomicalEntity.yaml">
        <rdfs:subClassOf rdf:resource="http://purl.obolibrary.org/obo/upheno/patterns-dev/abnormalMorphologyOfAnatomicalEntity.yaml"/>
        <obo:IAO_0000115>An abnormally formed/malformed &apos;anatomical entity&apos;.</obo:IAO_0000115>
        <terms:title>malformedAnatomicalEntity</terms:title>
        <oboInOwl:hasExactSynonym>malformed &apos;anatomical entity&apos;</oboInOwl:hasExactSynonym>
        <rdfs:label>abnormally formed &apos;anatomical entity&apos;</rdfs:label>
    </owl:Class>
    


    <!-- http://purl.obolibrary.org/obo/upheno/patterns-dev/malformedAnatomicalEntityByType.yaml -->

    <owl:Class rdf:about="http://purl.obolibrary.org/obo/upheno/patterns-dev/malformedAnatomicalEntityByType.yaml">
        <rdfs:subClassOf rdf:resource="http://purl.obolibrary.org/obo/upheno/patterns-dev/abnormalMorphologyOfAnatomicalEntity.yaml"/>
        <obo:IAO_0000115>A &apos;malformed&apos; &apos;anatomical entity&apos;.</obo:IAO_0000115>
        <terms:title>malformedAnatomicalEntityByType</terms:title>
        <rdfs:label>&apos;malformed&apos; &apos;anatomical entity&apos;</rdfs:label>
    </owl:Class>
    


    <!-- http://purl.obolibrary.org/obo/upheno/patterns-dev/malformedAnatomicalEntityInLocation.yaml -->

    <owl:Class rdf:about="http://purl.obolibrary.org/obo/upheno/patterns-dev/malformedAnatomicalEntityInLocation.yaml">
        <rdfs:subClassOf rdf:resource="http://purl.obolibrary.org/obo/upheno/patterns-dev/abnormalMorphologyOfAnatomicalEntityInLocation.yaml"/>
        <rdfs:subClassOf rdf:resource="http://purl.obolibrary.org/obo/upheno/patterns-dev/malformedAnatomicalEntity.yaml"/>
        <rdfs:subClassOf rdf:resource="http://purl.obolibrary.org/obo/upheno/patterns-dev/malformedAnatomicalEntityByType.yaml"/>
        <obo:IAO_0000115>An abnormally formed/malformed &apos;anatomical entity&apos; in &apos;independent continuant&apos;.</obo:IAO_0000115>
        <terms:title>malformedAnatomicalEntityInLocation</terms:title>
        <oboInOwl:hasExactSynonym>malformed &apos;anatomical entity&apos; in &apos;independent continuant&apos;</oboInOwl:hasExactSynonym>
        <rdfs:label>abnormally formed &apos;anatomical entity&apos; in &apos;independent continuant&apos;</rdfs:label>
    </owl:Class>
    


    <!-- http://purl.obolibrary.org/obo/upheno/patterns-dev/metaplasticAnatomicalEntity.yaml -->

    <owl:Class rdf:about="http://purl.obolibrary.org/obo/upheno/patterns-dev/metaplasticAnatomicalEntity.yaml">
        <rdfs:subClassOf rdf:resource="http://purl.obolibrary.org/obo/upheno/patterns-dev/abnormalAnatomicalEntityNotParts.yaml"/>
        <obo:IAO_0000115>Abnormal change from one fully differentiated cellular state into another in &apos;anatomical entity&apos;.</obo:IAO_0000115>
        <terms:title>metaplasticAnatomicalEntity</terms:title>
        <rdfs:label>metaplastic &apos;anatomical entity&apos;</rdfs:label>
    </owl:Class>
    


    <!-- http://purl.obolibrary.org/obo/upheno/patterns-dev/mislocalisedAnatomicalEntity.yaml -->

    <owl:Class rdf:about="http://purl.obolibrary.org/obo/upheno/patterns-dev/mislocalisedAnatomicalEntity.yaml">
        <rdfs:subClassOf rdf:resource="http://purl.obolibrary.org/obo/upheno/patterns-dev/abnormalPositionOfAnatomicalEntity.yaml"/>
        <obo:IAO_0000115>An abnormally localised &apos;anatomical entity&apos;.</obo:IAO_0000115>
        <terms:title>mislocalisedAnatomicalEntity</terms:title>
        <oboInOwl:hasExactSynonym>abnormal position of &apos;anatomical entity&apos;</oboInOwl:hasExactSynonym>
        <rdfs:label>abnormally localised &apos;anatomical entity&apos;</rdfs:label>
    </owl:Class>
    


    <!-- http://purl.obolibrary.org/obo/upheno/patterns-dev/mislocalisedAnatomicalEntityInLocation.yaml -->

    <owl:Class rdf:about="http://purl.obolibrary.org/obo/upheno/patterns-dev/mislocalisedAnatomicalEntityInLocation.yaml">
        <rdfs:subClassOf rdf:resource="http://purl.obolibrary.org/obo/upheno/patterns-dev/abnormalPositionOfAnatomicalEntityInLocation.yaml"/>
        <rdfs:subClassOf rdf:resource="http://purl.obolibrary.org/obo/upheno/patterns-dev/mislocalisedAnatomicalEntity.yaml"/>
        <obo:IAO_0000115>Abnormal location of the &apos;anatomical entity&apos; in the &apos;independent continuant&apos;.</obo:IAO_0000115>
        <terms:title>mislocalisedAnatomicalEntityInLocation</terms:title>
        <oboInOwl:hasExactSynonym>abnormal position of &apos;anatomical entity&apos; in &apos;independent continuant&apos;</oboInOwl:hasExactSynonym>
        <rdfs:label>abnormally localised &apos;anatomical entity&apos; in &apos;independent continuant&apos;</rdfs:label>
    </owl:Class>
    


    <!-- http://purl.obolibrary.org/obo/upheno/patterns-dev/necroticAnatomicalEntity.yaml -->

    <owl:Class rdf:about="http://purl.obolibrary.org/obo/upheno/patterns-dev/necroticAnatomicalEntity.yaml">
        <rdfs:subClassOf rdf:resource="http://purl.obolibrary.org/obo/upheno/patterns-dev/abnormalMorphologyOfAnatomicalEntity.yaml"/>
        <obo:IAO_0000115>An abnormally necrotic &apos;anatomical entity&apos;.</obo:IAO_0000115>
        <terms:title>necroticAnatomicalEntity</terms:title>
        <rdfs:label>abnormally necrotic &apos;anatomical entity&apos;</rdfs:label>
    </owl:Class>
    


    <!-- http://purl.obolibrary.org/obo/upheno/patterns-dev/neoplasticAnatomicalEntity.yaml -->

    <owl:Class rdf:about="http://purl.obolibrary.org/obo/upheno/patterns-dev/neoplasticAnatomicalEntity.yaml">
        <rdfs:subClassOf rdf:resource="http://purl.obolibrary.org/obo/upheno/patterns-dev/abnormalMorphologyOfAnatomicalEntity.yaml"/>
        <obo:IAO_0000115>The presence of abnormally proliferating masses of cells in &apos;anatomical entity&apos;.</obo:IAO_0000115>
        <terms:title>neoplasticAnatomicalEntity</terms:title>
        <oboInOwl:hasExactSynonym>tumorous &apos;anatomical entity&apos;</oboInOwl:hasExactSynonym>
        <rdfs:label>neoplastic &apos;anatomical entity&apos;</rdfs:label>
    </owl:Class>
    


    <!-- http://purl.obolibrary.org/obo/upheno/patterns-dev/non-functionalAnatomicalEntity.yaml -->

    <owl:Class rdf:about="http://purl.obolibrary.org/obo/upheno/patterns-dev/non-functionalAnatomicalEntity.yaml">
        <rdfs:subClassOf rdf:resource="http://purl.obolibrary.org/obo/upheno/patterns-dev/abnormalFunctionalityOfAnatomicalEntity.yaml"/>
        <obo:IAO_0000115>Inability or failure of &apos;anatomical_entity&apos; to perform its regular function or functions.</obo:IAO_0000115>
        <terms:title>non-functionalAnatomicalEntity</terms:title>
        <oboInOwl:hasExactSynonym>&apos;anatomical_entity&apos; failure</oboInOwl:hasExactSynonym>
        <rdfs:label>non-functional &apos;anatomical_entity&apos;</rdfs:label>
    </owl:Class>
    


    <!-- http://purl.obolibrary.org/obo/upheno/patterns-dev/obstructedAnatomicalEntity.yaml -->

    <owl:Class rdf:about="http://purl.obolibrary.org/obo/upheno/patterns-dev/obstructedAnatomicalEntity.yaml">
        <rdfs:subClassOf rdf:resource="http://purl.obolibrary.org/obo/upheno/patterns-dev/abnormallyClosedAnatomicalEntity.yaml"/>
        <obo:IAO_0000115>Obstructed &apos;anatomical_entity&apos; due to it being blocked or filled with one or more obstacles.</obo:IAO_0000115>
        <terms:title>obstructedAnatomicalEntity</terms:title>
        <oboInOwl:hasExactSynonym>obstructed &apos;anatomical_entity&apos;</oboInOwl:hasExactSynonym>
        <oboInOwl:hasExactSynonym>obstruction of &apos;anatomical_entity&apos;</oboInOwl:hasExactSynonym>
        <rdfs:label>&apos;anatomical_entity&apos; obstruction</rdfs:label>
    </owl:Class>
    


    <!-- http://purl.obolibrary.org/obo/upheno/patterns-dev/paralysedAnatomicalEntity.yaml -->

    <owl:Class rdf:about="http://purl.obolibrary.org/obo/upheno/patterns-dev/paralysedAnatomicalEntity.yaml">
        <rdfs:subClassOf rdf:resource="http://purl.obolibrary.org/obo/upheno/patterns-dev/abnormalAnatomicalEntityNotParts.yaml"/>
        <obo:IAO_0000115>Complete loss of the ability to move &apos;anatomical entity&apos;.</obo:IAO_0000115>
        <terms:title>paralysedAnatomicalEntity</terms:title>
        <oboInOwl:hasExactSynonym>&apos;anatomical entity&apos; paralysis</oboInOwl:hasExactSynonym>
        <oboInOwl:hasExactSynonym>paralysis of &apos;anatomical entity&apos;</oboInOwl:hasExactSynonym>
        <rdfs:label>paralysed &apos;anatomical entity&apos;</rdfs:label>
    </owl:Class>
    


    <!-- http://purl.obolibrary.org/obo/upheno/patterns-dev/perforateAnatomicalEntity.yaml -->

    <owl:Class rdf:about="http://purl.obolibrary.org/obo/upheno/patterns-dev/perforateAnatomicalEntity.yaml">
        <rdfs:subClassOf rdf:resource="http://purl.obolibrary.org/obo/upheno/patterns-dev/abnormalMorphologyOfAnatomicalEntity.yaml"/>
        <obo:IAO_0000115>The presence of one or more abnormal holes in &apos;anatomical_entity&apos;.</obo:IAO_0000115>
        <terms:title>perforateAnatomicalEntity</terms:title>
        <oboInOwl:hasExactSynonym>perforated &apos;anatomical_entity&apos;</oboInOwl:hasExactSynonym>
        <rdfs:label>&apos;anatomical_entity&apos; perforation</rdfs:label>
    </owl:Class>
    


    <!-- http://purl.obolibrary.org/obo/upheno/patterns-dev/prematureClosureOfAnatomicalEntity.yaml -->

    <owl:Class rdf:about="http://purl.obolibrary.org/obo/upheno/patterns-dev/prematureClosureOfAnatomicalEntity.yaml">
        <rdfs:subClassOf rdf:resource="http://purl.obolibrary.org/obo/upheno/patterns-dev/abnormalAnatomicalEntityNotParts.yaml"/>
        <obo:IAO_0000115>Premature closure of &apos;anatomical_entity&apos;.</obo:IAO_0000115>
        <terms:title>prematureClosureOfAnatomicalEntity</terms:title>
        <oboInOwl:hasExactSynonym>premature closure of &apos;anatomical_entity&apos;</oboInOwl:hasExactSynonym>
        <rdfs:label>premature &apos;anatomical_entity&apos; closure</rdfs:label>
    </owl:Class>
    


    <!-- http://purl.obolibrary.org/obo/upheno/patterns-dev/spatialDeviationOfAnatomicalEntity.yaml -->

    <owl:Class rdf:about="http://purl.obolibrary.org/obo/upheno/patterns-dev/spatialDeviationOfAnatomicalEntity.yaml">
        <rdfs:subClassOf rdf:resource="http://purl.obolibrary.org/obo/upheno/patterns-dev/abnormalSpatialPatternOfAnatomicalEntity.yaml"/>
        <obo:IAO_0000115>Spatial deviation of &apos;anatomical_entity&apos; from its normal direction or position.</obo:IAO_0000115>
        <terms:title>spatialDeviationOfAnatomicalEntity</terms:title>
        <oboInOwl:hasExactSynonym>&apos;anatomical_entity&apos; deviation</oboInOwl:hasExactSynonym>
        <oboInOwl:hasExactSynonym>deviated &apos;anatomical_entity&apos;</oboInOwl:hasExactSynonym>
        <rdfs:label>deviation of &apos;anatomical_entity&apos;</rdfs:label>
    </owl:Class>
    


    <!-- http://purl.obolibrary.org/obo/upheno/patterns-dev/wrinkledAnatomicalEntity.yaml -->

    <owl:Class rdf:about="http://purl.obolibrary.org/obo/upheno/patterns-dev/wrinkledAnatomicalEntity.yaml">
        <rdfs:subClassOf rdf:resource="http://purl.obolibrary.org/obo/upheno/patterns-dev/abnormalMorphologyOfAnatomicalEntity.yaml"/>
        <obo:IAO_0000115>Wrinkled &apos;anatomical_entity&apos; displaying one or more creases in a normally smooth surface.</obo:IAO_0000115>
        <terms:title>wrinkledAnatomicalEntity</terms:title>
        <oboInOwl:hasExactSynonym>abnormally wrinkled &apos;anatomical_entity&apos;</oboInOwl:hasExactSynonym>
        <rdfs:label>wrinkled &apos;anatomical_entity&apos;</rdfs:label>
    </owl:Class>
    


    <!-- http://purl.obolibrary.org/obo/upheno/patterns/abnormalAnatomicalEntity.yaml -->

    <owl:Class rdf:about="http://purl.obolibrary.org/obo/upheno/patterns/abnormalAnatomicalEntity.yaml">
        <obo:IAO_0000115>Abnormality of &apos;anatomical entity&apos;.</obo:IAO_0000115>
        <terms:title>abnormalAnatomicalEntity</terms:title>
        <oboInOwl:hasExactSynonym>abnormality of &apos;anatomical entity&apos;</oboInOwl:hasExactSynonym>
        <rdfs:label>abnormal &apos;anatomical entity&apos;</rdfs:label>
    </owl:Class>
    


    <!-- http://purl.obolibrary.org/obo/upheno/patterns/abnormalCellularComponent.yaml -->

    <owl:Class rdf:about="http://purl.obolibrary.org/obo/upheno/patterns/abnormalCellularComponent.yaml">
        <obo:IAO_0000115>Abnormality of &apos;cellular component&apos;.</obo:IAO_0000115>
        <terms:title>abnormalCellularComponent</terms:title>
        <oboInOwl:hasExactSynonym>abnormality of &apos;cellular component&apos;</oboInOwl:hasExactSynonym>
        <rdfs:label>abnormal &apos;cellular component&apos;</rdfs:label>
    </owl:Class>
    


    <!-- http://purl.obolibrary.org/obo/upheno/patterns/abnormalHasExtraPartsOfTypeAnatomicalEntityInLocation.yaml -->

    <owl:Class rdf:about="http://purl.obolibrary.org/obo/upheno/patterns/abnormalHasExtraPartsOfTypeAnatomicalEntityInLocation.yaml">
        <rdfs:subClassOf rdf:resource="http://purl.obolibrary.org/obo/upheno/patterns-dev/abnormalHasExtraPartsOfTypeAnatomicalEntity.yaml"/>
        <rdfs:subClassOf rdf:resource="http://purl.obolibrary.org/obo/upheno/patterns-dev/abnormalMorphologyOfAnatomicalEntityInLocation.yaml"/>
        <rdfs:subClassOf rdf:resource="http://purl.obolibrary.org/obo/upheno/patterns-dev/abnormallyIncreasedNumberOfAnatomicalEntityInLocation.yaml"/>
        <obo:IAO_0000115>Any structural anomaly that causes there to be extra parts of type &apos;anatomical entity&apos; in &apos;independent continuant&apos;.</obo:IAO_0000115>
        <terms:title>abnormalHasExtraPartsOfTypeAnatomicalEntityInLocation</terms:title>
        <oboInOwl:hasExactSynonym>extra &apos;anatomical entity&apos;s in &apos;independent continuant&apos;</oboInOwl:hasExactSynonym>
        <rdfs:label>has extra parts of type &apos;anatomical entity&apos; in &apos;independent continuant&apos;</rdfs:label>
    </owl:Class>
    


    <!-- http://purl.obolibrary.org/obo/upheno/patterns/abnormalHasFewerPartsOfTypeAnatomicalEntityInLocation.yaml -->

    <owl:Class rdf:about="http://purl.obolibrary.org/obo/upheno/patterns/abnormalHasFewerPartsOfTypeAnatomicalEntityInLocation.yaml">
        <rdfs:subClassOf rdf:resource="http://purl.obolibrary.org/obo/upheno/patterns-dev/abnormalMorphologyOfAnatomicalEntity.yaml"/>
        <rdfs:subClassOf rdf:resource="http://purl.obolibrary.org/obo/upheno/patterns-dev/abnormallyDecreasedNumberOfAnatomicalEntity.yaml"/>
        <obo:IAO_0000115>Any structural anomaly that causes there to be fewer parts of type &apos;anatomical entity&apos; in the &apos;anatomical entity&apos;.</obo:IAO_0000115>
        <terms:title>abnormalHasFewerPartsOfTypeAnatomicalEntityInLocation</terms:title>
        <oboInOwl:hasExactSynonym>fewer &apos;anatomical entity&apos;s in &apos;anatomical entity&apos;, located in &apos;independent continuant&apos;</oboInOwl:hasExactSynonym>
        <rdfs:label>has fewer parts of type &apos;anatomical entity&apos; in &apos;anatomical entity&apos;, which is located in &apos;independent continuant&apos;</rdfs:label>
    </owl:Class>
    


    <!-- http://purl.obolibrary.org/obo/upheno/patterns/abnormalLevelOfChemicalEntity.yaml -->

    <owl:Class rdf:about="http://purl.obolibrary.org/obo/upheno/patterns/abnormalLevelOfChemicalEntity.yaml">
        <obo:IAO_0000115>An abnormal level of &apos;chemical entity&apos;.</obo:IAO_0000115>
        <terms:title>abnormalLevelOfChemicalEntity</terms:title>
        <rdfs:label>abnormal &apos;chemical entity&apos; level</rdfs:label>
    </owl:Class>
    


    <!-- http://purl.obolibrary.org/obo/upheno/patterns/abnormalLevelOfChemicalEntityInLocation.yaml -->

    <owl:Class rdf:about="http://purl.obolibrary.org/obo/upheno/patterns/abnormalLevelOfChemicalEntityInLocation.yaml">
        <rdfs:subClassOf rdf:resource="http://purl.obolibrary.org/obo/upheno/patterns/abnormalLevelOfChemicalEntity.yaml"/>
        <obo:IAO_0000115>An abnormal level of &apos;chemical entity&apos; in the &apos;independent continuant&apos;.</obo:IAO_0000115>
        <terms:title>abnormalLevelOfChemicalEntityInLocation</terms:title>
        <rdfs:label>abnormal &apos;independent continuant&apos; &apos;chemical entity&apos; level</rdfs:label>
    </owl:Class>
    


    <!-- http://purl.obolibrary.org/obo/upheno/patterns/abnormallyIncompleteClosureOfAnatomicalEntity.yaml -->

    <owl:Class rdf:about="http://purl.obolibrary.org/obo/upheno/patterns/abnormallyIncompleteClosureOfAnatomicalEntity.yaml">
        <rdfs:subClassOf rdf:resource="http://purl.obolibrary.org/obo/upheno/patterns-dev/abnormallyOpenAnatomicalEntity.yaml"/>
        <obo:IAO_0000115>Abnormally incompletely closed &apos;anatomical entity&apos;.</obo:IAO_0000115>
        <terms:title>abnormallyIncompleteClosureOfAnatomicalEntity</terms:title>
        <oboInOwl:hasExactSynonym>abnormally incompletely closed &apos;anatomical entity&apos;</oboInOwl:hasExactSynonym>
        <rdfs:label>abnormal incomplete closing of the &apos;anatomical entity&apos;</rdfs:label>
    </owl:Class>
    


    <!-- http://purl.obolibrary.org/obo/upheno/patterns/bifurcatedAnatomicalEntity.yaml -->

    <owl:Class rdf:about="http://purl.obolibrary.org/obo/upheno/patterns/bifurcatedAnatomicalEntity.yaml">
        <rdfs:subClassOf rdf:resource="http://purl.obolibrary.org/obo/upheno/patterns-dev/abnormalShapeOfAnatomicalEntityByShapeType.yaml"/>
        <obo:IAO_0000115>Bifurcation of the &apos;anatomical entity&apos;.</obo:IAO_0000115>
        <terms:title>bifurcatedAnatomicalEntity</terms:title>
        <oboInOwl:hasExactSynonym>&apos;anatomical entity&apos; bifurcation</oboInOwl:hasExactSynonym>
        <rdfs:label>bifurcated &apos;anatomical entity&apos;</rdfs:label>
    </owl:Class>
    


    <!-- http://purl.obolibrary.org/obo/upheno/patterns/bifurcatedAnatomicalEntityInLocation.yaml -->

    <owl:Class rdf:about="http://purl.obolibrary.org/obo/upheno/patterns/bifurcatedAnatomicalEntityInLocation.yaml">
        <rdfs:subClassOf rdf:resource="http://purl.obolibrary.org/obo/upheno/patterns-dev/abnormalShapeOfAnatomicalEntityByShapeTypeInLocation.yaml"/>
        <rdfs:subClassOf rdf:resource="http://purl.obolibrary.org/obo/upheno/patterns/bifurcatedAnatomicalEntity.yaml"/>
        <obo:IAO_0000115>Bifurcation of the &apos;anatomical entity&apos; in &apos;independent continuant&apos;.</obo:IAO_0000115>
        <terms:title>bifurcatedAnatomicalEntityInLocation</terms:title>
        <oboInOwl:hasExactSynonym>bifurcation of &apos;anatomical entity&apos; in &apos;independent continuant&apos;</oboInOwl:hasExactSynonym>
        <rdfs:label>bifurcated &apos;anatomical entity&apos; in &apos;independent continuant&apos;</rdfs:label>
    </owl:Class>
</rdf:RDF>



<!-- Generated by the OWL API (version 4.5.29) https://github.com/owlcs/owlapi -->

